<rdf:RDF
    xmlns:rdf="http://www.w3.org/1999/02/22-rdf-syntax-ns#"
    xmlns:dcterms="http://purl.org/dc/terms/"
    xmlns:s4ener="https://saref.etsi.org/saref4ener/"
    xmlns:time="http://www.w3.org/2006/time#"
    xmlns:owl="http://www.w3.org/2002/07/owl#"
    xmlns:rdfs="http://www.w3.org/2000/01/rdf-schema#"
    xmlns:saref="https://saref.etsi.org/core/"
    xmlns:vann="http://purl.org/vocab/vann/"
    xmlns:foaf="http://xmlns.com/foaf/0.1/"
    xmlns:xsd="http://www.w3.org/2001/XMLSchema#">
  <owl:Ontology rdf:about="https://saref.etsi.org/saref4ener/">
    <owl:versionIRI rdf:resource="https://saref.etsi.org/saref4ener/v1.2.1/"/>
    <dcterms:contributor>
      <owl:NamedIndividual rdf:about="https://www.linkedin.com/in/ana%C3%AFs-walle-050baa159/">
        <rdfs:label>Anais Walle</rdfs:label>
      </owl:NamedIndividual>
    </dcterms:contributor>
    <dcterms:creator rdf:resource="https://www.linkedin.com/in/giulia-biagioni"/>
    <vann:preferredNamespaceUri>https://saref.etsi.org/saref4ener/</vann:preferredNamespaceUri>
    <dcterms:license rdf:resource="https://forge.etsi.org/etsi-software-license"/>
    <owl:imports rdf:resource="https://saref.etsi.org/core/v3.1.1/"/>
    <dcterms:publisher rdf:resource="https://www.etsi.org/"/>
    <dcterms:creator rdf:resource="https://www.linkedin.com/in/lauradaniele"/>
    <dcterms:contributor>
      <owl:NamedIndividual rdf:about="https://www.linkedin.com/in/wilco-wijbrandi-3994ab4b/">
        <rdfs:label>Wilco Wijbrandi</rdfs:label>
      </owl:NamedIndividual>
    </dcterms:contributor>
    <dcterms:title xml:lang="en">SAREF for Energy Flexibility</dcterms:title>
    <dcterms:modified rdf:datatype="http://www.w3.org/2001/XMLSchema#date"
    >2023-03-29</dcterms:modified>
    <dcterms:contributor rdf:resource="https://www.linkedin.com/in/mente-konsman-b0a1711/"/>
    <owl:versionInfo>v1.2.1</owl:versionInfo>
    <dcterms:description xml:lang="en">The flexibility ontology module (ic-flex) is by design tightly integrated with SAREF, &#xD;
SAREF4ENER and the following InterConnect modules: power limit (ic-pwlm), &#xD;
incentive table (ic-inc), S2 (ic-s2), data-point (ic-data) and forecast (ic-fc) &#xD;
&#xD;
The main concept of the ic-flex module is the s4ener:FlexOffer, which allows to &#xD;
represent a flexibility offer (or schedule) as a combination of multiple time-series, data-points and forecasts. &#xD;
&#xD;
It also allows to specify a creation time (s4ener:hasCreationTime), validity &#xD;
period (s4ener:hasEffectivePeriod) and provenance (s4ener:producedBy) for &#xD;
the offer, on top of the creation time, validity period and provenance already specified for the time-series and data-points included in the offer.&#xD;
&#xD;
The additional key aspect captured in the ic-flex module is that a flex offer can also include various categories of flexibility, which are modelled as subclasses of the s4ener:FlexibilityProfile class, as follows:&#xD;
- Power Profile flexibilty is modelled as s4ener:PowerProfile based on the EEBUS spec&#xD;
- Tariff based flexibility (s4ener:TariffBased) is implemented using the incentive table (ic-inc) ontology based on the EEBUS spec (note that tariif-based felxibility does note exist in S2)&#xD;
- Power limit flexibility (ic-pwlm:PowerLimit) is implemented using  thepower limit (ic-pwlm) ontology based on the EEBUS spec (and compliant also with S2)&#xD;
- Power Envelope flexibility (s4ener:PowerEnvelope) is implemented using theS2 (ic-s2) that follows the S2 specification (and compliant also with EEBUS)&#xD;
- Demand driven flexibility (s4ener:DemandDriven)  flexibility (s4ener:PowerEnvelope) is implemented using theS2 (ic-s2) that follows the S2 specification (and compliant also with EEBUS)&#xD;
- Operation mode flexibility (s4ener:OperationMode) is implemented using theS2 (ic-s2) that follows the S2 specification (and compliant also with S2)&#xD;
- Fill rate based flexibility (s4ener:FillRateBased is implemented using theS2 (ic-s2) that follows the S2 specification (and compliant also with S2)</dcterms:description>
    <dcterms:creator rdf:resource="https://www.linkedin.com/in/bouterca/"/>
    <dcterms:contributor>
      <owl:NamedIndividual rdf:about="https://www.linkedin.com/in/georgjung/">
        <rdfs:label>Georg Jung</rdfs:label>
      </owl:NamedIndividual>
    </dcterms:contributor>
    <dcterms:contributor>
      <owl:NamedIndividual rdf:about="https://www.linkedin.com/in/josef-baumeister-a221422/">
        <rdfs:label>Josef Baumeister</rdfs:label>
      </owl:NamedIndividual>
    </dcterms:contributor>
    <dcterms:source rdf:resource="https://saref.etsi.org/sources/saref4ener/"/>
    <dcterms:contributor>
      <owl:NamedIndividual rdf:about="https://www.linkedin.com/in/george-hallak-368301157/">
        <rdfs:label>George Hallak</rdfs:label>
      </owl:NamedIndividual>
    </dcterms:contributor>
    <vann:preferredNamespacePrefix>s4ener</vann:preferredNamespacePrefix>
    <dcterms:issued rdf:datatype="http://www.w3.org/2001/XMLSchema#date"
    >2024-04-25</dcterms:issued>
    <rdfs:seeAlso rdf:resource="https://www.etsi.org/deliver/etsi_ts/103400_103499/10341001/01.02.01_60/ts_10341001v010201p.pdf"/>
    <owl:priorVersion rdf:resource="https://saref.etsi.org/saref4ener/v1.1.2/"/>
  </owl:Ontology>
  <rdfs:Class rdf:about="https://saref.etsi.org/saref4ener/AllowedLimitRange">
    <rdfs:subClassOf rdf:resource="http://www.w3.org/2002/07/owl#Thing"/>
    <rdfs:label xml:lang="en">Allowed limit range</rdfs:label>
    <rdfs:comment>The actual constraints of an Power Envelope Based Profile.</rdfs:comment>
  </rdfs:Class>
  <owl:Class rdf:about="https://saref.etsi.org/saref4ener/AnticipationDurationDescription">
    <owl:deprecated rdf:datatype="http://www.w3.org/2001/XMLSchema#boolean"
    >true</owl:deprecated>
    <rdfs:subClassOf>
      <owl:Class rdf:about="http://www.w3.org/2006/time#DurationDescription"/>
    </rdfs:subClassOf>
    <rdfs:label xml:lang="en">Anticipation duration description</rdfs:label>
    <rdfs:comment xml:lang="en">The duration description for the anticipation duration temporal entities</rdfs:comment>
  </owl:Class>
  <owl:Class rdf:about="https://saref.etsi.org/saref4ener/TimePeriodDurationDescription">
    <owl:deprecated rdf:datatype="http://www.w3.org/2001/XMLSchema#boolean"
    >true</owl:deprecated>
    <rdfs:subClassOf rdf:resource="http://www.w3.org/2006/time#DurationDescription"/>
    <rdfs:label xml:lang="en">Time period duration description</rdfs:label>
    <rdfs:comment xml:lang="en">The duration description for the time period duration temporal entities</rdfs:comment>
  </owl:Class>
  <owl:Class rdf:about="https://saref.etsi.org/saref4ener/DemandDrivenProfile">
    <rdfs:subClassOf>
      <owl:Class rdf:about="https://saref.etsi.org/saref4ener/FlexibilityProfile"/>
    </rdfs:subClassOf>
    <rdfs:label xml:lang="en">Demand driven control</rdfs:label>
    <rdfs:comment>The Flexibility Profile following the Demand Driven strategy.</rdfs:comment>
  </owl:Class>
  <owl:Class rdf:about="https://saref.etsi.org/saref4ener/ActuatorLevel">
    <rdfs:subClassOf rdf:resource="https://saref.etsi.org/core/Actuator"/>
    <rdfs:label xml:lang="en">Actuator level</rdfs:label>
    <rdfs:comment xml:lang="en">Independent from the ActuatorSwitch class, the ActuatorLevel class enables a user or application to model LEVEL commands (start, up, percentageAbsolute, relative, etc.). This can be used to dim a light, set the speed of an electric motor, etc.</rdfs:comment>
  </owl:Class>
  <owl:Class rdf:about="https://saref.etsi.org/saref4ener/ActivationDelayDurationDescription">
    <owl:deprecated rdf:datatype="http://www.w3.org/2001/XMLSchema#boolean"
    >true</owl:deprecated>
    <rdfs:subClassOf rdf:resource="http://www.w3.org/2006/time#DurationDescription"/>
    <rdfs:label xml:lang="en">Activation delay duration description</rdfs:label>
    <rdfs:comment xml:lang="en">The duration description for the activation delay duration temporal entity</rdfs:comment>
  </owl:Class>
  <owl:Class rdf:about="https://saref.etsi.org/saref4ener/PowerEnvelopeLimitType">
    <rdfs:subClassOf rdf:resource="http://www.w3.org/2002/07/owl#Thing"/>
    <rdfs:label xml:lang="en">Power Envelope Limit Type</rdfs:label>
    <rdfs:comment>An enumeration containing the codelist for Power Envelope Limit Types, which may be Lower limit or Upper limit.</rdfs:comment>
  </owl:Class>
  <owl:Class rdf:about="https://saref.etsi.org/saref4ener/FlexOffer">
    <rdfs:subClassOf>
      <owl:Restriction>
        <owl:onProperty>
          <owl:ObjectProperty rdf:about="https://saref.etsi.org/saref4ener/hasEffectivePeriod"/>
        </owl:onProperty>
        <owl:onClass>
          <owl:Class rdf:about="http://www.w3.org/2006/time#Interval"/>
        </owl:onClass>
        <owl:maxQualifiedCardinality rdf:datatype="http://www.w3.org/2001/XMLSchema#nonNegativeInteger"
        >1</owl:maxQualifiedCardinality>
      </owl:Restriction>
    </rdfs:subClassOf>
    <rdfs:subClassOf>
      <owl:Restriction>
        <owl:onProperty>
          <owl:DatatypeProperty rdf:about="https://saref.etsi.org/saref4ener/hasCreationTime"/>
        </owl:onProperty>
        <owl:maxCardinality rdf:datatype="http://www.w3.org/2001/XMLSchema#nonNegativeInteger"
        >1</owl:maxCardinality>
      </owl:Restriction>
    </rdfs:subClassOf>
    <rdfs:subClassOf>
      <owl:Restriction>
        <owl:onProperty>
          <owl:ObjectProperty rdf:about="https://saref.etsi.org/saref4ener/includes"/>
        </owl:onProperty>
        <owl:allValuesFrom>
          <owl:Class>
            <owl:unionOf rdf:parseType="Collection">
              <owl:Class rdf:about="https://saref.etsi.org/saref4ener/DataPoint"/>
              <owl:Class rdf:about="https://saref.etsi.org/saref4ener/TimeSeries"/>
              <owl:Class rdf:about="https://saref.etsi.org/saref4ener/FlexibilityProfile"/>
            </owl:unionOf>
          </owl:Class>
        </owl:allValuesFrom>
      </owl:Restriction>
    </rdfs:subClassOf>
    <rdfs:subClassOf>
      <owl:Restriction>
        <owl:onProperty>
          <owl:ObjectProperty rdf:about="https://saref.etsi.org/saref4ener/producedBy"/>
        </owl:onProperty>
        <owl:allValuesFrom>
          <owl:Class>
            <owl:unionOf rdf:parseType="Collection">
              <owl:Class rdf:about="http://xmlns.com/foaf/0.1/Agent"/>
              <rdf:Description rdf:about="https://saref.etsi.org/core/Device"/>
            </owl:unionOf>
          </owl:Class>
        </owl:allValuesFrom>
      </owl:Restriction>
    </rdfs:subClassOf>
    <rdfs:subClassOf>
      <owl:Restriction>
        <owl:onProperty>
          <owl:ObjectProperty rdf:about="https://saref.etsi.org/saref4ener/hasRecipient"/>
        </owl:onProperty>
        <owl:allValuesFrom>
          <owl:Class>
            <owl:unionOf rdf:parseType="Collection">
              <owl:Class rdf:about="http://xmlns.com/foaf/0.1/Agent"/>
              <rdf:Description rdf:about="https://saref.etsi.org/core/Device"/>
            </owl:unionOf>
          </owl:Class>
        </owl:allValuesFrom>
      </owl:Restriction>
    </rdfs:subClassOf>
    <rdfs:label xml:lang="en">Flex offer</rdfs:label>
    <rdfs:comment xml:lang="en">It  allows to represent a flexibility offer (or schedule) as a combination of multiple time-series, data-points and forecasts. For example, we can create a flexibility offer that includes a time-series ex:T-power of power values, combined with a time-series ex:T-costs of associated costs.</rdfs:comment>
  </owl:Class>
  <owl:Class rdf:about="https://saref.etsi.org/saref4ener/State">
    <rdfs:subClassOf rdf:resource="https://saref.etsi.org/core/State"/>
    <rdfs:label xml:lang="en">State</rdfs:label>
    <rdfs:comment xml:lang="en">An entity that represents the possible states in SAREF4EE</rdfs:comment>
  </owl:Class>
  <owl:Class rdf:about="https://saref.etsi.org/saref4ener/RemainingPauseTime">
    <owl:deprecated rdf:datatype="http://www.w3.org/2001/XMLSchema#boolean"
    >true</owl:deprecated>
    <rdfs:subClassOf>
      <owl:Class rdf:about="http://www.w3.org/2006/time#TemporalEntity"/>
    </rdfs:subClassOf>
    <rdfs:label xml:lang="en">Remaining pause time</rdfs:label>
    <rdfs:comment xml:lang="en">The duration that the current slot (s4ee:activeSlotNumber) permits being paused. This element SHALL ONLY be present if the power sequence is interruptible. Otherwise, it SHALL be omitted. In case the power sequence is interruptible the following rules apply: If the element is absent this means there is no explicit pause duration restriction for the current slot; a value of 0s denoted the slot does not permit being paused.</rdfs:comment>
  </owl:Class>
  <owl:Class rdf:about="https://saref.etsi.org/saref4ener/ActiveDurationMax">
    <owl:deprecated rdf:datatype="http://www.w3.org/2001/XMLSchema#boolean"
    >true</owl:deprecated>
    <rdfs:subClassOf rdf:resource="http://www.w3.org/2006/time#TemporalEntity"/>
    <rdfs:label xml:lang="en">Active duration max</rdfs:label>
    <rdfs:comment xml:lang="en">The active maximum duration a power sequence can run without interruption.</rdfs:comment>
  </owl:Class>
  <owl:Class rdf:about="https://saref.etsi.org/saref4ener/DurationUncertainty">
    <owl:deprecated rdf:datatype="http://www.w3.org/2001/XMLSchema#boolean"
    >true</owl:deprecated>
    <rdfs:subClassOf rdf:resource="http://www.w3.org/2006/time#TemporalEntity"/>
    <rdfs:label xml:lang="en">Duration uncertainty</rdfs:label>
    <rdfs:comment xml:lang="en">The uncertainty of the duration </rdfs:comment>
  </owl:Class>
  <owl:Class rdf:about="https://saref.etsi.org/saref4ener/PPBCInstruction">
    <rdfs:subClassOf>
      <owl:Class rdf:about="https://saref.etsi.org/saref4ener/FlexibilityInstruction"/>
    </rdfs:subClassOf>
    <rdfs:label xml:lang="en">Power Profile Based Control Instruction</rdfs:label>
    <rdfs:comment>An instruction for a Power Profile Based Flexibility Profile.</rdfs:comment>
  </owl:Class>
  <owl:Class rdf:about="https://saref.etsi.org/saref4ener/StartInterruptionInstruction">
    <rdfs:subClassOf>
      <owl:Class rdf:about="https://saref.etsi.org/saref4ener/InterruptionInstruction"/>
    </rdfs:subClassOf>
    <rdfs:label xml:lang="en">Start Interruption Instruction</rdfs:label>
    <rdfs:comment>An instruction or message indicating the start of an interruption.</rdfs:comment>
  </owl:Class>
  <owl:Class rdf:about="https://saref.etsi.org/saref4ener/ResumeCostEstimated">
    <rdfs:subClassOf rdf:resource="https://saref.etsi.org/core/Price"/>
    <rdfs:label xml:lang="en">Resume cost estimated</rdfs:label>
    <rdfs:comment xml:lang="en">In a power sequence the additional costs for the resumption of a device to its normal operation (after a pause).</rdfs:comment>
  </owl:Class>
  <owl:Class rdf:about="https://saref.etsi.org/saref4ener/MaxActivationDelay">
    <owl:deprecated rdf:datatype="http://www.w3.org/2001/XMLSchema#boolean"
    >true</owl:deprecated>
    <rdfs:subClassOf rdf:resource="http://www.w3.org/2006/time#TemporalEntity"/>
    <rdfs:label xml:lang="en">Max activation delay</rdfs:label>
    <rdfs:comment xml:lang="en">Maximum delay time between the end of the previous slot and the beginning of the current slot.</rdfs:comment>
  </owl:Class>
  <owl:Class rdf:about="https://saref.etsi.org/saref4ener/PauseTime">
    <owl:deprecated rdf:datatype="http://www.w3.org/2001/XMLSchema#boolean"
    >true</owl:deprecated>
    <rdfs:subClassOf rdf:resource="http://www.w3.org/2006/time#TemporalEntity"/>
    <rdfs:label xml:lang="en">Pause time</rdfs:label>
    <rdfs:comment xml:lang="en">The pause time of a power sequence or a slot</rdfs:comment>
  </owl:Class>
  <owl:Class rdf:about="https://saref.etsi.org/saref4ener/PowerRange">
    <rdfs:subClassOf rdf:resource="http://www.w3.org/2002/07/owl#Thing"/>
    <rdfs:label xml:lang="en">Power range</rdfs:label>
    <rdfs:comment>A class describing a power range, containing a start of range, an end of range, and a saref:Property indicating the type of power involved.</rdfs:comment>
  </owl:Class>
  <owl:Class rdf:about="https://saref.etsi.org/saref4ener/Energy">
    <rdfs:subClassOf rdf:resource="https://saref.etsi.org/core/Energy"/>
    <rdfs:label xml:lang="en">Energy</rdfs:label>
    <rdfs:comment xml:lang="en">Energy type and value in a slot (i.e., Energy, EnergyMin, EnergyMax, EnergyExpected, EnergyStandardDeviation, EnergySkewness); or the ResumeEnergyEstimated in a power sequence, i.e., the additional energy the device will consume before resuming its normal operation (after a pause)</rdfs:comment>
  </owl:Class>
  <owl:Class rdf:about="https://saref.etsi.org/saref4ener/PauseDurationDescription">
    <owl:deprecated rdf:datatype="http://www.w3.org/2001/XMLSchema#boolean"
    >true</owl:deprecated>
    <rdfs:subClassOf rdf:resource="http://www.w3.org/2006/time#DurationDescription"/>
    <rdfs:label xml:lang="en">Pause duration description</rdfs:label>
    <rdfs:comment xml:lang="en">The duration description for the pause duration (max and min) temporal entities</rdfs:comment>
  </owl:Class>
  <owl:Class rdf:about="https://saref.etsi.org/saref4ener/EnergyExpected">
    <rdfs:subClassOf rdf:resource="https://saref.etsi.org/saref4ener/Energy"/>
    <rdfs:label xml:lang="en">Energy expected</rdfs:label>
    <rdfs:comment xml:lang="en">A possible type of energy in a slot that represents the expected energy consumption and its value</rdfs:comment>
  </owl:Class>
  <owl:Class rdf:about="https://saref.etsi.org/saref4ener/PowerLimit">
    <rdfs:subClassOf>
      <owl:Restriction>
        <owl:onProperty>
          <owl:DatatypeProperty rdf:about="https://saref.etsi.org/saref4ener/isObligatory"/>
        </owl:onProperty>
        <owl:allValuesFrom rdf:resource="http://www.w3.org/2001/XMLSchema#boolean"/>
      </owl:Restriction>
    </rdfs:subClassOf>
    <rdfs:subClassOf>
      <owl:Restriction>
        <owl:onProperty>
          <owl:DatatypeProperty rdf:about="https://saref.etsi.org/saref4ener/isChangeable"/>
        </owl:onProperty>
        <owl:allValuesFrom rdf:resource="http://www.w3.org/2001/XMLSchema#boolean"/>
      </owl:Restriction>
    </rdfs:subClassOf>
    <rdfs:subClassOf rdf:resource="https://saref.etsi.org/saref4ener/AllowedLimitRange"/>
    <rdfs:label xml:lang="en">Power Limit</rdfs:label>
    <rdfs:comment xml:lang="en">A power limit is defined as the maximum value for power consumption and/or production that must not be exceeded by e.g. a (group of) device(s), a building, or also a district.</rdfs:comment>
  </owl:Class>
  <owl:Class rdf:about="https://saref.etsi.org/saref4ener/EndTimeDurationDescription">
    <rdfs:subClassOf rdf:resource="http://www.w3.org/2006/time#DurationDescription"/>
    <rdfs:label xml:lang="en">End time duration Description</rdfs:label>
    <rdfs:comment xml:lang="en">The duration description for the end time duration temporal entities</rdfs:comment>
  </owl:Class>
  <owl:Class rdf:about="https://saref.etsi.org/saref4ener/ScopeType">
    <rdfs:label xml:lang="en">Scope Type</rdfs:label>
    <rdfs:comment xml:lang="en">An incentive table may additionally define a scope type to indicate whether it is a preliminary or committed version.</rdfs:comment>
  </owl:Class>
  <owl:Class rdf:about="https://saref.etsi.org/saref4ener/LatestEndTime">
    <owl:deprecated rdf:datatype="http://www.w3.org/2001/XMLSchema#boolean"
    >true</owl:deprecated>
    <rdfs:subClassOf rdf:resource="http://www.w3.org/2006/time#TemporalEntity"/>
    <rdfs:label xml:lang="en">Latest end time</rdfs:label>
    <rdfs:comment xml:lang="en">The latest possible end time for a power sequence or a slot. Only 'xs:duration' value types SHALL be used to denote a relative time which relates to 'now' as time 0.&#xD;
Note: This element applies to the first repetition of the slot number only.</rdfs:comment>
  </owl:Class>
  <owl:Class rdf:about="https://saref.etsi.org/saref4ener/EnergyConstraint">
    <rdfs:label xml:lang="en">Energy Constraint</rdfs:label>
    <rdfs:comment>The energy constraint described in the Allowed Limit Range or Power Limit.</rdfs:comment>
  </owl:Class>
  <owl:Class rdf:about="https://saref.etsi.org/saref4ener/ValueSource">
    <rdfs:subClassOf rdf:resource="http://www.w3.org/2002/07/owl#Thing"/>
    <rdfs:label xml:lang="en">Value source</rdfs:label>
    <rdfs:comment>Indicates the source (origin/foundation) of the measurement forecasted values for a power sequence. If absent, the source is undefined. Remark: This element shall express the reliability of the forecast.</rdfs:comment>
  </owl:Class>
  <owl:Class rdf:about="https://saref.etsi.org/saref4ener/LeakageBehaviourElement">
    <rdfs:subClassOf rdf:resource="http://www.w3.org/2002/07/owl#Thing"/>
    <rdfs:label xml:lang="en">Leakage behaviour element</rdfs:label>
    <rdfs:comment>An element detailing the leakage behaviour of a storage.</rdfs:comment>
  </owl:Class>
  <owl:Class rdf:about="https://saref.etsi.org/saref4ener/EndInterruptionInstruction">
    <rdfs:subClassOf>
      <owl:Class rdf:about="https://saref.etsi.org/saref4ener/InterruptionInstruction"/>
    </rdfs:subClassOf>
    <rdfs:label xml:lang="en">End Interruption Instruction</rdfs:label>
    <rdfs:comment>An Instruction message indicating when an interruption can end.</rdfs:comment>
  </owl:Class>
  <owl:Class rdf:about="https://saref.etsi.org/saref4ener/DefaultDuration">
    <owl:deprecated rdf:datatype="http://www.w3.org/2001/XMLSchema#boolean"
    >true</owl:deprecated>
    <rdfs:subClassOf rdf:resource="http://www.w3.org/2006/time#TemporalEntity"/>
    <rdfs:label xml:lang="en">Default duration</rdfs:label>
    <rdfs:comment xml:lang="en">The duration of a slot (SHALL be present in case of 'determined slot'). If a slot has a configurable lenght, this element SHALL reflect the currently configured lenght</rdfs:comment>
  </owl:Class>
  <owl:Class rdf:about="https://saref.etsi.org/saref4ener/ValueTendency">
    <rdfs:subClassOf rdf:resource="http://www.w3.org/2002/07/owl#Thing"/>
    <rdfs:label xml:lang="en">Value tendency</rdfs:label>
    <rdfs:comment>This type indicates a codelist for the s4ener:valueTendency property about whether the tendency of a measurement is rising, stable or falling.</rdfs:comment>
  </owl:Class>
  <owl:Class rdf:about="https://saref.etsi.org/saref4ener/StartTimeDurationDescription">
    <owl:deprecated rdf:datatype="http://www.w3.org/2001/XMLSchema#boolean"
    >true</owl:deprecated>
    <rdfs:subClassOf rdf:resource="http://www.w3.org/2006/time#DurationDescription"/>
    <rdfs:label xml:lang="en">Start time duration description</rdfs:label>
    <rdfs:comment xml:lang="en">The duration description for the start time duration temporal entities</rdfs:comment>
  </owl:Class>
  <owl:Class rdf:about="https://saref.etsi.org/saref4ener/Role">
    <rdfs:subClassOf rdf:resource="http://www.w3.org/2002/07/owl#Thing"/>
    <rdfs:label xml:lang="en">Role</rdfs:label>
    <rdfs:comment>A codelist containing the various roles a device can take: producer, consumer, and storage.</rdfs:comment>
  </owl:Class>
  <owl:Class rdf:about="https://saref.etsi.org/saref4ener/StartTime">
    <owl:deprecated rdf:datatype="http://www.w3.org/2001/XMLSchema#boolean"
    >true</owl:deprecated>
    <rdfs:subClassOf rdf:resource="http://www.w3.org/2006/time#TemporalEntity"/>
    <rdfs:label xml:lang="en">Start time</rdfs:label>
    <rdfs:comment xml:lang="en">The startTime of a power sequence or slot. SHALL be present</rdfs:comment>
  </owl:Class>
  <owl:Class rdf:about="https://saref.etsi.org/saref4ener/MinDuration">
    <owl:deprecated rdf:datatype="http://www.w3.org/2001/XMLSchema#boolean"
    >true</owl:deprecated>
    <rdfs:subClassOf rdf:resource="http://www.w3.org/2006/time#TemporalEntity"/>
    <rdfs:label xml:lang="en">Min duration</rdfs:label>
    <rdfs:comment xml:lang="en">If a slot has a configurable duration, it SHALL be present and denote the minimum supported configuration. Note: This element applies to the first repetition of the slot number only.</rdfs:comment>
  </owl:Class>
  <owl:Class rdf:about="https://saref.etsi.org/saref4ener/PowerSkewness">
    <rdfs:subClassOf>
      <owl:Class rdf:about="https://saref.etsi.org/saref4ener/Power"/>
    </rdfs:subClassOf>
    <rdfs:label xml:lang="en">Power skewness</rdfs:label>
    <rdfs:comment xml:lang="en">A possible type of power in a slot that represents the power skewness and its value</rdfs:comment>
  </owl:Class>
  <owl:Class rdf:about="https://saref.etsi.org/saref4ener/EventActionProduce">
    <owl:oneOf rdf:parseType="Collection">
      <s4ener:EventActionProduce rdf:about="https://saref.etsi.org/saref4ener/Pause">
        <rdfs:label xml:lang="en">Pause</rdfs:label>
        <rdfs:comment xml:lang="en">Load control event action with value 'pause'</rdfs:comment>
        <rdf:type>
          <owl:Class rdf:about="https://saref.etsi.org/saref4ener/EventActionConsume"/>
        </rdf:type>
        <rdf:type rdf:resource="http://www.w3.org/2002/07/owl#NamedIndividual"/>
      </s4ener:EventActionProduce>
      <s4ener:EventActionProduce rdf:about="https://saref.etsi.org/saref4ener/Resume">
        <rdfs:label xml:lang="en">Resume</rdfs:label>
        <rdfs:comment xml:lang="en">Load control event action with value 'resume'</rdfs:comment>
        <rdf:type>
          <owl:Class rdf:about="https://saref.etsi.org/saref4ener/EventActionConsume"/>
        </rdf:type>
        <rdf:type rdf:resource="http://www.w3.org/2002/07/owl#NamedIndividual"/>
      </s4ener:EventActionProduce>
      <s4ener:EventActionProduce rdf:about="https://saref.etsi.org/saref4ener/Reduce">
        <rdfs:label xml:lang="en">Reduce</rdfs:label>
        <rdfs:comment xml:lang="en">Load control event action with value 'reduce'</rdfs:comment>
        <rdf:type>
          <owl:Class rdf:about="https://saref.etsi.org/saref4ener/EventActionConsume"/>
        </rdf:type>
        <rdf:type rdf:resource="http://www.w3.org/2002/07/owl#NamedIndividual"/>
      </s4ener:EventActionProduce>
      <s4ener:EventActionProduce rdf:about="https://saref.etsi.org/saref4ener/Increase">
        <rdfs:label xml:lang="en">Increase</rdfs:label>
        <rdfs:comment xml:lang="en">Load control event action with value 'increase'</rdfs:comment>
        <rdf:type>
          <owl:Class rdf:about="https://saref.etsi.org/saref4ener/EventActionConsume"/>
        </rdf:type>
        <rdf:type rdf:resource="http://www.w3.org/2002/07/owl#NamedIndividual"/>
      </s4ener:EventActionProduce>
      <s4ener:EventActionProduce rdf:about="https://saref.etsi.org/saref4ener/Emergency">
        <rdfs:label xml:lang="en">Emergency</rdfs:label>
        <rdfs:comment xml:lang="en">Load control event action with value 'emergency'</rdfs:comment>
        <rdf:type>
          <owl:Class rdf:about="https://saref.etsi.org/saref4ener/EventActionConsume"/>
        </rdf:type>
        <rdf:type rdf:resource="http://www.w3.org/2002/07/owl#NamedIndividual"/>
      </s4ener:EventActionProduce>
      <s4ener:EventActionProduce rdf:about="https://saref.etsi.org/saref4ener/Normal">
        <rdfs:label xml:lang="en">Normal</rdfs:label>
        <rdfs:comment xml:lang="en">The value NORMAL used to instantiate the Load Control Event Action class and MeasurandState class</rdfs:comment>
        <rdf:type>
          <owl:Class rdf:about="https://saref.etsi.org/saref4ener/EventActionConsume"/>
        </rdf:type>
        <rdf:type rdf:resource="http://www.w3.org/2002/07/owl#NamedIndividual"/>
      </s4ener:EventActionProduce>
    </owl:oneOf>
    <rdfs:subClassOf>
      <owl:Class rdf:about="https://saref.etsi.org/saref4ener/LoadControlEventAction"/>
    </rdfs:subClassOf>
    <rdfs:label xml:lang="en">Event action produce</rdfs:label>
    <rdfs:comment xml:lang="en">An action type used to express a produce action to be performed as a consequence of an event used to send overload warning severity level and related load control commands to a device (e.g. a household appliance or a smart meter).</rdfs:comment>
  </owl:Class>
  <owl:Class rdf:about="https://saref.etsi.org/saref4ener/PowerEnvelopeConsequenceType">
    <rdfs:subClassOf rdf:resource="http://www.w3.org/2002/07/owl#Thing"/>
    <rdfs:label xml:lang="en">Power Envelope Consequence Type</rdfs:label>
    <rdfs:comment>The type of consequence of limiting power, which can be Defer or Vanish.</rdfs:comment>
  </owl:Class>
  <owl:Class rdf:about="https://saref.etsi.org/saref4ener/PowerStandardDeviation">
    <rdfs:subClassOf>
      <owl:Class rdf:about="https://saref.etsi.org/saref4ener/Power"/>
    </rdfs:subClassOf>
    <rdfs:label xml:lang="en">Power standard deviation</rdfs:label>
    <rdfs:comment xml:lang="en">A possible type of power in a slot that represents the power standard deviation and its value</rdfs:comment>
  </owl:Class>
  <owl:Class rdf:about="https://saref.etsi.org/saref4ener/EndTime">
    <rdfs:subClassOf rdf:resource="http://www.w3.org/2006/time#TemporalEntity"/>
    <rdfs:label xml:lang="en">End time</rdfs:label>
    <rdfs:comment xml:lang="en">The endTime of a power sequence. If the value is available, it SHALL be denoted here. Otherwise the element SHALL be omitted.&#xD;
The end time of a slot MAY be stated in this element. The following equation SHALL apply: endTime - startTime = defaultDuration.</rdfs:comment>
  </owl:Class>
  <owl:Class rdf:about="https://saref.etsi.org/saref4ener/InterruptionInstruction">
    <rdfs:subClassOf rdf:resource="https://saref.etsi.org/saref4ener/PPBCInstruction"/>
    <rdfs:label xml:lang="en">Interruption Instruction</rdfs:label>
    <rdfs:comment>An instruction indicating an interruption to the process.</rdfs:comment>
  </owl:Class>
  <owl:Class rdf:about="https://saref.etsi.org/saref4ener/ActiveDurationDescription">
    <owl:deprecated rdf:datatype="http://www.w3.org/2001/XMLSchema#boolean"
    >true</owl:deprecated>
    <rdfs:subClassOf rdf:resource="http://www.w3.org/2006/time#DurationDescription"/>
    <rdfs:label xml:lang="en">Active duration description</rdfs:label>
    <rdfs:comment xml:lang="en">The duration description for the active duration (min and max, sum max and sum min) temporal entities</rdfs:comment>
  </owl:Class>
  <owl:Class rdf:about="https://saref.etsi.org/saref4ener/ActiveDurationSumMax">
    <owl:deprecated rdf:datatype="http://www.w3.org/2001/XMLSchema#boolean"
    >true</owl:deprecated>
    <rdfs:subClassOf rdf:resource="http://www.w3.org/2006/time#TemporalEntity"/>
    <rdfs:label xml:lang="en">Active duration sum max</rdfs:label>
    <rdfs:comment xml:lang="en">The active maximum duration a power sequence can run in total (summation of all active times).</rdfs:comment>
  </owl:Class>
  <owl:Class rdf:about="https://saref.etsi.org/saref4ener/PowerConstraint">
    <rdfs:subClassOf rdf:resource="http://www.w3.org/2002/07/owl#Thing"/>
    <rdfs:label xml:lang="en">Power constraint</rdfs:label>
    <rdfs:comment>The actual power constraint contained in the Allowed Limit Range or Power limit.</rdfs:comment>
  </owl:Class>
  <owl:Class rdf:about="https://saref.etsi.org/saref4ener/GaussianDataPoint">
    <rdfs:subClassOf>
      <owl:Restriction>
        <owl:someValuesFrom rdf:resource="http://www.w3.org/2001/XMLSchema#decimal"/>
        <owl:onProperty>
          <owl:DatatypeProperty rdf:about="https://saref.etsi.org/saref4ener/hasStandardDeviation"/>
        </owl:onProperty>
      </owl:Restriction>
    </rdfs:subClassOf>
    <rdfs:subClassOf>
      <owl:Class rdf:about="https://saref.etsi.org/saref4ener/DataPoint"/>
    </rdfs:subClassOf>
    <rdfs:label xml:lang="en">Gaussian data point</rdfs:label>
    <rdfs:comment xml:lang="en">A data point whose quantity is a standard deviation.</rdfs:comment>
  </owl:Class>
  <owl:Class rdf:about="https://saref.etsi.org/saref4ener/PauseDurationMin">
    <owl:deprecated rdf:datatype="http://www.w3.org/2001/XMLSchema#boolean"
    >true</owl:deprecated>
    <rdfs:subClassOf rdf:resource="http://www.w3.org/2006/time#TemporalEntity"/>
    <rdfs:label xml:lang="en">Pause duration min</rdfs:label>
    <rdfs:comment xml:lang="en">The minimum duration a power sequence can pause after the end of an activity.</rdfs:comment>
  </owl:Class>
  <owl:Class rdf:about="https://saref.etsi.org/saref4ener/PowerSequence">
    <rdfs:subClassOf>
      <owl:Restriction>
        <owl:onProperty>
          <owl:DatatypeProperty rdf:about="https://saref.etsi.org/saref4ener/isPausable"/>
        </owl:onProperty>
        <owl:maxCardinality rdf:datatype="http://www.w3.org/2001/XMLSchema#nonNegativeInteger"
        >1</owl:maxCardinality>
      </owl:Restriction>
    </rdfs:subClassOf>
    <rdfs:comment>A Power Sequence following S2 is a container containing one or more PowerSequenceElements among which the EMS can choose the Element with the best fit to the current energy demands.</rdfs:comment>
    <rdfs:subClassOf>
      <owl:Restriction>
        <owl:onProperty rdf:resource="https://saref.etsi.org/core/hasTime"/>
        <owl:onClass rdf:resource="https://saref.etsi.org/saref4ener/EndTime"/>
        <owl:maxQualifiedCardinality rdf:datatype="http://www.w3.org/2001/XMLSchema#nonNegativeInteger"
        >1</owl:maxQualifiedCardinality>
      </owl:Restriction>
    </rdfs:subClassOf>
    <rdfs:subClassOf>
      <owl:Restriction>
        <owl:onProperty rdf:resource="https://saref.etsi.org/core/hasTime"/>
        <owl:onClass rdf:resource="https://saref.etsi.org/saref4ener/LatestEndTime"/>
        <owl:maxQualifiedCardinality rdf:datatype="http://www.w3.org/2001/XMLSchema#nonNegativeInteger"
        >1</owl:maxQualifiedCardinality>
      </owl:Restriction>
    </rdfs:subClassOf>
    <rdfs:subClassOf>
      <owl:Restriction>
        <owl:onProperty rdf:resource="https://saref.etsi.org/core/consistsOf"/>
        <owl:onClass>
          <owl:Class rdf:about="https://saref.etsi.org/saref4ener/Slot"/>
        </owl:onClass>
        <owl:minQualifiedCardinality rdf:datatype="http://www.w3.org/2001/XMLSchema#nonNegativeInteger"
        >1</owl:minQualifiedCardinality>
      </owl:Restriction>
    </rdfs:subClassOf>
    <rdfs:subClassOf>
      <owl:Restriction>
        <owl:onProperty rdf:resource="https://saref.etsi.org/core/hasTime"/>
        <owl:onClass rdf:resource="https://saref.etsi.org/saref4ener/ActiveDurationSumMax"/>
        <owl:maxQualifiedCardinality rdf:datatype="http://www.w3.org/2001/XMLSchema#nonNegativeInteger"
        >1</owl:maxQualifiedCardinality>
      </owl:Restriction>
    </rdfs:subClassOf>
    <rdfs:subClassOf>
      <owl:Restriction>
        <owl:onProperty rdf:resource="https://saref.etsi.org/core/hasTime"/>
        <owl:onClass>
          <owl:Class rdf:about="https://saref.etsi.org/saref4ener/PauseDurationMax"/>
        </owl:onClass>
        <owl:maxQualifiedCardinality rdf:datatype="http://www.w3.org/2001/XMLSchema#nonNegativeInteger"
        >1</owl:maxQualifiedCardinality>
      </owl:Restriction>
    </rdfs:subClassOf>
    <rdfs:subClassOf>
      <owl:Restriction>
        <owl:onProperty rdf:resource="https://saref.etsi.org/core/hasTime"/>
        <owl:onClass rdf:resource="https://saref.etsi.org/saref4ener/PauseDurationMin"/>
        <owl:maxQualifiedCardinality rdf:datatype="http://www.w3.org/2001/XMLSchema#nonNegativeInteger"
        >1</owl:maxQualifiedCardinality>
      </owl:Restriction>
    </rdfs:subClassOf>
    <rdfs:subClassOf>
      <owl:Restriction>
        <owl:onProperty>
          <owl:DatatypeProperty rdf:about="https://saref.etsi.org/saref4ener/greenest"/>
        </owl:onProperty>
        <owl:maxCardinality rdf:datatype="http://www.w3.org/2001/XMLSchema#nonNegativeInteger"
        >1</owl:maxCardinality>
      </owl:Restriction>
    </rdfs:subClassOf>
    <rdfs:subClassOf>
      <owl:Restriction>
        <owl:qualifiedCardinality rdf:datatype="http://www.w3.org/2001/XMLSchema#nonNegativeInteger"
        >1</owl:qualifiedCardinality>
        <owl:onProperty>
          <owl:ObjectProperty rdf:about="https://saref.etsi.org/saref4ener/belongsTo"/>
        </owl:onProperty>
        <owl:onClass>
          <owl:Class rdf:about="https://saref.etsi.org/saref4ener/AlternativesGroup"/>
        </owl:onClass>
      </owl:Restriction>
    </rdfs:subClassOf>
    <rdfs:subClassOf>
      <owl:Restriction>
        <owl:onProperty>
          <owl:DatatypeProperty rdf:about="https://saref.etsi.org/saref4ener/isStoppable"/>
        </owl:onProperty>
        <owl:maxCardinality rdf:datatype="http://www.w3.org/2001/XMLSchema#nonNegativeInteger"
        >1</owl:maxCardinality>
      </owl:Restriction>
    </rdfs:subClassOf>
    <rdfs:comment xml:lang="en">The specification of a task, such as wash or tumble dry, according to user preferences and/or manufacturer's settings for a certain device.  It is the most 'coarse' view, a power sequence can represent all single steps of a whole task,where the single steps are represented by slots. If the power sequence is pausable by the bound power sequences client, the property 'saref:isInterruptionPossible' SHALL be present and set to true. Otherwise it SHALL be omitted. If the power sequence is stoppable by the bound power sequences client, the property 'saref:isFlexible' SHALL be present and set to true. Otherwise it SHALL be omitted.</rdfs:comment>
    <rdfs:subClassOf>
      <owl:Restriction>
        <owl:onProperty rdf:resource="https://saref.etsi.org/core/hasTime"/>
        <owl:onClass>
          <owl:Class rdf:about="https://saref.etsi.org/saref4ener/ActiveDurationSumMin"/>
        </owl:onClass>
        <owl:maxQualifiedCardinality rdf:datatype="http://www.w3.org/2001/XMLSchema#nonNegativeInteger"
        >1</owl:maxQualifiedCardinality>
      </owl:Restriction>
    </rdfs:subClassOf>
    <rdfs:subClassOf>
      <owl:Restriction>
        <owl:onProperty>
          <owl:DatatypeProperty rdf:about="https://saref.etsi.org/saref4ener/maxCyclesPerDay"/>
        </owl:onProperty>
        <owl:maxCardinality rdf:datatype="http://www.w3.org/2001/XMLSchema#nonNegativeInteger"
        >1</owl:maxCardinality>
      </owl:Restriction>
    </rdfs:subClassOf>
    <rdfs:subClassOf>
      <owl:Restriction>
        <owl:onProperty rdf:resource="https://saref.etsi.org/core/hasTime"/>
        <owl:onClass>
          <owl:Class rdf:about="https://saref.etsi.org/saref4ener/ElapsedSlotTime"/>
        </owl:onClass>
        <owl:maxQualifiedCardinality rdf:datatype="http://www.w3.org/2001/XMLSchema#nonNegativeInteger"
        >1</owl:maxQualifiedCardinality>
      </owl:Restriction>
    </rdfs:subClassOf>
    <rdfs:subClassOf>
      <owl:Restriction>
        <owl:onProperty rdf:resource="https://saref.etsi.org/core/hasDescription"/>
        <owl:maxCardinality rdf:datatype="http://www.w3.org/2001/XMLSchema#nonNegativeInteger"
        >1</owl:maxCardinality>
      </owl:Restriction>
    </rdfs:subClassOf>
    <rdfs:subClassOf>
      <owl:Restriction>
        <owl:onProperty>
          <owl:DatatypeProperty rdf:about="https://saref.etsi.org/saref4ener/activeRepetitionNumber"/>
        </owl:onProperty>
        <owl:maxCardinality rdf:datatype="http://www.w3.org/2001/XMLSchema#nonNegativeInteger"
        >1</owl:maxCardinality>
      </owl:Restriction>
    </rdfs:subClassOf>
    <rdfs:subClassOf>
      <owl:Restriction>
        <owl:onProperty rdf:resource="https://saref.etsi.org/core/hasTime"/>
        <owl:onClass rdf:resource="https://saref.etsi.org/saref4ener/StartTime"/>
        <owl:minQualifiedCardinality rdf:datatype="http://www.w3.org/2001/XMLSchema#nonNegativeInteger"
        >1</owl:minQualifiedCardinality>
      </owl:Restriction>
    </rdfs:subClassOf>
    <rdfs:subClassOf>
      <owl:Restriction>
        <owl:onProperty>
          <owl:ObjectProperty rdf:about="https://saref.etsi.org/saref4ener/belongsTo"/>
        </owl:onProperty>
        <owl:allValuesFrom>
          <owl:Class rdf:about="https://saref.etsi.org/saref4ener/AlternativesGroup"/>
        </owl:allValuesFrom>
      </owl:Restriction>
    </rdfs:subClassOf>
    <rdfs:subClassOf>
      <owl:Restriction>
        <owl:onProperty rdf:resource="https://saref.etsi.org/core/hasState"/>
        <owl:allValuesFrom>
          <owl:Class rdf:about="https://saref.etsi.org/saref4ener/PowerSequenceState"/>
        </owl:allValuesFrom>
      </owl:Restriction>
    </rdfs:subClassOf>
    <rdfs:subClassOf>
      <owl:Restriction>
        <owl:onProperty rdf:resource="https://saref.etsi.org/core/consistsOf"/>
        <owl:allValuesFrom>
          <owl:Class rdf:about="https://saref.etsi.org/saref4ener/Slot"/>
        </owl:allValuesFrom>
      </owl:Restriction>
    </rdfs:subClassOf>
    <rdfs:label xml:lang="en">Power sequence</rdfs:label>
    <rdfs:subClassOf>
      <owl:Restriction>
        <owl:onProperty>
          <owl:ObjectProperty rdf:about="https://saref.etsi.org/saref4ener/hasEnergy"/>
        </owl:onProperty>
        <owl:allValuesFrom>
          <owl:Class rdf:about="https://saref.etsi.org/saref4ener/ResumeEnergyEstimated"/>
        </owl:allValuesFrom>
      </owl:Restriction>
    </rdfs:subClassOf>
    <rdfs:subClassOf>
      <owl:Restriction>
        <owl:onProperty rdf:resource="https://saref.etsi.org/core/hasTime"/>
        <owl:onClass rdf:resource="https://saref.etsi.org/saref4ener/ActiveDurationMax"/>
        <owl:maxQualifiedCardinality rdf:datatype="http://www.w3.org/2001/XMLSchema#nonNegativeInteger"
        >1</owl:maxQualifiedCardinality>
      </owl:Restriction>
    </rdfs:subClassOf>
    <rdfs:subClassOf>
      <owl:Restriction>
        <owl:onProperty>
          <owl:DatatypeProperty rdf:about="https://saref.etsi.org/saref4ener/sequenceID"/>
        </owl:onProperty>
        <owl:cardinality rdf:datatype="http://www.w3.org/2001/XMLSchema#nonNegativeInteger"
        >1</owl:cardinality>
      </owl:Restriction>
    </rdfs:subClassOf>
    <rdfs:subClassOf>
      <owl:Restriction>
        <owl:onProperty>
          <owl:DatatypeProperty rdf:about="https://saref.etsi.org/saref4ener/sequenceRemoteControllable"/>
        </owl:onProperty>
        <owl:cardinality rdf:datatype="http://www.w3.org/2001/XMLSchema#nonNegativeInteger"
        >1</owl:cardinality>
      </owl:Restriction>
    </rdfs:subClassOf>
    <rdfs:subClassOf>
      <owl:Restriction>
        <owl:onProperty>
          <owl:ObjectProperty rdf:about="https://saref.etsi.org/saref4ener/hasValueSource"/>
        </owl:onProperty>
        <owl:minCardinality rdf:datatype="http://www.w3.org/2001/XMLSchema#nonNegativeInteger"
        >0</owl:minCardinality>
      </owl:Restriction>
    </rdfs:subClassOf>
    <rdfs:subClassOf>
      <owl:Restriction>
        <owl:onProperty rdf:resource="https://saref.etsi.org/core/hasPrice"/>
        <owl:onClass rdf:resource="https://saref.etsi.org/saref4ener/ResumeCostEstimated"/>
        <owl:maxQualifiedCardinality rdf:datatype="http://www.w3.org/2001/XMLSchema#nonNegativeInteger"
        >1</owl:maxQualifiedCardinality>
      </owl:Restriction>
    </rdfs:subClassOf>
    <rdfs:subClassOf>
      <owl:Restriction>
        <owl:onProperty rdf:resource="https://saref.etsi.org/core/hasTime"/>
        <owl:onClass>
          <owl:Class rdf:about="https://saref.etsi.org/saref4ener/EarliestStartTime"/>
        </owl:onClass>
        <owl:maxQualifiedCardinality rdf:datatype="http://www.w3.org/2001/XMLSchema#nonNegativeInteger"
        >1</owl:maxQualifiedCardinality>
      </owl:Restriction>
    </rdfs:subClassOf>
    <rdfs:subClassOf>
      <owl:Restriction>
        <owl:onProperty>
          <owl:DatatypeProperty rdf:about="https://saref.etsi.org/saref4ener/repetitionsTotal"/>
        </owl:onProperty>
        <owl:maxCardinality rdf:datatype="http://www.w3.org/2001/XMLSchema#nonNegativeInteger"
        >1</owl:maxCardinality>
      </owl:Restriction>
    </rdfs:subClassOf>
    <rdfs:subClassOf>
      <owl:Restriction>
        <owl:onProperty>
          <owl:ObjectProperty rdf:about="https://saref.etsi.org/saref4ener/hasEnergy"/>
        </owl:onProperty>
        <owl:onClass>
          <owl:Class rdf:about="https://saref.etsi.org/saref4ener/ResumeEnergyEstimated"/>
        </owl:onClass>
        <owl:maxQualifiedCardinality rdf:datatype="http://www.w3.org/2001/XMLSchema#nonNegativeInteger"
        >1</owl:maxQualifiedCardinality>
      </owl:Restriction>
    </rdfs:subClassOf>
    <rdfs:subClassOf>
      <owl:Restriction>
        <owl:onProperty rdf:resource="https://saref.etsi.org/core/hasTime"/>
        <owl:onClass>
          <owl:Class rdf:about="https://saref.etsi.org/saref4ener/RemainingSlotTime"/>
        </owl:onClass>
        <owl:maxQualifiedCardinality rdf:datatype="http://www.w3.org/2001/XMLSchema#nonNegativeInteger"
        >1</owl:maxQualifiedCardinality>
      </owl:Restriction>
    </rdfs:subClassOf>
    <rdfs:subClassOf>
      <owl:Restriction>
        <owl:onProperty rdf:resource="https://saref.etsi.org/core/hasState"/>
        <owl:onClass>
          <owl:Class rdf:about="https://saref.etsi.org/saref4ener/PowerSequenceState"/>
        </owl:onClass>
        <owl:minQualifiedCardinality rdf:datatype="http://www.w3.org/2001/XMLSchema#nonNegativeInteger"
        >1</owl:minQualifiedCardinality>
      </owl:Restriction>
    </rdfs:subClassOf>
    <rdfs:subClassOf rdf:resource="http://www.w3.org/2002/07/owl#Thing"/>
    <rdfs:subClassOf>
      <owl:Restriction>
        <owl:onProperty>
          <owl:DatatypeProperty rdf:about="https://saref.etsi.org/saref4ener/activeSlotNumber"/>
        </owl:onProperty>
        <owl:maxCardinality rdf:datatype="http://www.w3.org/2001/XMLSchema#nonNegativeInteger"
        >1</owl:maxCardinality>
      </owl:Restriction>
    </rdfs:subClassOf>
    <rdfs:subClassOf>
      <owl:Restriction>
        <owl:onProperty rdf:resource="https://saref.etsi.org/core/hasTime"/>
        <owl:onClass>
          <owl:Class rdf:about="https://saref.etsi.org/saref4ener/ActiveDurationMin"/>
        </owl:onClass>
        <owl:maxQualifiedCardinality rdf:datatype="http://www.w3.org/2001/XMLSchema#nonNegativeInteger"
        >1</owl:maxQualifiedCardinality>
      </owl:Restriction>
    </rdfs:subClassOf>
    <rdfs:subClassOf>
      <owl:Restriction>
        <owl:onProperty>
          <owl:DatatypeProperty rdf:about="https://saref.etsi.org/saref4ener/cheapest"/>
        </owl:onProperty>
        <owl:maxCardinality rdf:datatype="http://www.w3.org/2001/XMLSchema#nonNegativeInteger"
        >1</owl:maxCardinality>
      </owl:Restriction>
    </rdfs:subClassOf>
    <rdfs:subClassOf>
      <owl:Restriction>
        <owl:onProperty rdf:resource="https://saref.etsi.org/core/hasPrice"/>
        <owl:allValuesFrom rdf:resource="https://saref.etsi.org/saref4ener/ResumeCostEstimated"/>
      </owl:Restriction>
    </rdfs:subClassOf>
    <rdfs:subClassOf>
      <owl:Restriction>
        <owl:onProperty>
          <owl:DatatypeProperty rdf:about="https://saref.etsi.org/saref4ener/taskIdentifier"/>
        </owl:onProperty>
        <owl:minCardinality rdf:datatype="http://www.w3.org/2001/XMLSchema#nonNegativeInteger"
        >0</owl:minCardinality>
      </owl:Restriction>
    </rdfs:subClassOf>
  </owl:Class>
  <owl:Class rdf:about="https://saref.etsi.org/saref4ener/Storage">
    <rdfs:subClassOf>
      <owl:Class rdf:about="https://saref.etsi.org/saref4ener/Device"/>
    </rdfs:subClassOf>
    <rdfs:subClassOf rdf:resource="http://www.w3.org/2002/07/owl#Thing"/>
    <rdfs:label xml:lang="en">Storage</rdfs:label>
    <rdfs:comment>storage device which is the main component of Fill Rate Based Control type.). In the context of flexibility control and instructuons, a device shall be able to inform the CEM about its fill level, a measure of how full the storage is, and the lower and upper boundaries that the fill level should remain within. </rdfs:comment>
  </owl:Class>
  <owl:Class rdf:about="https://saref.etsi.org/saref4ener/FillLevelTargetProfileElement">
    <rdfs:subClassOf rdf:resource="http://www.w3.org/2002/07/owl#Thing"/>
    <rdfs:label xml:lang="en">Fill level target profile element</rdfs:label>
    <rdfs:comment>A description of the various Elements detailing the Fill Level Target Profile consists.</rdfs:comment>
  </owl:Class>
  <owl:Class rdf:about="https://saref.etsi.org/saref4ener/MaxDuration">
    <owl:deprecated rdf:datatype="http://www.w3.org/2001/XMLSchema#boolean"
    >true</owl:deprecated>
    <rdfs:subClassOf rdf:resource="http://www.w3.org/2006/time#TemporalEntity"/>
    <rdfs:label xml:lang="en">Max duration</rdfs:label>
    <rdfs:comment xml:lang="en">If a slot has a configurable duration, it SHALL be present and denote the maximum supported configuration. Note: This element applies to the first repetition of the slot number only</rdfs:comment>
  </owl:Class>
  <owl:Class rdf:about="https://saref.etsi.org/saref4ener/OperationModeElement">
    <rdfs:subClassOf rdf:resource="http://www.w3.org/2002/07/owl#Thing"/>
    <rdfs:label xml:lang="en">Operation Mode Element</rdfs:label>
    <rdfs:comment>Operation Mode Elements of a Fill Rate Based Control</rdfs:comment>
  </owl:Class>
  <owl:Class rdf:about="https://saref.etsi.org/saref4ener/ElapsedSlotTime">
    <rdfs:subClassOf rdf:resource="http://www.w3.org/2006/time#TemporalEntity"/>
    <rdfs:label xml:lang="en">Elapsed slot time</rdfs:label>
    <rdfs:comment xml:lang="en">If state is set to 'running' or 'paused' AND the slot is determined, this element CAN contain the time the slot has already been in 'running' state (this also means the value remains constant during a 'paused' state). Otherwise it SHALL be omitted.</rdfs:comment>
  </owl:Class>
  <owl:Class rdf:about="https://saref.etsi.org/saref4ener/IncentiveTableTier">
    <rdfs:subClassOf>
      <owl:Class rdf:about="https://saref.etsi.org/saref4ener/TimeSeries"/>
    </rdfs:subClassOf>
    <rdfs:label xml:lang="en">Incentive table tier</rdfs:label>
    <rdfs:comment>This concept specifies a Tier that an Incentive Table consists of. Each Tier indicates through a series of Boundaries the price per kilowatthour this incentive costs. For example, a tier may describe grid power, solar panel power, or surplus power.</rdfs:comment>
  </owl:Class>
  <owl:Class rdf:about="https://saref.etsi.org/saref4ener/Usage">
    <rdfs:label xml:lang="en">Usage</rdfs:label>
    <rdfs:comment xml:lang="en">The usage of a datapoint, time series or message.</rdfs:comment>
  </owl:Class>
  <owl:Class rdf:about="https://saref.etsi.org/saref4ener/PowerSequenceStatus">
    <rdfs:subClassOf rdf:resource="http://www.w3.org/2002/07/owl#Thing"/>
    <rdfs:label xml:lang="en">Power sequence status</rdfs:label>
    <rdfs:comment>A codelist for the various Power Sequence statuses.</rdfs:comment>
  </owl:Class>
  <owl:Class rdf:about="https://saref.etsi.org/saref4ener/FailsafeState">
    <rdfs:label xml:lang="en">Fail-safe state</rdfs:label>
    <rdfs:comment>State that indicates that the device currently is in its Fail-safe state. This means that it has lost its connection to a central energy manager. This may result in the device following stricter power limits.</rdfs:comment>
  </owl:Class>
  <owl:Class rdf:about="https://saref.etsi.org/saref4ener/DDBCInstruction">
    <rdfs:subClassOf>
      <owl:Class rdf:about="https://saref.etsi.org/saref4ener/FlexibilityInstruction"/>
    </rdfs:subClassOf>
    <rdfs:label xml:lang="en">Demand Driven Based Control Instruction</rdfs:label>
    <rdfs:comment>An Instruction as specified for an Demand Driven Based Control Profile.</rdfs:comment>
  </owl:Class>
  <owl:Class rdf:about="https://saref.etsi.org/saref4ener/DataPoint">
    <rdfs:subClassOf>
      <owl:Restriction>
        <owl:qualifiedCardinality rdf:datatype="http://www.w3.org/2001/XMLSchema#nonNegativeInteger"
        >1</owl:qualifiedCardinality>
        <owl:onProperty>
          <owl:ObjectProperty rdf:about="https://saref.etsi.org/saref4ener/hasEffectivePeriod"/>
        </owl:onProperty>
        <owl:onClass rdf:resource="http://www.w3.org/2006/time#Interval"/>
      </owl:Restriction>
    </rdfs:subClassOf>
    <rdfs:subClassOf>
      <owl:Restriction>
        <owl:onProperty>
          <owl:DatatypeProperty rdf:about="https://saref.etsi.org/saref4ener/hasUpdateRate"/>
        </owl:onProperty>
        <owl:maxCardinality rdf:datatype="http://www.w3.org/2001/XMLSchema#nonNegativeInteger"
        >1</owl:maxCardinality>
      </owl:Restriction>
    </rdfs:subClassOf>
    <rdfs:subClassOf>
      <owl:Restriction>
        <owl:onProperty>
          <owl:DatatypeProperty rdf:about="https://saref.etsi.org/saref4ener/hasQuantile"/>
        </owl:onProperty>
        <owl:maxCardinality rdf:datatype="http://www.w3.org/2001/XMLSchema#nonNegativeInteger"
        >1</owl:maxCardinality>
      </owl:Restriction>
    </rdfs:subClassOf>
    <rdfs:subClassOf>
      <owl:Restriction>
        <owl:onProperty>
          <owl:DatatypeProperty rdf:about="https://saref.etsi.org/saref4ener/hasCreationTime"/>
        </owl:onProperty>
        <owl:maxCardinality rdf:datatype="http://www.w3.org/2001/XMLSchema#nonNegativeInteger"
        >1</owl:maxCardinality>
      </owl:Restriction>
    </rdfs:subClassOf>
    <rdfs:subClassOf>
      <owl:Restriction>
        <owl:onProperty>
          <owl:ObjectProperty rdf:about="https://saref.etsi.org/saref4ener/hasUsage"/>
        </owl:onProperty>
        <owl:allValuesFrom rdf:resource="https://saref.etsi.org/saref4ener/Usage"/>
      </owl:Restriction>
    </rdfs:subClassOf>
    <rdfs:subClassOf rdf:resource="https://saref.etsi.org/core/Measurement"/>
    <rdfs:label xml:lang="en">Data point</rdfs:label>
    <rdfs:comment xml:lang="en">A data point is a quantity that is extended with various pieces of process information, namely&#xD;
 &#xD;
- A creation time (instant). This is the point in time when the data point was created, which is not necessarily the time for which it is valid. In the case of soft-sensors or forecasters, a data point might have been created ahead of time, in the case of a direcet measurement a data point might created at its time of validity (or at the end of its validity time interval) and in the case of an archived value the data point might have been created after the fact.&#xD;
&#xD;
 - A validity time (temporal entity) which will be named "time stamp". The validity time is the instant or interval in time in which a specific quantity is in effect. For example a room temperature might be measured at 12:00, which means it is in effect at this very instant. A specific amount of energy might me expended within the time-slot between 12:30 and 12:45, which means that the energy measurement is in effect during this time interval.&#xD;
&#xD;
 - A location or topological association. For example, a measurement might be taken in a specific room, a power avarage might have been measured by a specific meter, a forecast might be valid for a specific region or grid segment. This association is therefore not always a location.</rdfs:comment>
  </owl:Class>
  <owl:Class rdf:about="https://saref.etsi.org/saref4ener/DefaultDurationDescription">
    <owl:deprecated rdf:datatype="http://www.w3.org/2001/XMLSchema#boolean"
    >true</owl:deprecated>
    <rdfs:subClassOf rdf:resource="http://www.w3.org/2006/time#DurationDescription"/>
    <rdfs:label xml:lang="en">Default duration description</rdfs:label>
    <rdfs:comment xml:lang="en">The duration description for the default duration temporal entity</rdfs:comment>
  </owl:Class>
  <owl:Class rdf:about="https://saref.etsi.org/saref4ener/EventStateConsume">
    <owl:oneOf rdf:parseType="Collection">
      <s4ener:EventStateProduce rdf:about="https://saref.etsi.org/saref4ener/EventAccepted">
        <rdfs:label xml:lang="en">Event accepted</rdfs:label>
        <rdfs:comment xml:lang="en">Load control state with value 'event accepted'</rdfs:comment>
        <rdf:type rdf:resource="https://saref.etsi.org/saref4ener/EventStateConsume"/>
        <rdf:type rdf:resource="http://www.w3.org/2002/07/owl#NamedIndividual"/>
      </s4ener:EventStateProduce>
      <s4ener:EventStateProduce rdf:about="https://saref.etsi.org/saref4ener/EventStarted">
        <rdfs:label xml:lang="en">Event started</rdfs:label>
        <rdfs:comment xml:lang="en">Load control state with value 'event started'</rdfs:comment>
        <rdf:type rdf:resource="https://saref.etsi.org/saref4ener/EventStateConsume"/>
        <rdf:type rdf:resource="http://www.w3.org/2002/07/owl#NamedIndividual"/>
      </s4ener:EventStateProduce>
      <s4ener:EventStateProduce rdf:about="https://saref.etsi.org/saref4ener/EventStopped">
        <rdfs:label xml:lang="en">Event stopped</rdfs:label>
        <rdfs:comment xml:lang="en">Load control state with value 'event stopped'</rdfs:comment>
        <rdf:type rdf:resource="https://saref.etsi.org/saref4ener/EventStateConsume"/>
        <rdf:type rdf:resource="http://www.w3.org/2002/07/owl#NamedIndividual"/>
      </s4ener:EventStateProduce>
      <s4ener:EventStateProduce rdf:about="https://saref.etsi.org/saref4ener/EventRejected">
        <rdfs:label xml:lang="en">Event rejected</rdfs:label>
        <rdfs:comment xml:lang="en">Load control state with value 'event rejected'</rdfs:comment>
        <rdf:type rdf:resource="https://saref.etsi.org/saref4ener/EventStateConsume"/>
        <rdf:type rdf:resource="http://www.w3.org/2002/07/owl#NamedIndividual"/>
      </s4ener:EventStateProduce>
      <s4ener:EventStateProduce rdf:about="https://saref.etsi.org/saref4ener/EventCancelled">
        <rdfs:label xml:lang="en">Event cancelled</rdfs:label>
        <rdfs:comment xml:lang="en">Load control state with value 'event cancelled'</rdfs:comment>
        <rdf:type rdf:resource="https://saref.etsi.org/saref4ener/EventStateConsume"/>
        <rdf:type rdf:resource="http://www.w3.org/2002/07/owl#NamedIndividual"/>
      </s4ener:EventStateProduce>
      <s4ener:EventStateProduce rdf:about="https://saref.etsi.org/saref4ener/EventError">
        <rdfs:label xml:lang="en">Event error</rdfs:label>
        <rdfs:comment xml:lang="en">Load control state with value 'event error'</rdfs:comment>
        <rdf:type rdf:resource="https://saref.etsi.org/saref4ener/EventStateConsume"/>
        <rdf:type rdf:resource="http://www.w3.org/2002/07/owl#NamedIndividual"/>
      </s4ener:EventStateProduce>
    </owl:oneOf>
    <rdfs:subClassOf>
      <owl:Class rdf:about="https://saref.etsi.org/saref4ener/LoadControlEventState"/>
    </rdfs:subClassOf>
    <rdfs:label xml:lang="en">Event state consume</rdfs:label>
    <rdfs:comment xml:lang="en">In the load control, it expresses a consume state of an event used to send overload warning severity level and related load control commands to a device (e.g. a household appliance or a smart meter).</rdfs:comment>
  </owl:Class>
  <owl:Class rdf:about="https://saref.etsi.org/saref4ener/OperationMode">
    <rdfs:subClassOf rdf:resource="https://saref.etsi.org/core/State"/>
    <rdfs:label xml:lang="en">Operation Mode</rdfs:label>
    <rdfs:comment>A resource manager can declare multiple operation modes for a device. An operation mode is a mode/state that a device can find itself in, that is associated with a specific power value.</rdfs:comment>
  </owl:Class>
  <owl:Class rdf:about="https://saref.etsi.org/saref4ener/PowerPlan">
    <rdfs:subClassOf>
      <owl:Restriction>
        <owl:onProperty rdf:resource="https://saref.etsi.org/core/consistsOf"/>
        <owl:onClass>
          <owl:Class rdf:about="https://saref.etsi.org/saref4ener/TimeSeries"/>
        </owl:onClass>
        <owl:minQualifiedCardinality rdf:datatype="http://www.w3.org/2001/XMLSchema#nonNegativeInteger"
        >3</owl:minQualifiedCardinality>
      </owl:Restriction>
    </rdfs:subClassOf>
    <rdfs:subClassOf>
      <owl:Restriction>
        <owl:onProperty rdf:resource="https://saref.etsi.org/core/consistsOf"/>
        <owl:onClass>
          <owl:Class rdf:about="https://saref.etsi.org/saref4ener/TimeSeries"/>
        </owl:onClass>
        <owl:maxQualifiedCardinality rdf:datatype="http://www.w3.org/2001/XMLSchema#nonNegativeInteger"
        >3</owl:maxQualifiedCardinality>
      </owl:Restriction>
    </rdfs:subClassOf>
    <rdfs:subClassOf>
      <owl:Class rdf:about="https://saref.etsi.org/saref4ener/TimeSeries"/>
    </rdfs:subClassOf>
    <rdfs:label xml:lang="en">Power plan</rdfs:label>
    <rdfs:comment>The Power Plan that an energy manager creates for a device. It contains three timeseries indicating the minimum, average, and maximum respectively.</rdfs:comment>
  </owl:Class>
  <owl:Class rdf:about="https://saref.etsi.org/saref4ener/FailsafePowerLimit">
    <rdfs:subClassOf rdf:resource="https://saref.etsi.org/saref4ener/PowerLimit"/>
    <rdfs:label xml:lang="en">Failsafe Power Limit</rdfs:label>
    <rdfs:comment xml:lang="en">In case the communication between a device and the energy manager is interrupted, fail-safe values apply  and the device enters fail-safe state until the communication is re-established.</rdfs:comment>
  </owl:Class>
  <owl:Class rdf:about="https://saref.etsi.org/saref4ener/NumberRange">
    <rdfs:subClassOf rdf:resource="http://www.w3.org/2002/07/owl#Thing"/>
    <rdfs:label xml:lang="en">Number range</rdfs:label>
    <rdfs:comment>This class describes a range via a datatype property indicating the start of the range and another datatype property indicating the end of the range.</rdfs:comment>
  </owl:Class>
  <owl:Class rdf:about="https://saref.etsi.org/saref4ener/DurationUncertaintyDescription">
    <owl:deprecated rdf:datatype="http://www.w3.org/2001/XMLSchema#boolean"
    >true</owl:deprecated>
    <rdfs:subClassOf rdf:resource="http://www.w3.org/2006/time#DurationDescription"/>
    <rdfs:label xml:lang="en">Duration uncertainty description</rdfs:label>
    <rdfs:comment xml:lang="en">The duration description for the duration uncertainty temporal entity</rdfs:comment>
  </owl:Class>
  <owl:Class rdf:about="https://saref.etsi.org/saref4ener/RoleType">
    <rdfs:label xml:lang="en">Role Type</rdfs:label>
    <rdfs:comment>An enumeration containing the various roles a device can take up: consumer, producer, or storage.</rdfs:comment>
  </owl:Class>
  <owl:Class rdf:about="https://saref.etsi.org/saref4ener/SlotTimeDurationDescription">
    <owl:deprecated rdf:datatype="http://www.w3.org/2001/XMLSchema#boolean"
    >true</owl:deprecated>
    <rdfs:subClassOf rdf:resource="http://www.w3.org/2006/time#DurationDescription"/>
    <rdfs:label xml:lang="en">Slot time duration description</rdfs:label>
    <rdfs:comment xml:lang="en">The duration description for the slot time duration temporal entities</rdfs:comment>
  </owl:Class>
  <owl:Class rdf:about="https://saref.etsi.org/saref4ener/FlexRequest">
    <rdfs:subClassOf>
      <owl:Restriction>
        <owl:onProperty>
          <owl:ObjectProperty rdf:about="https://saref.etsi.org/saref4ener/includes"/>
        </owl:onProperty>
        <owl:allValuesFrom>
          <owl:Class>
            <owl:unionOf rdf:parseType="Collection">
              <owl:Class rdf:about="https://saref.etsi.org/saref4ener/DataPoint"/>
              <owl:Class rdf:about="https://saref.etsi.org/saref4ener/TimeSeries"/>
              <owl:Class rdf:about="https://saref.etsi.org/saref4ener/FlexibilityProfile"/>
              <owl:Class rdf:about="https://saref.etsi.org/saref4ener/IncentiveTableBasedProfile"/>
            </owl:unionOf>
          </owl:Class>
        </owl:allValuesFrom>
      </owl:Restriction>
    </rdfs:subClassOf>
    <rdfs:subClassOf>
      <owl:Restriction>
        <owl:onProperty>
          <owl:ObjectProperty rdf:about="https://saref.etsi.org/saref4ener/producedBy"/>
        </owl:onProperty>
        <owl:allValuesFrom>
          <owl:Class>
            <owl:unionOf rdf:parseType="Collection">
              <owl:Class rdf:about="http://xmlns.com/foaf/0.1/Agent"/>
              <rdf:Description rdf:about="https://saref.etsi.org/core/Device"/>
            </owl:unionOf>
          </owl:Class>
        </owl:allValuesFrom>
      </owl:Restriction>
    </rdfs:subClassOf>
    <rdfs:subClassOf>
      <owl:Restriction>
        <owl:onProperty>
          <owl:ObjectProperty rdf:about="https://saref.etsi.org/saref4ener/hasRecipient"/>
        </owl:onProperty>
        <owl:allValuesFrom>
          <owl:Class>
            <owl:unionOf rdf:parseType="Collection">
              <owl:Class rdf:about="http://xmlns.com/foaf/0.1/Agent"/>
              <rdf:Description rdf:about="https://saref.etsi.org/core/Device"/>
            </owl:unionOf>
          </owl:Class>
        </owl:allValuesFrom>
      </owl:Restriction>
    </rdfs:subClassOf>
    <rdfs:subClassOf>
      <owl:Restriction>
        <owl:onProperty>
          <owl:ObjectProperty rdf:about="https://saref.etsi.org/saref4ener/hasEffectivePeriod"/>
        </owl:onProperty>
        <owl:allValuesFrom rdf:resource="http://www.w3.org/2006/time#Interval"/>
      </owl:Restriction>
    </rdfs:subClassOf>
    <rdfs:subClassOf>
      <owl:Restriction>
        <owl:onProperty>
          <owl:DatatypeProperty rdf:about="https://saref.etsi.org/saref4ener/hasCreationTime"/>
        </owl:onProperty>
        <owl:allValuesFrom rdf:resource="http://www.w3.org/2001/XMLSchema#dateTime"/>
      </owl:Restriction>
    </rdfs:subClassOf>
    <rdfs:subClassOf rdf:resource="http://www.w3.org/2002/07/owl#Thing"/>
    <rdfs:label xml:lang="en">Flex request</rdfs:label>
    <rdfs:comment xml:lang="en">The flexibility request</rdfs:comment>
  </owl:Class>
  <owl:Class rdf:about="https://saref.etsi.org/saref4ener/ScheduleInstruction">
    <rdfs:subClassOf rdf:resource="https://saref.etsi.org/saref4ener/PPBCInstruction"/>
    <rdfs:label xml:lang="en">Schedule Instruction</rdfs:label>
    <rdfs:comment>Schedule instruction for a power profile flexibility profile.</rdfs:comment>
  </owl:Class>
  <owl:Class rdf:about="https://saref.etsi.org/saref4ener/TimeSeries">
    <rdfs:subClassOf>
      <owl:Restriction>
        <owl:onProperty>
          <owl:ObjectProperty rdf:about="https://saref.etsi.org/saref4ener/hasDataPoint"/>
        </owl:onProperty>
        <owl:onClass rdf:resource="https://saref.etsi.org/saref4ener/DataPoint"/>
        <owl:minQualifiedCardinality rdf:datatype="http://www.w3.org/2001/XMLSchema#nonNegativeInteger"
        >0</owl:minQualifiedCardinality>
      </owl:Restriction>
    </rdfs:subClassOf>
    <rdfs:subClassOf>
      <owl:Restriction>
        <owl:onProperty>
          <owl:DatatypeProperty rdf:about="https://saref.etsi.org/saref4ener/hasUpdateRate"/>
        </owl:onProperty>
        <owl:maxCardinality rdf:datatype="http://www.w3.org/2001/XMLSchema#nonNegativeInteger"
        >1</owl:maxCardinality>
      </owl:Restriction>
    </rdfs:subClassOf>
    <rdfs:subClassOf>
      <owl:Restriction>
        <owl:onProperty>
          <owl:DatatypeProperty rdf:about="https://saref.etsi.org/saref4ener/hasTemporalResolution"/>
        </owl:onProperty>
        <owl:maxCardinality rdf:datatype="http://www.w3.org/2001/XMLSchema#nonNegativeInteger"
        >1</owl:maxCardinality>
      </owl:Restriction>
    </rdfs:subClassOf>
    <rdfs:subClassOf>
      <owl:Restriction>
        <owl:onProperty>
          <owl:DatatypeProperty rdf:about="https://saref.etsi.org/saref4ener/hasCreationTime"/>
        </owl:onProperty>
        <owl:maxCardinality rdf:datatype="http://www.w3.org/2001/XMLSchema#nonNegativeInteger"
        >1</owl:maxCardinality>
      </owl:Restriction>
    </rdfs:subClassOf>
    <rdfs:subClassOf>
      <owl:Restriction>
        <owl:onProperty>
          <owl:ObjectProperty rdf:about="https://saref.etsi.org/saref4ener/hasUsage"/>
        </owl:onProperty>
        <owl:allValuesFrom rdf:resource="https://saref.etsi.org/saref4ener/Usage"/>
      </owl:Restriction>
    </rdfs:subClassOf>
    <rdfs:subClassOf>
      <owl:Restriction>
        <owl:onProperty>
          <owl:ObjectProperty rdf:about="https://saref.etsi.org/saref4ener/hasEffectivePeriod"/>
        </owl:onProperty>
        <owl:allValuesFrom rdf:resource="http://www.w3.org/2006/time#Interval"/>
      </owl:Restriction>
    </rdfs:subClassOf>
    <rdfs:label xml:lang="en">Time Series</rdfs:label>
    <rdfs:comment xml:lang="en">An ordered sequence of data points of a quantity observed at spaced time intervals is referred to as a time series. Time series can be a result of prediction algorithm.</rdfs:comment>
  </owl:Class>
  <owl:Class rdf:about="https://saref.etsi.org/saref4ener/PowerExpected">
    <rdfs:subClassOf>
      <owl:Class rdf:about="https://saref.etsi.org/saref4ener/Power"/>
    </rdfs:subClassOf>
    <rdfs:label xml:lang="en">Power expected </rdfs:label>
    <rdfs:comment xml:lang="en">A possible type of power in a slot that represents the expected power consumption and its value</rdfs:comment>
  </owl:Class>
  <owl:Class rdf:about="https://saref.etsi.org/saref4ener/EnergyMax">
    <rdfs:subClassOf rdf:resource="https://saref.etsi.org/saref4ener/Energy"/>
    <rdfs:label xml:lang="en">Energy max</rdfs:label>
    <rdfs:comment xml:lang="en">A possible type of energy in a slot that represents the maximum energy consumption and its value</rdfs:comment>
  </owl:Class>
  <owl:Class rdf:about="https://saref.etsi.org/saref4ener/FillRateProfile">
    <rdfs:subClassOf>
      <owl:Class rdf:about="https://saref.etsi.org/saref4ener/FlexibilityProfile"/>
    </rdfs:subClassOf>
    <rdfs:label xml:lang="en">Fill rate control</rdfs:label>
    <rdfs:comment>A flexibility profile specified through a Fill Rate Based Profile.</rdfs:comment>
  </owl:Class>
  <owl:Class rdf:about="https://saref.etsi.org/saref4ener/PowerSequenceElement">
    <rdfs:subClassOf rdf:resource="http://www.w3.org/2002/07/owl#Thing"/>
    <rdfs:label xml:lang="en">Power sequence element</rdfs:label>
    <rdfs:comment>An element of a power sequence, roughly equivalent to slots in the existing S4ener.</rdfs:comment>
  </owl:Class>
  <owl:Class rdf:about="https://saref.etsi.org/saref4ener/FlexibilityProfile">
    <rdfs:subClassOf rdf:resource="https://saref.etsi.org/core/Profile"/>
    <rdfs:label xml:lang="en">Flexibility Profile</rdfs:label>
    <rdfs:comment>Different control types to describe the energy flexibility that a device has to offer.  Charging of an EV for instance, may be controlled by power profile-based control or fill-rate -based control. It is not allowed to mix different control types at the same time, but different control types may be used sequentially.&#xD;
Control Types dictates flexibility instructions. Control Type provides Flexibility options.</rdfs:comment>
  </owl:Class>
  <owl:Class rdf:about="https://saref.etsi.org/saref4ener/EnergyStandardDeviation">
    <rdfs:subClassOf rdf:resource="https://saref.etsi.org/saref4ener/Energy"/>
    <rdfs:label xml:lang="en">Energy Standard Deviation</rdfs:label>
    <rdfs:comment xml:lang="en">A possible type of energy in a slot  that represents the energy standard deviation and its value</rdfs:comment>
  </owl:Class>
  <owl:Class rdf:about="https://saref.etsi.org/saref4ener/PEBCInstruction">
    <rdfs:subClassOf>
      <owl:Class rdf:about="https://saref.etsi.org/saref4ener/FlexibilityInstruction"/>
    </rdfs:subClassOf>
    <rdfs:label xml:lang="en">Power Envelop Based Control Instruction</rdfs:label>
    <rdfs:comment>An instruction for the Power Envelope Based Profile.</rdfs:comment>
  </owl:Class>
  <owl:Class rdf:about="https://saref.etsi.org/saref4ener/LoadControlEventState">
    <rdfs:subClassOf rdf:resource="https://saref.etsi.org/saref4ener/State"/>
    <rdfs:label xml:lang="en">Load control event state </rdfs:label>
    <rdfs:comment xml:lang="en">In the load control, it expresses the possible states of an event used to send overload warning severity level and related load control commands to a device (e.g. a household appliance or a smart meter).</rdfs:comment>
  </owl:Class>
  <owl:Class rdf:about="https://saref.etsi.org/saref4ener/ActuatorSwitch">
    <rdfs:subClassOf rdf:resource="https://saref.etsi.org/core/Actuator"/>
    <rdfs:label xml:lang="en">Actuator switch</rdfs:label>
    <rdfs:comment xml:lang="en">Basic on/off operations on a simple actuator can be modelled with the ActuatorSwitch class. Whether the function turns a device itself ON or OFF, or whether it switches a specific feature, depends on the implementation. For example, one could model the super freeze program of a freezer using ActuatorSwitch class. An ON command would then activate the super freeze program and an OFF command would deactivate it. This example shall just give an idea how ActuatorSwitch can be used for more purposes than only turning devices on and off.</rdfs:comment>
  </owl:Class>
  <owl:Class rdf:about="https://saref.etsi.org/saref4ener/LeakageBehaviour">
    <rdfs:subClassOf rdf:resource="http://www.w3.org/2002/07/owl#Thing"/>
    <rdfs:label xml:lang="en">Leakage behaviour</rdfs:label>
    <rdfs:comment>A description of the Leakage Behaviour associated with this Fill Rate Flexibility Profile.</rdfs:comment>
  </owl:Class>
  <owl:Class rdf:about="https://saref.etsi.org/saref4ener/Power">
    <rdfs:subClassOf rdf:resource="https://saref.etsi.org/core/Power"/>
    <rdfs:label xml:lang="en">Power</rdfs:label>
    <rdfs:comment xml:lang="en">Power type and value in a slot (i.e. power, powerMin, powerMax, powerExpectedValue, powerStandardDeviation, powerSkewness)</rdfs:comment>
  </owl:Class>
  <owl:Class rdf:about="https://saref.etsi.org/saref4ener/MaxAnticipation">
    <owl:deprecated rdf:datatype="http://www.w3.org/2001/XMLSchema#boolean"
    >true</owl:deprecated>
    <rdfs:subClassOf rdf:resource="http://www.w3.org/2006/time#TemporalEntity"/>
    <rdfs:label xml:lang="en">Max anticipation</rdfs:label>
    <rdfs:comment xml:lang="en">This field allows the anticipation of the phase if (and only if) the previous phase has the energy set to 0 Wh, each unit is a minute.</rdfs:comment>
  </owl:Class>
  <owl:Class rdf:about="https://saref.etsi.org/saref4ener/ContractualPowerLimit">
    <rdfs:subClassOf rdf:resource="https://saref.etsi.org/saref4ener/PowerLimit"/>
    <rdfs:label xml:lang="en">Contractual Power Limit</rdfs:label>
    <rdfs:comment xml:lang="en">The contractual power limit of a device</rdfs:comment>
  </owl:Class>
  <owl:Class rdf:about="https://saref.etsi.org/saref4ener/AlternativesGroup">
    <rdfs:subClassOf>
      <owl:Restriction>
        <owl:qualifiedCardinality rdf:datatype="http://www.w3.org/2001/XMLSchema#nonNegativeInteger"
        >1</owl:qualifiedCardinality>
        <owl:onProperty>
          <owl:DatatypeProperty rdf:about="https://saref.etsi.org/saref4ener/alternativesGroupID"/>
        </owl:onProperty>
        <owl:onDataRange rdf:resource="http://www.w3.org/2001/XMLSchema#unsignedInt"/>
      </owl:Restriction>
    </rdfs:subClassOf>
    <rdfs:subClassOf>
      <owl:Restriction>
        <owl:qualifiedCardinality rdf:datatype="http://www.w3.org/2001/XMLSchema#nonNegativeInteger"
        >1</owl:qualifiedCardinality>
        <owl:onProperty>
          <owl:ObjectProperty rdf:about="https://saref.etsi.org/saref4ener/belongsTo"/>
        </owl:onProperty>
        <owl:onClass>
          <owl:Class rdf:about="https://saref.etsi.org/saref4ener/PowerProfile"/>
        </owl:onClass>
      </owl:Restriction>
    </rdfs:subClassOf>
    <rdfs:subClassOf>
      <owl:Restriction>
        <owl:onProperty rdf:resource="https://saref.etsi.org/core/consistsOf"/>
        <owl:onClass rdf:resource="https://saref.etsi.org/saref4ener/PowerSequence"/>
        <owl:minQualifiedCardinality rdf:datatype="http://www.w3.org/2001/XMLSchema#nonNegativeInteger"
        >1</owl:minQualifiedCardinality>
      </owl:Restriction>
    </rdfs:subClassOf>
    <rdfs:subClassOf>
      <owl:Restriction>
        <owl:onProperty rdf:resource="https://saref.etsi.org/core/consistsOf"/>
        <owl:allValuesFrom rdf:resource="https://saref.etsi.org/saref4ener/PowerSequence"/>
      </owl:Restriction>
    </rdfs:subClassOf>
    <rdfs:subClassOf>
      <owl:Restriction>
        <owl:onProperty>
          <owl:ObjectProperty rdf:about="https://saref.etsi.org/saref4ener/belongsTo"/>
        </owl:onProperty>
        <owl:allValuesFrom>
          <owl:Class rdf:about="https://saref.etsi.org/saref4ener/PowerProfile"/>
        </owl:allValuesFrom>
      </owl:Restriction>
    </rdfs:subClassOf>
    <rdfs:label xml:lang="en">Alternatives group</rdfs:label>
    <rdfs:comment xml:lang="en">A collection of power sequences for a certain profile</rdfs:comment>
  </owl:Class>
  <owl:Class rdf:about="https://saref.etsi.org/saref4ener/ActiveDurationSumMin">
    <owl:deprecated rdf:datatype="http://www.w3.org/2001/XMLSchema#boolean"
    >true</owl:deprecated>
    <rdfs:subClassOf rdf:resource="http://www.w3.org/2006/time#TemporalEntity"/>
    <rdfs:label xml:lang="en">Active duration sum min</rdfs:label>
    <rdfs:comment xml:lang="en">The active minimum duration a power sequence must run in total (summation of all active times).</rdfs:comment>
  </owl:Class>
  <owl:Class rdf:about="https://saref.etsi.org/saref4ener/Slot">
    <rdfs:subClassOf>
      <owl:Restriction>
        <owl:onProperty>
          <owl:DatatypeProperty rdf:about="https://saref.etsi.org/saref4ener/slotActivated"/>
        </owl:onProperty>
        <owl:maxCardinality rdf:datatype="http://www.w3.org/2001/XMLSchema#nonNegativeInteger"
        >1</owl:maxCardinality>
      </owl:Restriction>
    </rdfs:subClassOf>
    <rdfs:subClassOf>
      <owl:Restriction>
        <owl:onProperty>
          <owl:ObjectProperty rdf:about="https://saref.etsi.org/saref4ener/hasPowerValueType"/>
        </owl:onProperty>
        <owl:allValuesFrom rdf:resource="https://saref.etsi.org/saref4ener/Power"/>
      </owl:Restriction>
    </rdfs:subClassOf>
    <rdfs:subClassOf>
      <owl:Restriction>
        <owl:onProperty rdf:resource="https://saref.etsi.org/core/hasTime"/>
        <owl:onClass rdf:resource="https://saref.etsi.org/saref4ener/LatestEndTime"/>
        <owl:maxQualifiedCardinality rdf:datatype="http://www.w3.org/2001/XMLSchema#nonNegativeInteger"
        >1</owl:maxQualifiedCardinality>
      </owl:Restriction>
    </rdfs:subClassOf>
    <rdfs:subClassOf>
      <owl:Restriction>
        <owl:onProperty rdf:resource="https://saref.etsi.org/core/hasTime"/>
        <owl:allValuesFrom rdf:resource="https://saref.etsi.org/core/Time"/>
      </owl:Restriction>
    </rdfs:subClassOf>
    <rdfs:subClassOf>
      <owl:Restriction>
        <owl:onProperty>
          <owl:ObjectProperty rdf:about="https://saref.etsi.org/saref4ener/hasEnergyValueType"/>
        </owl:onProperty>
        <owl:allValuesFrom rdf:resource="https://saref.etsi.org/saref4ener/Energy"/>
      </owl:Restriction>
    </rdfs:subClassOf>
    <rdfs:subClassOf>
      <owl:Restriction>
        <owl:onProperty rdf:resource="https://saref.etsi.org/core/hasTime"/>
        <owl:onClass rdf:resource="https://saref.etsi.org/saref4ener/StartTime"/>
        <owl:maxQualifiedCardinality rdf:datatype="http://www.w3.org/2001/XMLSchema#nonNegativeInteger"
        >1</owl:maxQualifiedCardinality>
      </owl:Restriction>
    </rdfs:subClassOf>
    <rdfs:subClassOf>
      <owl:Restriction>
        <owl:onProperty>
          <owl:DatatypeProperty rdf:about="https://saref.etsi.org/saref4ener/optionalSlot"/>
        </owl:onProperty>
        <owl:maxCardinality rdf:datatype="http://www.w3.org/2001/XMLSchema#nonNegativeInteger"
        >1</owl:maxCardinality>
      </owl:Restriction>
    </rdfs:subClassOf>
    <rdfs:subClassOf>
      <owl:Restriction>
        <owl:onProperty>
          <owl:ObjectProperty rdf:about="https://saref.etsi.org/saref4ener/belongsTo"/>
        </owl:onProperty>
        <owl:allValuesFrom rdf:resource="https://saref.etsi.org/saref4ener/PowerSequence"/>
      </owl:Restriction>
    </rdfs:subClassOf>
    <rdfs:subClassOf>
      <owl:Restriction>
        <owl:qualifiedCardinality rdf:datatype="http://www.w3.org/2001/XMLSchema#nonNegativeInteger"
        >1</owl:qualifiedCardinality>
        <owl:onProperty>
          <owl:ObjectProperty rdf:about="https://saref.etsi.org/saref4ener/belongsTo"/>
        </owl:onProperty>
        <owl:onClass rdf:resource="https://saref.etsi.org/saref4ener/PowerSequence"/>
      </owl:Restriction>
    </rdfs:subClassOf>
    <rdfs:subClassOf>
      <owl:Restriction>
        <owl:onProperty rdf:resource="https://saref.etsi.org/core/hasTime"/>
        <owl:onClass rdf:resource="https://saref.etsi.org/saref4ener/DefaultDuration"/>
        <owl:maxQualifiedCardinality rdf:datatype="http://www.w3.org/2001/XMLSchema#nonNegativeInteger"
        >1</owl:maxQualifiedCardinality>
      </owl:Restriction>
    </rdfs:subClassOf>
    <rdfs:label xml:lang="en">Slot</rdfs:label>
    <rdfs:subClassOf>
      <owl:Restriction>
        <owl:onProperty rdf:resource="https://saref.etsi.org/core/hasDescription"/>
        <owl:maxCardinality rdf:datatype="http://www.w3.org/2001/XMLSchema#nonNegativeInteger"
        >1</owl:maxCardinality>
      </owl:Restriction>
    </rdfs:subClassOf>
    <rdfs:subClassOf>
      <owl:Restriction>
        <owl:onProperty rdf:resource="https://saref.etsi.org/core/hasTime"/>
        <owl:onClass rdf:resource="https://saref.etsi.org/saref4ener/MaxDuration"/>
        <owl:maxQualifiedCardinality rdf:datatype="http://www.w3.org/2001/XMLSchema#nonNegativeInteger"
        >1</owl:maxQualifiedCardinality>
      </owl:Restriction>
    </rdfs:subClassOf>
    <rdfs:subClassOf>
      <owl:Restriction>
        <owl:onProperty rdf:resource="https://saref.etsi.org/core/hasTime"/>
        <owl:onClass rdf:resource="https://saref.etsi.org/saref4ener/DurationUncertainty"/>
        <owl:maxQualifiedCardinality rdf:datatype="http://www.w3.org/2001/XMLSchema#nonNegativeInteger"
        >1</owl:maxQualifiedCardinality>
      </owl:Restriction>
    </rdfs:subClassOf>
    <rdfs:subClassOf>
      <owl:Restriction>
        <owl:onProperty rdf:resource="https://saref.etsi.org/core/hasTime"/>
        <owl:onClass>
          <owl:Class rdf:about="https://saref.etsi.org/saref4ener/EarliestStartTime"/>
        </owl:onClass>
        <owl:maxQualifiedCardinality rdf:datatype="http://www.w3.org/2001/XMLSchema#nonNegativeInteger"
        >1</owl:maxQualifiedCardinality>
      </owl:Restriction>
    </rdfs:subClassOf>
    <rdfs:comment xml:lang="en">The single steps of a power sequence are represented by slots. A slot is associated with a slot number (while a power sequence is associated with a power sequence identifier). The slot numbers of two power sequences should be considered independent from each other, i.e., slot number 7 of sequence 1 describes a different slot than slot number 7 of sequence 2. Therefore a slot is only uniquely identified in combination with a sequence ID. </rdfs:comment>
    <rdfs:subClassOf>
      <owl:Restriction>
        <owl:onProperty>
          <owl:DatatypeProperty rdf:about="https://saref.etsi.org/saref4ener/slotNumber"/>
        </owl:onProperty>
        <owl:cardinality rdf:datatype="http://www.w3.org/2001/XMLSchema#nonNegativeInteger"
        >1</owl:cardinality>
      </owl:Restriction>
    </rdfs:subClassOf>
    <rdfs:subClassOf>
      <owl:Restriction>
        <owl:onProperty rdf:resource="https://saref.etsi.org/core/hasTime"/>
        <owl:onClass rdf:resource="https://saref.etsi.org/saref4ener/EndTime"/>
        <owl:maxQualifiedCardinality rdf:datatype="http://www.w3.org/2001/XMLSchema#nonNegativeInteger"
        >1</owl:maxQualifiedCardinality>
      </owl:Restriction>
    </rdfs:subClassOf>
    <rdfs:subClassOf>
      <owl:Restriction>
        <owl:onProperty rdf:resource="https://saref.etsi.org/core/hasTime"/>
        <owl:onClass rdf:resource="https://saref.etsi.org/saref4ener/RemainingPauseTime"/>
        <owl:maxQualifiedCardinality rdf:datatype="http://www.w3.org/2001/XMLSchema#nonNegativeInteger"
        >1</owl:maxQualifiedCardinality>
      </owl:Restriction>
    </rdfs:subClassOf>
    <rdfs:subClassOf>
      <owl:Restriction>
        <owl:onProperty rdf:resource="https://saref.etsi.org/core/hasTime"/>
        <owl:onClass rdf:resource="https://saref.etsi.org/saref4ener/MinDuration"/>
        <owl:maxQualifiedCardinality rdf:datatype="http://www.w3.org/2001/XMLSchema#nonNegativeInteger"
        >1</owl:maxQualifiedCardinality>
      </owl:Restriction>
    </rdfs:subClassOf>
    <rdfs:subClassOf>
      <owl:Restriction>
        <owl:onProperty>
          <owl:ObjectProperty rdf:about="https://saref.etsi.org/saref4ener/hasValueType"/>
        </owl:onProperty>
        <owl:onClass>
          <owl:Class>
            <owl:unionOf rdf:parseType="Collection">
              <owl:Class rdf:about="https://saref.etsi.org/saref4ener/Energy"/>
              <owl:Class rdf:about="https://saref.etsi.org/saref4ener/Power"/>
            </owl:unionOf>
          </owl:Class>
        </owl:onClass>
        <owl:minQualifiedCardinality rdf:datatype="http://www.w3.org/2001/XMLSchema#nonNegativeInteger"
        >1</owl:minQualifiedCardinality>
      </owl:Restriction>
    </rdfs:subClassOf>
  </owl:Class>
  <owl:Class rdf:about="https://saref.etsi.org/saref4ener/EventStateProduce">
    <owl:oneOf rdf:parseType="Collection">
      <s4ener:EventStateProduce rdf:about="https://saref.etsi.org/saref4ener/EventAccepted"/>
      <s4ener:EventStateProduce rdf:about="https://saref.etsi.org/saref4ener/EventStarted"/>
      <s4ener:EventStateProduce rdf:about="https://saref.etsi.org/saref4ener/EventStopped"/>
      <s4ener:EventStateProduce rdf:about="https://saref.etsi.org/saref4ener/EventRejected"/>
      <s4ener:EventStateProduce rdf:about="https://saref.etsi.org/saref4ener/EventCancelled"/>
      <s4ener:EventStateProduce rdf:about="https://saref.etsi.org/saref4ener/EventError"/>
    </owl:oneOf>
    <rdfs:subClassOf rdf:resource="https://saref.etsi.org/saref4ener/LoadControlEventState"/>
    <rdfs:label xml:lang="en">Event state produce</rdfs:label>
    <rdfs:comment xml:lang="en">In the load control, it expresses a produce state of an event an event used to send overload warning severity level and related load control commands to a device (e.g. a household appliance or a smart meter).</rdfs:comment>
  </owl:Class>
  <owl:Class rdf:about="https://saref.etsi.org/saref4ener/PowerProfile">
    <rdfs:subClassOf>
      <owl:Restriction>
        <owl:onProperty rdf:resource="https://saref.etsi.org/core/consistsOf"/>
        <owl:onClass rdf:resource="https://saref.etsi.org/saref4ener/AlternativesGroup"/>
        <owl:minQualifiedCardinality rdf:datatype="http://www.w3.org/2001/XMLSchema#nonNegativeInteger"
        >0</owl:minQualifiedCardinality>
      </owl:Restriction>
    </rdfs:subClassOf>
    <rdfs:subClassOf rdf:resource="https://saref.etsi.org/core/Profile"/>
    <rdfs:subClassOf>
      <owl:Restriction>
        <owl:onProperty>
          <owl:DatatypeProperty rdf:about="https://saref.etsi.org/saref4ener/supportsSingleSlotSchedulingOnly"/>
        </owl:onProperty>
        <owl:cardinality rdf:datatype="http://www.w3.org/2001/XMLSchema#nonNegativeInteger"
        >1</owl:cardinality>
      </owl:Restriction>
    </rdfs:subClassOf>
    <rdfs:label xml:lang="en">Power profile control</rdfs:label>
    <rdfs:comment xml:lang="en">A way to model curves of power and energy over time, which also provides definitions for the modelling of power scheduling including alternative plans. With a PowerProfile, a device (or power sequences server) exposes the power sequences that are potentially relevant for the CEM (or power sequences client). </rdfs:comment>
    <rdfs:subClassOf>
      <owl:Restriction>
        <owl:onProperty>
          <owl:DatatypeProperty rdf:about="https://saref.etsi.org/saref4ener/nodeRemoteControllable"/>
        </owl:onProperty>
        <owl:cardinality rdf:datatype="http://www.w3.org/2001/XMLSchema#nonNegativeInteger"
        >1</owl:cardinality>
      </owl:Restriction>
    </rdfs:subClassOf>
    <rdfs:subClassOf>
      <owl:Restriction>
        <owl:onProperty>
          <owl:DatatypeProperty rdf:about="https://saref.etsi.org/saref4ener/totalSequencesCountMax"/>
        </owl:onProperty>
        <owl:cardinality rdf:datatype="http://www.w3.org/2001/XMLSchema#nonNegativeInteger"
        >1</owl:cardinality>
      </owl:Restriction>
    </rdfs:subClassOf>
    <rdfs:comment>PPBC.PowerProfileDefinition</rdfs:comment>
    <rdfs:subClassOf>
      <owl:Restriction>
        <owl:onProperty>
          <owl:ObjectProperty rdf:about="https://saref.etsi.org/saref4ener/belongsTo"/>
        </owl:onProperty>
        <owl:allValuesFrom>
          <owl:Class rdf:about="https://saref.etsi.org/saref4ener/Device"/>
        </owl:allValuesFrom>
      </owl:Restriction>
    </rdfs:subClassOf>
    <rdfs:subClassOf>
      <owl:Restriction>
        <owl:onProperty>
          <owl:DatatypeProperty rdf:about="https://saref.etsi.org/saref4ener/supportsReselection"/>
        </owl:onProperty>
        <owl:cardinality rdf:datatype="http://www.w3.org/2001/XMLSchema#nonNegativeInteger"
        >1</owl:cardinality>
      </owl:Restriction>
    </rdfs:subClassOf>
    <rdfs:subClassOf>
      <owl:Restriction>
        <owl:qualifiedCardinality rdf:datatype="http://www.w3.org/2001/XMLSchema#nonNegativeInteger"
        >1</owl:qualifiedCardinality>
        <owl:onProperty>
          <owl:ObjectProperty rdf:about="https://saref.etsi.org/saref4ener/belongsTo"/>
        </owl:onProperty>
        <owl:onClass>
          <owl:Class rdf:about="https://saref.etsi.org/saref4ener/Device"/>
        </owl:onClass>
      </owl:Restriction>
    </rdfs:subClassOf>
    <rdfs:subClassOf>
      <owl:Restriction>
        <owl:onProperty rdf:resource="https://saref.etsi.org/core/consistsOf"/>
        <owl:allValuesFrom rdf:resource="https://saref.etsi.org/saref4ener/AlternativesGroup"/>
      </owl:Restriction>
    </rdfs:subClassOf>
    <rdfs:subClassOf>
      <owl:Restriction>
        <owl:onProperty>
          <owl:DatatypeProperty rdf:about="https://saref.etsi.org/saref4ener/alternativesCount"/>
        </owl:onProperty>
        <owl:cardinality rdf:datatype="http://www.w3.org/2001/XMLSchema#nonNegativeInteger"
        >1</owl:cardinality>
      </owl:Restriction>
    </rdfs:subClassOf>
  </owl:Class>
  <owl:Class rdf:about="https://saref.etsi.org/saref4ener/PowerSource">
    <rdfs:subClassOf rdf:resource="http://www.w3.org/2002/07/owl#Thing"/>
    <rdfs:label xml:lang="en">Power source</rdfs:label>
    <rdfs:comment xml:lang="en">Indicates the power source of a device. Possible values are e.g. mainsSinglePhase or battery</rdfs:comment>
  </owl:Class>
  <owl:Class rdf:about="https://saref.etsi.org/saref4ener/FillLevelTargetProfile">
    <rdfs:subClassOf rdf:resource="http://www.w3.org/2002/07/owl#Thing"/>
    <rdfs:label xml:lang="en">Fill level target profile</rdfs:label>
    <rdfs:comment>The target profile that a fill rate based control flexibility profile tries to follow.</rdfs:comment>
  </owl:Class>
  <owl:Class rdf:about="https://saref.etsi.org/saref4ener/OMBCInstruction">
    <rdfs:subClassOf>
      <owl:Class rdf:about="https://saref.etsi.org/saref4ener/FlexibilityInstruction"/>
    </rdfs:subClassOf>
    <rdfs:label xml:lang="en">Operation Mode Based Control Instruction</rdfs:label>
    <rdfs:comment>An instruction following the Operation Mode Based Profile.</rdfs:comment>
  </owl:Class>
  <owl:Class rdf:about="https://saref.etsi.org/saref4ener/PowerSequenceContainer">
    <rdfs:subClassOf rdf:resource="http://www.w3.org/2002/07/owl#Thing"/>
    <rdfs:label xml:lang="en">Power profile container</rdfs:label>
    <rdfs:comment>A container containing the various Power Sequences among which the EMS may choose for the appropriate Power Sequence at a given time.</rdfs:comment>
  </owl:Class>
  <owl:Class rdf:about="https://saref.etsi.org/saref4ener/PauseDurationMax">
    <owl:deprecated rdf:datatype="http://www.w3.org/2001/XMLSchema#boolean"
    >true</owl:deprecated>
    <rdfs:subClassOf rdf:resource="http://www.w3.org/2006/time#TemporalEntity"/>
    <rdfs:label xml:lang="en">Pause duration max</rdfs:label>
    <rdfs:comment xml:lang="en">The maximum duration a power sequence can pause after the end of an activity.</rdfs:comment>
  </owl:Class>
  <owl:Class rdf:about="https://saref.etsi.org/saref4ener/RemainingSlotTime">
    <owl:deprecated rdf:datatype="http://www.w3.org/2001/XMLSchema#boolean"
    >true</owl:deprecated>
    <rdfs:subClassOf rdf:resource="http://www.w3.org/2006/time#TemporalEntity"/>
    <rdfs:label xml:lang="en">Remaining slot time</rdfs:label>
    <rdfs:comment xml:lang="en">If state is set to 'running' or 'paused' AND the slot is determined, this element SHALL contain the time the slot still needs to be in 'running' state (this also means the value remains constant during a 'paused' state). Otherwise it SHALL be omitted.</rdfs:comment>
  </owl:Class>
  <owl:Class rdf:about="https://saref.etsi.org/saref4ener/NominalPowerLimit">
    <rdfs:subClassOf rdf:resource="https://saref.etsi.org/saref4ener/PowerLimit"/>
    <rdfs:label xml:lang="en">Nominal Power Limit</rdfs:label>
    <rdfs:comment xml:lang="en">A device may have nominal power consumption and/or production values that are defined by the manufacturer and must not be exceeded, so that the power limit must stay within these constraints.</rdfs:comment>
  </owl:Class>
  <owl:Class rdf:about="https://saref.etsi.org/saref4ener/FlexibilityInstruction">
    <rdfs:label xml:lang="en">Flexibility Instruction</rdfs:label>
    <rdfs:comment>The various types of instructions Flexibility Sources can send and/or receive.</rdfs:comment>
  </owl:Class>
  <owl:Class rdf:about="https://saref.etsi.org/saref4ener/Device">
    <rdfs:subClassOf>
      <owl:Restriction>
        <owl:onProperty>
          <owl:DatatypeProperty rdf:about="https://saref.etsi.org/saref4ener/vendorName"/>
        </owl:onProperty>
        <owl:maxCardinality rdf:datatype="http://www.w3.org/2001/XMLSchema#nonNegativeInteger"
        >1</owl:maxCardinality>
      </owl:Restriction>
    </rdfs:subClassOf>
    <rdfs:subClassOf>
      <owl:Restriction>
        <owl:onProperty>
          <owl:ObjectProperty rdf:about="https://saref.etsi.org/saref4ener/receives"/>
        </owl:onProperty>
        <owl:allValuesFrom>
          <owl:Class rdf:about="https://saref.etsi.org/saref4ener/LoadControlEventData"/>
        </owl:allValuesFrom>
      </owl:Restriction>
    </rdfs:subClassOf>
    <rdfs:subClassOf>
      <owl:Restriction>
        <owl:onProperty>
          <owl:DatatypeProperty rdf:about="https://saref.etsi.org/saref4ener/manufacturerNodeIdentification"/>
        </owl:onProperty>
        <owl:maxCardinality rdf:datatype="http://www.w3.org/2001/XMLSchema#nonNegativeInteger"
        >1</owl:maxCardinality>
      </owl:Restriction>
    </rdfs:subClassOf>
    <rdfs:subClassOf>
      <owl:Restriction>
        <owl:onProperty>
          <owl:DatatypeProperty rdf:about="https://saref.etsi.org/saref4ener/deviceCode"/>
        </owl:onProperty>
        <owl:maxCardinality rdf:datatype="http://www.w3.org/2001/XMLSchema#nonNegativeInteger"
        >1</owl:maxCardinality>
      </owl:Restriction>
    </rdfs:subClassOf>
    <rdfs:subClassOf>
      <owl:Restriction>
        <owl:onProperty>
          <owl:ObjectProperty rdf:about="https://saref.etsi.org/saref4ener/receives"/>
        </owl:onProperty>
        <owl:onClass>
          <owl:Class rdf:about="https://saref.etsi.org/saref4ener/LoadControlEventData"/>
        </owl:onClass>
        <owl:minQualifiedCardinality rdf:datatype="http://www.w3.org/2001/XMLSchema#nonNegativeInteger"
        >0</owl:minQualifiedCardinality>
      </owl:Restriction>
    </rdfs:subClassOf>
    <rdfs:subClassOf>
      <owl:Restriction>
        <owl:onProperty>
          <owl:DatatypeProperty rdf:about="https://saref.etsi.org/saref4ener/brandName"/>
        </owl:onProperty>
        <owl:maxCardinality rdf:datatype="http://www.w3.org/2001/XMLSchema#nonNegativeInteger"
        >1</owl:maxCardinality>
      </owl:Restriction>
    </rdfs:subClassOf>
    <rdfs:subClassOf>
      <owl:Restriction>
        <owl:onProperty>
          <owl:DatatypeProperty rdf:about="https://saref.etsi.org/saref4ener/serialNumber"/>
        </owl:onProperty>
        <owl:maxCardinality rdf:datatype="http://www.w3.org/2001/XMLSchema#nonNegativeInteger"
        >1</owl:maxCardinality>
      </owl:Restriction>
    </rdfs:subClassOf>
    <rdfs:subClassOf>
      <owl:Restriction>
        <owl:onProperty>
          <owl:DatatypeProperty rdf:about="https://saref.etsi.org/saref4ener/deviceName"/>
        </owl:onProperty>
        <owl:maxCardinality rdf:datatype="http://www.w3.org/2001/XMLSchema#nonNegativeInteger"
        >1</owl:maxCardinality>
      </owl:Restriction>
    </rdfs:subClassOf>
    <rdfs:label xml:lang="en">Device</rdfs:label>
    <rdfs:subClassOf>
      <owl:Restriction>
        <owl:onProperty>
          <owl:DatatypeProperty rdf:about="https://saref.etsi.org/saref4ener/softwareRevision"/>
        </owl:onProperty>
        <owl:maxCardinality rdf:datatype="http://www.w3.org/2001/XMLSchema#nonNegativeInteger"
        >1</owl:maxCardinality>
      </owl:Restriction>
    </rdfs:subClassOf>
    <rdfs:subClassOf>
      <owl:Restriction>
        <owl:onProperty>
          <owl:ObjectProperty rdf:about="https://saref.etsi.org/saref4ener/hasPowerSource"/>
        </owl:onProperty>
        <owl:minCardinality rdf:datatype="http://www.w3.org/2001/XMLSchema#nonNegativeInteger"
        >0</owl:minCardinality>
      </owl:Restriction>
    </rdfs:subClassOf>
    <rdfs:subClassOf>
      <owl:Restriction>
        <owl:onProperty>
          <owl:DatatypeProperty rdf:about="https://saref.etsi.org/saref4ener/manufacturerDescription"/>
        </owl:onProperty>
        <owl:maxCardinality rdf:datatype="http://www.w3.org/2001/XMLSchema#nonNegativeInteger"
        >1</owl:maxCardinality>
      </owl:Restriction>
    </rdfs:subClassOf>
    <rdfs:subClassOf>
      <owl:Restriction>
        <owl:onProperty>
          <owl:DatatypeProperty rdf:about="https://saref.etsi.org/saref4ener/manufacturerLabel"/>
        </owl:onProperty>
        <owl:maxCardinality rdf:datatype="http://www.w3.org/2001/XMLSchema#nonNegativeInteger"
        >1</owl:maxCardinality>
      </owl:Restriction>
    </rdfs:subClassOf>
    <rdfs:subClassOf>
      <owl:Restriction>
        <owl:onProperty>
          <owl:DatatypeProperty rdf:about="https://saref.etsi.org/saref4ener/vendorCode"/>
        </owl:onProperty>
        <owl:maxCardinality rdf:datatype="http://www.w3.org/2001/XMLSchema#nonNegativeInteger"
        >1</owl:maxCardinality>
      </owl:Restriction>
    </rdfs:subClassOf>
    <rdfs:subClassOf>
      <owl:Restriction>
        <owl:onProperty>
          <owl:DatatypeProperty rdf:about="https://saref.etsi.org/saref4ener/hardwareRevision"/>
        </owl:onProperty>
        <owl:maxCardinality rdf:datatype="http://www.w3.org/2001/XMLSchema#nonNegativeInteger"
        >1</owl:maxCardinality>
      </owl:Restriction>
    </rdfs:subClassOf>
    <rdfs:comment xml:lang="en">A specialization of a saref:Device that exposes a power profile with power sequences to the CEM (note that a s4ee:Device can also be called 'power sequence server'). Most of the existing devices can expose at most 1 power profile, but there are special cases in which more than one power profiles can be exposed by the same device. For example, consider the case of a combined fridge-freezer in which there are 2 logical devices (fridge and freezer) combined in 1 physical device. This combined device can expose 2 power profiles, one for the fridge and one for the freezer. A s4ee:Device (e.g. a household appliance or a smart meter) can also receive events about overload warning severity level and related load control commands (LoadControlEventData)</rdfs:comment>
    <rdfs:subClassOf rdf:resource="https://saref.etsi.org/core/Device"/>
  </owl:Class>
  <owl:Class rdf:about="https://saref.etsi.org/saref4ener/IncentiveType">
    <rdfs:label xml:lang="en">Incentive Type</rdfs:label>
    <rdfs:comment xml:lang="en">In the incentive table, an incentive type is defined  in the form of costs (relative or absolute), CO2 emissions or renewable energy percentage.</rdfs:comment>
  </owl:Class>
  <owl:Class rdf:about="https://saref.etsi.org/saref4ener/Incentive">
    <rdfs:subClassOf rdf:resource="https://saref.etsi.org/saref4ener/DataPoint"/>
    <rdfs:label xml:lang="en">Incentive</rdfs:label>
    <rdfs:comment>An Incentive indicates the intersection of a tier with a slot. In this particular combination of slot and tier there are a particular costs to draw this type of energy. For example, drawing power from the grid costs 0.30 euro per kilowatthour during the afternoon, but will only be activated from a lower boundary of 3000W.</rdfs:comment>
  </owl:Class>
  <owl:Class rdf:about="https://saref.etsi.org/saref4ener/EarliestStartTime">
    <rdfs:subClassOf rdf:resource="http://www.w3.org/2006/time#TemporalEntity"/>
    <rdfs:label xml:lang="en">Earliest start time</rdfs:label>
    <rdfs:comment xml:lang="en">The earliest possible start time for a power sequence or a slot. Only 'xs:duration' value types SHALL be used to denote a relative time which relates to 'now' as time 0.&#xD;
Note: This element applies to the first repetition of the slot number only.</rdfs:comment>
  </owl:Class>
  <owl:Class rdf:about="https://saref.etsi.org/saref4ener/PowerSequenceState">
    <rdfs:subClassOf rdf:resource="https://saref.etsi.org/saref4ener/State"/>
    <rdfs:label xml:lang="en">Power sequence state</rdfs:label>
    <rdfs:comment xml:lang="en">The current state of the power sequence. It can assume one of the values 'running', 'paused', 'scheduled', 'scheduled paused', 'pending', 'inactive', 'completed',  or 'invalid'.</rdfs:comment>
  </owl:Class>
  <owl:Class rdf:about="https://saref.etsi.org/saref4ener/LoadControlEventData">
    <rdfs:subClassOf>
      <owl:Restriction>
        <owl:onProperty rdf:resource="https://saref.etsi.org/core/hasTimestamp"/>
        <owl:allValuesFrom rdf:resource="http://www.w3.org/2001/XMLSchema#dateTime"/>
      </owl:Restriction>
    </rdfs:subClassOf>
    <rdfs:subClassOf>
      <owl:Restriction>
        <owl:onProperty rdf:resource="https://saref.etsi.org/core/hasTime"/>
        <owl:allValuesFrom>
          <owl:Class rdf:about="https://saref.etsi.org/saref4ener/TimePeriod"/>
        </owl:allValuesFrom>
      </owl:Restriction>
    </rdfs:subClassOf>
    <rdfs:subClassOf>
      <owl:Restriction>
        <owl:onProperty>
          <owl:ObjectProperty rdf:about="https://saref.etsi.org/saref4ener/hasDevice"/>
        </owl:onProperty>
        <owl:allValuesFrom rdf:resource="https://saref.etsi.org/saref4ener/Device"/>
      </owl:Restriction>
    </rdfs:subClassOf>
    <rdfs:subClassOf>
      <owl:Restriction>
        <owl:onProperty>
          <owl:ObjectProperty rdf:about="https://saref.etsi.org/saref4ener/triggersEventActionProduce"/>
        </owl:onProperty>
        <owl:allValuesFrom rdf:resource="https://saref.etsi.org/saref4ener/EventActionProduce"/>
      </owl:Restriction>
    </rdfs:subClassOf>
    <rdfs:subClassOf>
      <owl:Restriction>
        <owl:onProperty>
          <owl:ObjectProperty rdf:about="https://saref.etsi.org/saref4ener/triggersEventActionProduce"/>
        </owl:onProperty>
        <owl:onClass rdf:resource="https://saref.etsi.org/saref4ener/EventActionProduce"/>
        <owl:minQualifiedCardinality rdf:datatype="http://www.w3.org/2001/XMLSchema#nonNegativeInteger"
        >0</owl:minQualifiedCardinality>
      </owl:Restriction>
    </rdfs:subClassOf>
    <rdfs:subClassOf>
      <owl:Restriction>
        <owl:onProperty>
          <owl:ObjectProperty rdf:about="https://saref.etsi.org/saref4ener/triggersEventActionConsume"/>
        </owl:onProperty>
        <owl:onClass>
          <owl:Class rdf:about="https://saref.etsi.org/saref4ener/EventActionConsume"/>
        </owl:onClass>
        <owl:minQualifiedCardinality rdf:datatype="http://www.w3.org/2001/XMLSchema#nonNegativeInteger"
        >0</owl:minQualifiedCardinality>
      </owl:Restriction>
    </rdfs:subClassOf>
    <rdfs:subClassOf>
      <owl:Restriction>
        <owl:onProperty>
          <owl:ObjectProperty rdf:about="https://saref.etsi.org/saref4ener/hasDevice"/>
        </owl:onProperty>
        <owl:onClass rdf:resource="https://saref.etsi.org/saref4ener/Device"/>
        <owl:minQualifiedCardinality rdf:datatype="http://www.w3.org/2001/XMLSchema#nonNegativeInteger"
        >1</owl:minQualifiedCardinality>
      </owl:Restriction>
    </rdfs:subClassOf>
    <rdfs:subClassOf>
      <owl:Restriction>
        <owl:onProperty rdf:resource="https://saref.etsi.org/core/hasTimestamp"/>
        <owl:onDataRange rdf:resource="http://www.w3.org/2001/XMLSchema#dateTime"/>
        <owl:minQualifiedCardinality rdf:datatype="http://www.w3.org/2001/XMLSchema#nonNegativeInteger"
        >1</owl:minQualifiedCardinality>
      </owl:Restriction>
    </rdfs:subClassOf>
    <rdfs:subClassOf>
      <owl:Restriction>
        <owl:onProperty rdf:resource="https://saref.etsi.org/core/hasTime"/>
        <owl:onClass>
          <owl:Class rdf:about="https://saref.etsi.org/saref4ener/TimePeriod"/>
        </owl:onClass>
        <owl:minQualifiedCardinality rdf:datatype="http://www.w3.org/2001/XMLSchema#nonNegativeInteger"
        >1</owl:minQualifiedCardinality>
      </owl:Restriction>
    </rdfs:subClassOf>
    <rdfs:comment xml:lang="en">An event used to send overload warning severity level and related load control commands to a device (e.g. a household appliance or a smart meter).</rdfs:comment>
    <rdfs:subClassOf>
      <owl:Restriction>
        <owl:onProperty>
          <owl:ObjectProperty rdf:about="https://saref.etsi.org/saref4ener/triggersEventActionConsume"/>
        </owl:onProperty>
        <owl:allValuesFrom>
          <owl:Class rdf:about="https://saref.etsi.org/saref4ener/EventActionConsume"/>
        </owl:allValuesFrom>
      </owl:Restriction>
    </rdfs:subClassOf>
    <rdfs:subClassOf>
      <owl:Restriction>
        <owl:onProperty>
          <owl:DatatypeProperty rdf:about="https://saref.etsi.org/saref4ener/eventID"/>
        </owl:onProperty>
        <owl:minCardinality rdf:datatype="http://www.w3.org/2001/XMLSchema#nonNegativeInteger"
        >0</owl:minCardinality>
      </owl:Restriction>
    </rdfs:subClassOf>
    <rdfs:label xml:lang="en">Load control event data</rdfs:label>
  </owl:Class>
  <owl:Class rdf:about="https://saref.etsi.org/saref4ener/PowerMin">
    <rdfs:subClassOf rdf:resource="https://saref.etsi.org/saref4ener/Power"/>
    <rdfs:label xml:lang="en">Power min</rdfs:label>
    <rdfs:comment xml:lang="en">A possible type of power in a slot that represents the minimum power consumption and its value</rdfs:comment>
  </owl:Class>
  <owl:Class rdf:about="https://saref.etsi.org/saref4ener/PowerEnvelope">
    <rdfs:subClassOf rdf:resource="http://www.w3.org/2002/07/owl#Thing"/>
    <rdfs:label xml:lang="en">Power Envelope</rdfs:label>
    <rdfs:comment>A specific Power Envelope to be followed by an energy manager</rdfs:comment>
  </owl:Class>
  <owl:Class rdf:about="https://saref.etsi.org/saref4ener/CommodityQuantity">
    <rdfs:label xml:lang="en">Commodity Quantity</rdfs:label>
    <rdfs:comment>The various commodity quantities introduced by the S2 standard.</rdfs:comment>
  </owl:Class>
  <owl:Class rdf:about="https://saref.etsi.org/saref4ener/FRBCInstruction">
    <rdfs:subClassOf rdf:resource="https://saref.etsi.org/saref4ener/FlexibilityInstruction"/>
    <rdfs:label xml:lang="en">Fill Rate Based Control Instruction</rdfs:label>
    <rdfs:comment>A Fill Rate Based Instruction message. </rdfs:comment>
  </owl:Class>
  <owl:Class rdf:about="https://saref.etsi.org/saref4ener/IncentiveTableBasedProfile">
    <rdfs:subClassOf>
      <owl:Restriction>
        <owl:onProperty>
          <owl:ObjectProperty rdf:about="https://saref.etsi.org/saref4ener/hasScopeType"/>
        </owl:onProperty>
        <owl:allValuesFrom rdf:resource="https://saref.etsi.org/saref4ener/ScopeType"/>
      </owl:Restriction>
    </rdfs:subClassOf>
    <rdfs:subClassOf>
      <owl:Restriction>
        <owl:onProperty>
          <owl:DatatypeProperty rdf:about="https://saref.etsi.org/saref4ener/requiresUpdate"/>
        </owl:onProperty>
        <owl:allValuesFrom rdf:resource="http://www.w3.org/2001/XMLSchema#boolean"/>
      </owl:Restriction>
    </rdfs:subClassOf>
    <rdfs:subClassOf>
      <owl:Restriction>
        <owl:onProperty>
          <owl:DatatypeProperty rdf:about="https://saref.etsi.org/saref4ener/isChangeable"/>
        </owl:onProperty>
        <owl:allValuesFrom rdf:resource="http://www.w3.org/2001/XMLSchema#boolean"/>
      </owl:Restriction>
    </rdfs:subClassOf>
    <rdfs:subClassOf rdf:resource="https://saref.etsi.org/saref4ener/FlexibilityProfile"/>
    <rdfs:label xml:lang="en">Incentive table based profile</rdfs:label>
    <rdfs:comment xml:lang="en">This flexibility profile describes the usage of an incentive table to describe an incentive type in the form of costs (relative or absolute), CO2 emissions or renewable energy percentage that can be associated to power values (expressed as a time-series of power data-points).</rdfs:comment>
  </owl:Class>
  <owl:Class rdf:about="https://saref.etsi.org/saref4ener/Timer">
    <rdfs:subClassOf rdf:resource="http://www.w3.org/2002/07/owl#Thing"/>
    <rdfs:label xml:lang="en">Timer</rdfs:label>
    <rdfs:comment>A timer for time-based operation mode and transition constraints.</rdfs:comment>
  </owl:Class>
  <owl:Class rdf:about="https://saref.etsi.org/saref4ener/ActiveDurationMin">
    <owl:deprecated rdf:datatype="http://www.w3.org/2001/XMLSchema#boolean"
    >true</owl:deprecated>
    <rdfs:subClassOf rdf:resource="http://www.w3.org/2006/time#TemporalEntity"/>
    <rdfs:label xml:lang="en">Active duration min</rdfs:label>
    <rdfs:comment xml:lang="en">The active mininum duration a power sequence can run without interruption.</rdfs:comment>
  </owl:Class>
  <owl:Class rdf:about="https://saref.etsi.org/saref4ener/TimePeriod">
    <owl:deprecated rdf:datatype="http://www.w3.org/2001/XMLSchema#boolean"
    >true</owl:deprecated>
    <rdfs:subClassOf rdf:resource="http://www.w3.org/2006/time#TemporalEntity"/>
    <rdfs:label xml:lang="en">Time period</rdfs:label>
    <rdfs:comment xml:lang="en">The time period associated with load control event data</rdfs:comment>
  </owl:Class>
  <owl:Class rdf:about="https://saref.etsi.org/saref4ener/LoadControlStateData">
    <rdfs:subClassOf>
      <owl:Restriction>
        <owl:onProperty>
          <owl:ObjectProperty rdf:about="https://saref.etsi.org/saref4ener/hasEventStateConsume"/>
        </owl:onProperty>
        <owl:allValuesFrom rdf:resource="https://saref.etsi.org/saref4ener/EventStateConsume"/>
      </owl:Restriction>
    </rdfs:subClassOf>
    <rdfs:subClassOf>
      <owl:Restriction>
        <owl:onProperty>
          <owl:ObjectProperty rdf:about="https://saref.etsi.org/saref4ener/hasAppliedEventActionConsume"/>
        </owl:onProperty>
        <owl:onClass>
          <owl:Class rdf:about="https://saref.etsi.org/saref4ener/EventActionConsume"/>
        </owl:onClass>
        <owl:minQualifiedCardinality rdf:datatype="http://www.w3.org/2001/XMLSchema#nonNegativeInteger"
        >0</owl:minQualifiedCardinality>
      </owl:Restriction>
    </rdfs:subClassOf>
    <rdfs:label xml:lang="en">Load control state data</rdfs:label>
    <rdfs:subClassOf>
      <owl:Restriction>
        <owl:onProperty>
          <owl:ObjectProperty rdf:about="https://saref.etsi.org/saref4ener/hasAppliedEventActionProduce"/>
        </owl:onProperty>
        <owl:allValuesFrom rdf:resource="https://saref.etsi.org/saref4ener/EventActionProduce"/>
      </owl:Restriction>
    </rdfs:subClassOf>
    <rdfs:subClassOf>
      <owl:Restriction>
        <owl:onProperty>
          <owl:ObjectProperty rdf:about="https://saref.etsi.org/saref4ener/hasEventStateConsume"/>
        </owl:onProperty>
        <owl:onClass rdf:resource="https://saref.etsi.org/saref4ener/EventStateConsume"/>
        <owl:minQualifiedCardinality rdf:datatype="http://www.w3.org/2001/XMLSchema#nonNegativeInteger"
        >0</owl:minQualifiedCardinality>
      </owl:Restriction>
    </rdfs:subClassOf>
    <rdfs:subClassOf>
      <owl:Restriction>
        <owl:onProperty>
          <owl:ObjectProperty rdf:about="https://saref.etsi.org/saref4ener/hasEventStateProduce"/>
        </owl:onProperty>
        <owl:onClass rdf:resource="https://saref.etsi.org/saref4ener/EventStateProduce"/>
        <owl:minQualifiedCardinality rdf:datatype="http://www.w3.org/2001/XMLSchema#nonNegativeInteger"
        >0</owl:minQualifiedCardinality>
      </owl:Restriction>
    </rdfs:subClassOf>
    <rdfs:subClassOf>
      <owl:Restriction>
        <owl:onProperty>
          <owl:ObjectProperty rdf:about="https://saref.etsi.org/saref4ener/hasAppliedEventActionProduce"/>
        </owl:onProperty>
        <owl:onClass rdf:resource="https://saref.etsi.org/saref4ener/EventActionProduce"/>
        <owl:minQualifiedCardinality rdf:datatype="http://www.w3.org/2001/XMLSchema#nonNegativeInteger"
        >0</owl:minQualifiedCardinality>
      </owl:Restriction>
    </rdfs:subClassOf>
    <rdfs:subClassOf>
      <owl:Restriction>
        <owl:onProperty>
          <owl:DatatypeProperty rdf:about="https://saref.etsi.org/saref4ener/eventID"/>
        </owl:onProperty>
        <owl:onDataRange rdf:resource="http://www.w3.org/2001/XMLSchema#unsignedInt"/>
        <owl:minQualifiedCardinality rdf:datatype="http://www.w3.org/2001/XMLSchema#nonNegativeInteger"
        >0</owl:minQualifiedCardinality>
      </owl:Restriction>
    </rdfs:subClassOf>
    <rdfs:subClassOf>
      <owl:Restriction>
        <owl:onProperty rdf:resource="https://saref.etsi.org/core/hasTimestamp"/>
        <owl:onDataRange rdf:resource="http://www.w3.org/2001/XMLSchema#dateTime"/>
        <owl:minQualifiedCardinality rdf:datatype="http://www.w3.org/2001/XMLSchema#nonNegativeInteger"
        >1</owl:minQualifiedCardinality>
      </owl:Restriction>
    </rdfs:subClassOf>
    <rdfs:subClassOf>
      <owl:Restriction>
        <owl:onProperty>
          <owl:ObjectProperty rdf:about="https://saref.etsi.org/saref4ener/hasEventStateProduce"/>
        </owl:onProperty>
        <owl:allValuesFrom rdf:resource="https://saref.etsi.org/saref4ener/EventStateProduce"/>
      </owl:Restriction>
    </rdfs:subClassOf>
    <rdfs:comment xml:lang="en">The representation of the state of an event used to send overload warning severity level and related load control commands to a device (e.g. a household appliance or a smart meter).</rdfs:comment>
    <rdfs:subClassOf>
      <owl:Restriction>
        <owl:onProperty rdf:resource="https://saref.etsi.org/core/hasTimestamp"/>
        <owl:allValuesFrom rdf:resource="http://www.w3.org/2001/XMLSchema#dateTime"/>
      </owl:Restriction>
    </rdfs:subClassOf>
    <rdfs:subClassOf>
      <owl:Restriction>
        <owl:onProperty>
          <owl:ObjectProperty rdf:about="https://saref.etsi.org/saref4ener/hasAppliedEventActionConsume"/>
        </owl:onProperty>
        <owl:allValuesFrom>
          <owl:Class rdf:about="https://saref.etsi.org/saref4ener/EventActionConsume"/>
        </owl:allValuesFrom>
      </owl:Restriction>
    </rdfs:subClassOf>
  </owl:Class>
  <owl:Class rdf:about="https://saref.etsi.org/saref4ener/PowerEnvelopeProfile">
    <rdfs:subClassOf rdf:resource="https://saref.etsi.org/saref4ener/FlexibilityProfile"/>
    <rdfs:label xml:lang="en">Power envelope control</rdfs:label>
    <rdfs:comment>A Flexibility Profile described through a Power Envelope Profile.</rdfs:comment>
  </owl:Class>
  <owl:Class rdf:about="https://saref.etsi.org/saref4ener/EventActionConsume">
    <owl:oneOf rdf:parseType="Collection">
      <s4ener:EventActionProduce rdf:about="https://saref.etsi.org/saref4ener/Pause"/>
      <s4ener:EventActionProduce rdf:about="https://saref.etsi.org/saref4ener/Resume"/>
      <s4ener:EventActionProduce rdf:about="https://saref.etsi.org/saref4ener/Reduce"/>
      <s4ener:EventActionProduce rdf:about="https://saref.etsi.org/saref4ener/Increase"/>
      <s4ener:EventActionProduce rdf:about="https://saref.etsi.org/saref4ener/Emergency"/>
      <s4ener:EventActionProduce rdf:about="https://saref.etsi.org/saref4ener/Normal"/>
    </owl:oneOf>
    <rdfs:subClassOf>
      <owl:Class rdf:about="https://saref.etsi.org/saref4ener/LoadControlEventAction"/>
    </rdfs:subClassOf>
    <rdfs:label xml:lang="en">Event action consume</rdfs:label>
    <rdfs:comment xml:lang="en">An action type used to express a consume action to be performed as a consequence of an event used to send overload warning severity level and related load control commands to a device (e.g. a household appliance or a smart meter).</rdfs:comment>
  </owl:Class>
  <owl:Class rdf:about="https://saref.etsi.org/saref4ener/ResumeEnergyEstimated">
    <rdfs:subClassOf rdf:resource="https://saref.etsi.org/saref4ener/Energy"/>
    <rdfs:label xml:lang="en">Resume energy estimated</rdfs:label>
    <rdfs:comment xml:lang="en">In a power sequence, the additional energy the device will consume before resuming its normal operation (after a pause). This is only an estimated value which will not be added to the value stated in any slot value information.</rdfs:comment>
  </owl:Class>
  <owl:Class rdf:about="https://saref.etsi.org/saref4ener/EnergySkewness">
    <rdfs:subClassOf rdf:resource="https://saref.etsi.org/saref4ener/Energy"/>
    <rdfs:label xml:lang="en">Energy skewness</rdfs:label>
    <rdfs:comment xml:lang="en">A possible type of energy in a slot that represents the energy skewness and its value</rdfs:comment>
  </owl:Class>
  <owl:Class rdf:about="https://saref.etsi.org/saref4ener/OperationModeProfile">
    <rdfs:subClassOf rdf:resource="https://saref.etsi.org/saref4ener/FlexibilityProfile"/>
    <rdfs:label xml:lang="en">Operation mode control</rdfs:label>
    <rdfs:comment>A resource manager can declare multiple operation modes for a device. An operation mode is a mode/state that a device can find itself in, that is associated with a specific power value.</rdfs:comment>
  </owl:Class>
  <owl:Class rdf:about="https://saref.etsi.org/saref4ener/EnergyMin">
    <rdfs:subClassOf rdf:resource="https://saref.etsi.org/saref4ener/Energy"/>
    <rdfs:label xml:lang="en">Energy min</rdfs:label>
    <rdfs:comment xml:lang="en">A possible type of energy in a slot that represents the minimum energy consumption and its value</rdfs:comment>
  </owl:Class>
  <owl:Class rdf:about="https://saref.etsi.org/saref4ener/Transition">
    <rdfs:subClassOf rdf:resource="http://www.w3.org/2002/07/owl#Thing"/>
    <rdfs:label xml:lang="en">Transition</rdfs:label>
    <rdfs:comment>Possible transitions to switch from one Operation Mode to another or to set new parameters.</rdfs:comment>
  </owl:Class>
  <owl:Class rdf:about="https://saref.etsi.org/saref4ener/InstructionStatus">
    <rdfs:subClassOf rdf:resource="http://www.w3.org/2002/07/owl#Thing"/>
    <rdfs:label xml:lang="en">Instruction Status</rdfs:label>
    <rdfs:comment>The status an instruction has at a specific moment.</rdfs:comment>
  </owl:Class>
  <owl:Class rdf:about="https://saref.etsi.org/saref4ener/PowerLimitProfile">
    <rdfs:subClassOf rdf:resource="https://saref.etsi.org/saref4ener/FlexibilityProfile"/>
    <rdfs:label xml:lang="en">Power limit profile</rdfs:label>
    <rdfs:comment>This profile describes the energy flexibility of a device via a set of power limits, following the SPINE documentation</rdfs:comment>
  </owl:Class>
  <owl:Class rdf:about="https://saref.etsi.org/saref4ener/PowerMax">
    <rdfs:subClassOf rdf:resource="https://saref.etsi.org/saref4ener/Power"/>
    <rdfs:label xml:lang="en">Power max</rdfs:label>
    <rdfs:comment xml:lang="en">A possible type of power in a slot that represents the maximum power consumption and its value</rdfs:comment>
  </owl:Class>
  <owl:Class rdf:about="https://saref.etsi.org/saref4ener/IncentiveTableSlot">
    <rdfs:subClassOf rdf:resource="https://saref.etsi.org/saref4ener/Slot"/>
    <rdfs:label xml:lang="en">Incentive table slot</rdfs:label>
    <rdfs:comment>This concept describes a slot that belongs to a Incentive Table. Each slot of the Incentive Table consists of a series of (lower) boundaries, each indicating the power at which a change to another incentive takes place. Additionally, each boundary is associated with a IncentiveTableTier.</rdfs:comment>
  </owl:Class>
  <owl:Class rdf:about="https://saref.etsi.org/saref4ener/LoadControlEventAction">
    <rdfs:label xml:lang="en">Load Control event action</rdfs:label>
    <rdfs:comment xml:lang="en">An action type used to express the action to be performed as a consequence of an event used to send overload warning severity level and related load control commands to a device (e.g. a household appliance or a smart meter).</rdfs:comment>
  </owl:Class>
  <owl:ObjectProperty rdf:about="https://saref.etsi.org/saref4ener/hasNominalConsumption">
    <rdfs:subPropertyOf>
      <owl:ObjectProperty rdf:about="https://saref.etsi.org/saref4ener/hasPowerLimitConsumptionMax"/>
    </rdfs:subPropertyOf>
    <rdfs:range rdf:resource="https://saref.etsi.org/core/Measurement"/>
    <rdfs:label xml:lang="en">has nominal consumption Max</rdfs:label>
    <rdfs:domain rdf:resource="https://saref.etsi.org/saref4ener/NominalPowerLimit"/>
    <rdfs:comment xml:lang="en">The relationship between the nominal power limit and the value indicating the max limit consumption.</rdfs:comment>
  </owl:ObjectProperty>
  <owl:ObjectProperty rdf:about="https://saref.etsi.org/saref4ener/hasAppliedEventActionProduce">
    <rdfs:label xml:lang="en">has applied event action produce</rdfs:label>
    <rdfs:comment xml:lang="en">A relationship between the state of a load control event produce and the action to be performed as a consequence of this event.</rdfs:comment>
  </owl:ObjectProperty>
  <owl:ObjectProperty rdf:about="https://saref.etsi.org/saref4ener/hasLeakageBehaviourElement">
    <rdfs:range rdf:resource="https://saref.etsi.org/saref4ener/LeakageBehaviourElement"/>
    <rdfs:label xml:lang="en">has leakage behaviour element</rdfs:label>
    <rdfs:domain rdf:resource="https://saref.etsi.org/saref4ener/LeakageBehaviour"/>
    <rdfs:comment>This property relates the LeakageBehaviour description to the LeakageBehaviourElements indicating the detailed description.</rdfs:comment>
  </owl:ObjectProperty>
  <owl:ObjectProperty rdf:about="https://saref.etsi.org/saref4ener/hasActivationPlan">
    <rdfs:range rdf:resource="https://saref.etsi.org/saref4ener/TimeSeries"/>
    <rdfs:label xml:lang="en">has activation plan</rdfs:label>
    <rdfs:domain rdf:resource="https://saref.etsi.org/saref4ener/FlexibilityInstruction"/>
    <rdfs:comment xml:lang="en">The relationship between the s4ener:FlexibilityInstruction and s4ener:TimeSeries.</rdfs:comment>
  </owl:ObjectProperty>
  <owl:ObjectProperty rdf:about="https://saref.etsi.org/saref4ener/startsTimer">
    <rdfs:range rdf:resource="https://saref.etsi.org/saref4ener/Timer"/>
    <rdfs:label xml:lang="en">Starts Timer</rdfs:label>
    <rdfs:domain rdf:resource="https://saref.etsi.org/saref4ener/Transition"/>
    <rdfs:comment>List of IDs of Timers that will be (re)started when this transition is initiated</rdfs:comment>
  </owl:ObjectProperty>
  <owl:ObjectProperty rdf:about="https://saref.etsi.org/saref4ener/hasCost">
    <rdfs:range rdf:resource="https://saref.etsi.org/saref4ener/DataPoint"/>
    <rdfs:label xml:lang="en">hasCost</rdfs:label>
    <rdfs:label xml:lang="en">has cost</rdfs:label>
    <rdfs:domain rdf:resource="https://saref.etsi.org/saref4ener/OperationMode"/>
    <rdfs:domain rdf:resource="https://saref.etsi.org/saref4ener/FlexibilityInstruction"/>
    <rdfs:comment xml:lang="en">The relationship between the s4ener:FlexibilityInstruction and s4ener:DataPoint</rdfs:comment>
    <rdfs:comment> Additional costs per second (e.g. wear, services) associated with this operation mode in the currency defined by the ResourceManagerDetails , excluding the commodity cost. The range is expressing uncertainty and is not linked to the operation_mode_factor.</rdfs:comment>
  </owl:ObjectProperty>
  <owl:ObjectProperty rdf:about="https://saref.etsi.org/saref4ener/hasDevice">
    <rdfs:label xml:lang="en">has device</rdfs:label>
    <rdfs:comment xml:lang="en">A relationship between a load control event (used to send overload warning severity level and related load control commands) and the device interested by this event.</rdfs:comment>
  </owl:ObjectProperty>
  <owl:ObjectProperty rdf:about="https://saref.etsi.org/saref4ener/valueTendency">
    <rdfs:range rdf:resource="https://saref.etsi.org/saref4ener/ValueTendency"/>
    <rdfs:label xml:lang="en">value tendency</rdfs:label>
    <rdfs:comment xml:lang="en">Indicates whether the tendency of a measurement is rising, stable, or falling.</rdfs:comment>
  </owl:ObjectProperty>
  <owl:ObjectProperty rdf:about="https://saref.etsi.org/saref4ener/receivesPowerLimit">
    <rdfs:range rdf:resource="https://saref.etsi.org/saref4ener/PowerLimit"/>
    <rdfs:label xml:lang="en">receives power limit</rdfs:label>
    <rdfs:domain rdf:resource="https://saref.etsi.org/saref4ener/PowerLimitProfile"/>
    <rdfs:comment xml:lang="en">The relationship between a power limit profile and the power limit it has received for its device to follow</rdfs:comment>
  </owl:ObjectProperty>
  <owl:ObjectProperty rdf:about="https://saref.etsi.org/saref4ener/relatesToPowerProfileSequence">
    <rdfs:range rdf:resource="https://saref.etsi.org/saref4ener/PowerSequence"/>
    <rdfs:label xml:lang="en">Relates to power profile sequence</rdfs:label>
    <rdfs:domain rdf:resource="https://saref.etsi.org/saref4ener/PPBCInstruction"/>
    <rdfs:comment>ID of the PPBC.PowerSequence that is being selected and scheduled by the CEM.</rdfs:comment>
  </owl:ObjectProperty>
  <owl:ObjectProperty rdf:about="https://saref.etsi.org/saref4ener/hasEventStateProduce">
    <rdfs:subPropertyOf rdf:resource="https://saref.etsi.org/core/hasState"/>
    <rdfs:label xml:lang="en">has event state produce</rdfs:label>
    <rdfs:comment xml:lang="en">A relationship between the specification of the state of a load control event produce and the value that this state can assume.</rdfs:comment>
  </owl:ObjectProperty>
  <owl:ObjectProperty rdf:about="https://saref.etsi.org/saref4ener/hasSlotValue">
    <rdfs:range>
      <owl:Restriction>
        <owl:onProperty rdf:resource="https://saref.etsi.org/core/relatesToProperty"/>
        <owl:onClass>
          <owl:Class>
            <owl:unionOf rdf:parseType="Collection">
              <rdf:Description rdf:about="https://saref.etsi.org/core/Energy"/>
              <rdf:Description rdf:about="https://saref.etsi.org/core/Power"/>
            </owl:unionOf>
          </owl:Class>
        </owl:onClass>
        <owl:minQualifiedCardinality rdf:datatype="http://www.w3.org/2001/XMLSchema#nonNegativeInteger"
        >1</owl:minQualifiedCardinality>
      </owl:Restriction>
    </rdfs:range>
    <rdfs:range rdf:resource="https://saref.etsi.org/core/Measurement"/>
    <rdfs:label xml:lang="en">has slot value</rdfs:label>
    <rdfs:domain rdf:resource="https://saref.etsi.org/saref4ener/Slot"/>
    <rdfs:comment>This property is intended to specify the power or energy value of a slot in a power sequence as part of a power profile.&#xD;
&#xD;
This property is a suggestion to be added in Saref4Energy v2.</rdfs:comment>
  </owl:ObjectProperty>
  <owl:ObjectProperty rdf:about="https://saref.etsi.org/saref4ener/startOfRange">
    <rdfs:range rdf:resource="https://saref.etsi.org/core/Measurement"/>
    <rdfs:label xml:lang="en">start of range</rdfs:label>
    <rdfs:domain rdf:resource="https://saref.etsi.org/saref4ener/NumberRange"/>
    <rdfs:comment>This property indicates the start of a number range.</rdfs:comment>
  </owl:ObjectProperty>
  <owl:ObjectProperty rdf:about="https://saref.etsi.org/saref4ener/hasPowerSequenceContainer">
    <rdfs:range rdf:resource="https://saref.etsi.org/saref4ener/PowerSequenceContainer"/>
    <rdfs:label xml:lang="en">has power sequence container</rdfs:label>
    <rdfs:domain rdf:resource="https://saref.etsi.org/saref4ener/PowerProfile"/>
    <rdfs:comment>The various power sequence containers contained within an S2 Power Profile. The containers have to executed one after the other. Each container contains various Power Sequence anong which the EMS can choose the appropriate Power Sequence for the current energy demands.</rdfs:comment>
  </owl:ObjectProperty>
  <owl:ObjectProperty rdf:about="https://saref.etsi.org/saref4ener/hasActiveOperationMode">
    <rdfs:range rdf:resource="https://saref.etsi.org/saref4ener/OperationMode"/>
    <rdfs:label xml:lang="en">has active operation mode</rdfs:label>
    <rdfs:domain>
      <owl:Class>
        <owl:unionOf rdf:parseType="Collection">
          <owl:Class rdf:about="https://saref.etsi.org/saref4ener/OperationMode"/>
          <rdf:Description rdf:about="https://saref.etsi.org/core/Actuator"/>
        </owl:unionOf>
      </owl:Class>
    </rdfs:domain>
    <rdfs:comment>A reference to the OperationMode that is presently active</rdfs:comment>
  </owl:ObjectProperty>
  <owl:ObjectProperty rdf:about="https://saref.etsi.org/saref4ener/hasDataPoint">
    <rdfs:range rdf:resource="https://saref.etsi.org/saref4ener/DataPoint"/>
    <rdfs:label xml:lang="en">has data point</rdfs:label>
    <rdfs:domain rdf:resource="https://saref.etsi.org/saref4ener/TimeSeries"/>
    <rdfs:comment xml:lang="en">This relationship connects a time series to data point.</rdfs:comment>
  </owl:ObjectProperty>
  <owl:ObjectProperty rdf:about="https://saref.etsi.org/saref4ener/hasTransition">
    <rdfs:range rdf:resource="https://saref.etsi.org/saref4ener/Transition"/>
    <rdfs:label xml:lang="en">has transition</rdfs:label>
    <rdfs:domain>
      <owl:Class>
        <owl:unionOf rdf:parseType="Collection">
          <rdf:Description rdf:about="https://saref.etsi.org/core/Actuator"/>
          <owl:Class rdf:about="https://saref.etsi.org/saref4ener/OperationModeProfile"/>
        </owl:unionOf>
      </owl:Class>
    </rdfs:domain>
    <rdfs:comment>The transitions between various saref:States or s4ener:OperationModes that either the Actuator or the OperationModeProfile can support.</rdfs:comment>
  </owl:ObjectProperty>
  <owl:ObjectProperty rdf:about="https://saref.etsi.org/saref4ener/hasNumberRange">
    <rdfs:range rdf:resource="https://saref.etsi.org/saref4ener/NumberRange"/>
    <rdfs:label xml:lang="en">has number range</rdfs:label>
    <rdfs:domain rdf:resource="https://saref.etsi.org/saref4ener/PowerRange"/>
    <rdfs:comment>This property provides the association between a power range and its number range.</rdfs:comment>
  </owl:ObjectProperty>
  <owl:ObjectProperty rdf:about="https://saref.etsi.org/saref4ener/hasInstructionStatus">
    <rdfs:range rdf:resource="https://saref.etsi.org/saref4ener/InstructionStatus"/>
    <rdfs:label xml:lang="en">has Instruction Status</rdfs:label>
    <rdfs:comment>Present status of this instruction.</rdfs:comment>
  </owl:ObjectProperty>
  <owl:ObjectProperty rdf:about="https://saref.etsi.org/saref4ener/hasConsequenceType">
    <rdfs:range rdf:resource="https://saref.etsi.org/saref4ener/PowerEnvelopeConsequenceType"/>
    <rdfs:label xml:lang="en">Has Consequence Type</rdfs:label>
    <rdfs:domain rdf:resource="https://saref.etsi.org/saref4ener/PowerConstraint"/>
    <rdfs:comment>The consequence type associated with this Power Constraint, which can be Defer or Vanish.</rdfs:comment>
  </owl:ObjectProperty>
  <owl:ObjectProperty rdf:about="https://saref.etsi.org/saref4ener/hasIncentiveType">
    <rdfs:range rdf:resource="https://saref.etsi.org/saref4ener/IncentiveType"/>
    <rdfs:label xml:lang="en">has incentive type</rdfs:label>
    <rdfs:domain rdf:resource="https://saref.etsi.org/saref4ener/IncentiveTableTier"/>
    <rdfs:comment xml:lang="en">The relationship between the tier and its incentive type</rdfs:comment>
  </owl:ObjectProperty>
  <owl:ObjectProperty rdf:about="https://saref.etsi.org/saref4ener/hasRunningCosts">
    <rdfs:range rdf:resource="https://saref.etsi.org/saref4ener/NumberRange"/>
    <rdfs:label xml:lang="en">has running costs</rdfs:label>
    <rdfs:domain rdf:resource="https://saref.etsi.org/saref4ener/OperationModeElement"/>
    <rdfs:comment>Additional costs per second (e.g. wear, services) associated with this operation mode in the currency defined by the ResourceManagerDetails , excluding the commodity cost. The range is expressing uncertainty and is not linked to the operation_mode_factor.</rdfs:comment>
  </owl:ObjectProperty>
  <owl:ObjectProperty rdf:about="https://saref.etsi.org/saref4ener/hasScopeType">
    <rdfs:range rdf:resource="https://saref.etsi.org/saref4ener/ScopeType"/>
    <rdfs:label xml:lang="en">has scope type</rdfs:label>
    <rdfs:domain rdf:resource="https://saref.etsi.org/saref4ener/IncentiveTableBasedProfile"/>
    <rdfs:comment xml:lang="en">The relationship between the incentive table and the scope type</rdfs:comment>
  </owl:ObjectProperty>
  <owl:ObjectProperty rdf:about="https://saref.etsi.org/saref4ener/isActuatedBy">
    <rdfs:range rdf:resource="https://saref.etsi.org/core/Actuator"/>
    <rdfs:label xml:lang="en">is actuated by</rdfs:label>
    <rdfs:domain>
      <owl:Class>
        <owl:unionOf rdf:parseType="Collection">
          <owl:Class rdf:about="https://saref.etsi.org/saref4ener/DemandDrivenProfile"/>
          <owl:Class rdf:about="https://saref.etsi.org/saref4ener/FillRateProfile"/>
          <owl:Class rdf:about="https://saref.etsi.org/saref4ener/FRBCInstruction"/>
          <owl:Class rdf:about="https://saref.etsi.org/saref4ener/DDBCInstruction"/>
        </owl:unionOf>
      </owl:Class>
    </rdfs:domain>
    <rdfs:comment>A reference to an (external) actuator that can potentially activate this profile or where the instruction originates from.</rdfs:comment>
  </owl:ObjectProperty>
  <owl:ObjectProperty rdf:about="https://saref.etsi.org/saref4ener/hasExpression">
    <owl:deprecated rdf:datatype="http://www.w3.org/2001/XMLSchema#boolean"
    >true</owl:deprecated>
    <rdfs:label xml:lang="en">has expression</rdfs:label>
    <rdfs:comment xml:lang="en">A relationship between an appliance parameter compatibility action and the associated expressions</rdfs:comment>
  </owl:ObjectProperty>
  <owl:ObjectProperty rdf:about="https://saref.etsi.org/saref4ener/hasCommodity">
    <rdfs:range rdf:resource="https://saref.etsi.org/core/Commodity"/>
    <rdfs:label xml:lang="en">Uses commodity</rdfs:label>
    <rdfs:domain rdf:resource="https://saref.etsi.org/saref4ener/Role"/>
    <rdfs:comment>An indication of which commodity this Role is a consumer, producer, or storer of.</rdfs:comment>
  </owl:ObjectProperty>
  <owl:ObjectProperty rdf:about="https://saref.etsi.org/saref4ener/toOperationMode">
    <rdfs:range rdf:resource="https://saref.etsi.org/saref4ener/OperationMode"/>
    <rdfs:label xml:lang="en">to state operation mode</rdfs:label>
    <rdfs:domain rdf:resource="https://saref.etsi.org/saref4ener/Transition"/>
    <rdfs:comment>ID of the OperationMode (exact type differs per ControlType) that will be switched to.</rdfs:comment>
  </owl:ObjectProperty>
  <owl:ObjectProperty rdf:about="https://saref.etsi.org/saref4ener/triggersEventActionProduce">
    <rdfs:label xml:lang="en">triggers event action produce</rdfs:label>
    <rdfs:comment xml:lang="en">A relationship between a load control event and the produce action triggered by this event</rdfs:comment>
  </owl:ObjectProperty>
  <owl:ObjectProperty rdf:about="https://saref.etsi.org/saref4ener/endOfRange">
    <rdfs:range rdf:resource="https://saref.etsi.org/core/Measurement"/>
    <rdfs:label xml:lang="en">end of range</rdfs:label>
    <rdfs:domain rdf:resource="https://saref.etsi.org/saref4ener/NumberRange"/>
    <rdfs:comment>This property indicates the end of a number range.</rdfs:comment>
  </owl:ObjectProperty>
  <owl:ObjectProperty rdf:about="https://saref.etsi.org/saref4ener/hasStorage">
    <rdfs:range rdf:resource="https://saref.etsi.org/saref4ener/Storage"/>
    <rdfs:label xml:lang="en">has storage</rdfs:label>
    <rdfs:domain rdf:resource="https://saref.etsi.org/saref4ener/FillRateProfile"/>
    <rdfs:comment>The storage regulated by the related Fill Rate Profile.</rdfs:comment>
  </owl:ObjectProperty>
  <owl:ObjectProperty rdf:about="https://saref.etsi.org/saref4ener/hasContractualConsumptionMax">
    <rdfs:subPropertyOf>
      <owl:ObjectProperty rdf:about="https://saref.etsi.org/saref4ener/hasPowerLimitConsumptionMax"/>
    </rdfs:subPropertyOf>
    <rdfs:range rdf:resource="https://saref.etsi.org/core/Measurement"/>
    <rdfs:label xml:lang="en">has contractual consumption Max</rdfs:label>
    <rdfs:domain rdf:resource="https://saref.etsi.org/saref4ener/ContractualPowerLimit"/>
    <rdfs:comment xml:lang="en">The relationship between the contractual power limit and the value indicating the max limit consumption.</rdfs:comment>
  </owl:ObjectProperty>
  <owl:ObjectProperty rdf:about="https://saref.etsi.org/saref4ener/fillRate">
    <rdfs:range rdf:resource="https://saref.etsi.org/saref4ener/NumberRange"/>
    <rdfs:label xml:lang="en">Fill Rate Level</rdfs:label>
    <rdfs:domain>
      <owl:Class>
        <owl:unionOf rdf:parseType="Collection">
          <owl:Class rdf:about="https://saref.etsi.org/saref4ener/Storage"/>
          <owl:Class rdf:about="https://saref.etsi.org/saref4ener/OperationModeElement"/>
        </owl:unionOf>
      </owl:Class>
    </rdfs:domain>
    <rdfs:comment>Indicates the change in fill_level per second. The lower_boundary of the NumberRange is associated with an operation_mode_factor of 0, the upper_boundary is associated with an operation_mode_factor of 1.</rdfs:comment>
  </owl:ObjectProperty>
  <owl:ObjectProperty rdf:about="https://saref.etsi.org/saref4ener/hasUsage">
    <rdfs:range rdf:resource="https://saref.etsi.org/saref4ener/Usage"/>
    <rdfs:label xml:lang="en">has usage</rdfs:label>
    <rdfs:comment xml:lang="en">This property provides the possibility to add some additional information about the usage of a data-point or time-series. For example, a data point or time series can be used as an upper limit, lower limit or a baseline, a maximum versus minimum value, or a consumption versus a production value.</rdfs:comment>
  </owl:ObjectProperty>
  <owl:ObjectProperty rdf:about="https://saref.etsi.org/saref4ener/hasFailsafeProductionMax">
    <rdfs:subPropertyOf>
      <owl:ObjectProperty rdf:about="https://saref.etsi.org/saref4ener/hasPowerLimitProductionMax"/>
    </rdfs:subPropertyOf>
    <rdfs:range rdf:resource="https://saref.etsi.org/core/Measurement"/>
    <rdfs:label xml:lang="en">has failsafe production max</rdfs:label>
    <rdfs:domain rdf:resource="https://saref.etsi.org/saref4ener/FailsafePowerLimit"/>
    <rdfs:comment xml:lang="en">The relationship between the failsafe power limit and the value indicating its production.</rdfs:comment>
  </owl:ObjectProperty>
  <owl:ObjectProperty rdf:about="https://saref.etsi.org/saref4ener/hasConnection">
    <owl:deprecated rdf:datatype="http://www.w3.org/2001/XMLSchema#boolean"
    >true</owl:deprecated>
    <rdfs:label xml:lang="en">has connection</rdfs:label>
    <rdfs:comment xml:lang="en">In the Remote Network Management (RemoteNWM) use case, a relationship between a node in a network (i.e., a s4ee:Device) and its connections (i.e., a s4ee:DeviceConnections). The same s4ee:Device (or node) can have multiple device connections as it can be connected to several networks at the same time.</rdfs:comment>
  </owl:ObjectProperty>
  <owl:ObjectProperty rdf:about="https://saref.etsi.org/saref4ener/hasRecipient">
    <rdfs:label xml:lang="en">has recipient</rdfs:label>
    <rdfs:comment xml:lang="en">This property can be used to connect a flexibility offer or/and flexibility request to a foaf:agent or saref:Device.</rdfs:comment>
  </owl:ObjectProperty>
  <owl:ObjectProperty rdf:about="https://saref.etsi.org/saref4ener/hasContractualProductionMax">
    <rdfs:subPropertyOf>
      <owl:ObjectProperty rdf:about="https://saref.etsi.org/saref4ener/hasPowerLimitProductionMax"/>
    </rdfs:subPropertyOf>
    <rdfs:range rdf:resource="https://saref.etsi.org/core/Measurement"/>
    <rdfs:label xml:lang="en">has contractual production Max</rdfs:label>
    <rdfs:domain rdf:resource="https://saref.etsi.org/saref4ener/ContractualPowerLimit"/>
    <rdfs:comment xml:lang="en">The relationship between the contractual power limit and the value indicating the max limit production.</rdfs:comment>
  </owl:ObjectProperty>
  <owl:ObjectProperty rdf:about="https://saref.etsi.org/saref4ener/isBoundTo">
    <rdfs:range rdf:resource="https://saref.etsi.org/saref4ener/ContractualPowerLimit"/>
    <rdfs:label xml:lang="en">is bound to</rdfs:label>
    <rdfs:domain rdf:resource="https://saref.etsi.org/saref4ener/PowerLimitProfile"/>
    <rdfs:comment xml:lang="en">The relationship between a device and its contractual power limit</rdfs:comment>
  </owl:ObjectProperty>
  <owl:ObjectProperty rdf:about="https://saref.etsi.org/saref4ener/hasFillLevelRange">
    <rdfs:range rdf:resource="https://saref.etsi.org/saref4ener/NumberRange"/>
    <rdfs:label xml:lang="en">Fill Level Range</rdfs:label>
    <rdfs:domain>
      <owl:Class>
        <owl:unionOf rdf:parseType="Collection">
          <owl:Class rdf:about="https://saref.etsi.org/saref4ener/Storage"/>
          <owl:Class rdf:about="https://saref.etsi.org/saref4ener/OperationModeElement"/>
          <owl:Class rdf:about="https://saref.etsi.org/saref4ener/LeakageBehaviourElement"/>
          <owl:Class rdf:about="https://saref.etsi.org/saref4ener/FillLevelTargetProfileElement"/>
        </owl:unionOf>
      </owl:Class>
    </rdfs:domain>
    <rdfs:comment>The range of the fill level for which this FRBC.OperationModeElement applies. &#xD;
&#xD;
If this concept is applied on a Storage it indicated the range in which a storage should remain.</rdfs:comment>
  </owl:ObjectProperty>
  <owl:ObjectProperty rdf:about="https://saref.etsi.org/saref4ener/hasEnergyValueType">
    <rdfs:subPropertyOf>
      <owl:ObjectProperty rdf:about="https://saref.etsi.org/saref4ener/hasValueType"/>
    </rdfs:subPropertyOf>
    <rdfs:label xml:lang="en">has energy value type</rdfs:label>
    <rdfs:comment xml:lang="en">A relationship representing an energy value type</rdfs:comment>
  </owl:ObjectProperty>
  <owl:ObjectProperty rdf:about="https://saref.etsi.org/saref4ener/hasFailsafeConsumptionMax">
    <rdfs:subPropertyOf>
      <owl:ObjectProperty rdf:about="https://saref.etsi.org/saref4ener/hasPowerLimitConsumptionMax"/>
    </rdfs:subPropertyOf>
    <rdfs:range rdf:resource="https://saref.etsi.org/core/Measurement"/>
    <rdfs:label xml:lang="en">has failsafe consumption max</rdfs:label>
    <rdfs:domain rdf:resource="https://saref.etsi.org/saref4ener/FailsafePowerLimit"/>
    <rdfs:comment xml:lang="en">The relationship between the failsafe power limit and the value indicating its consumption.</rdfs:comment>
  </owl:ObjectProperty>
  <owl:ObjectProperty rdf:about="https://saref.etsi.org/saref4ener/isBlockedBy">
    <rdfs:range rdf:resource="https://saref.etsi.org/saref4ener/Timer"/>
    <rdfs:label xml:lang="en">is blocked by</rdfs:label>
    <rdfs:domain rdf:resource="https://saref.etsi.org/saref4ener/Transition"/>
    <rdfs:comment>The Timers that block this Transition from initiating while at least one of these Timers is not yet finished</rdfs:comment>
  </owl:ObjectProperty>
  <owl:ObjectProperty rdf:about="https://saref.etsi.org/saref4ener/hasPowerValueType">
    <rdfs:subPropertyOf>
      <owl:ObjectProperty rdf:about="https://saref.etsi.org/saref4ener/hasValueType"/>
    </rdfs:subPropertyOf>
    <rdfs:label xml:lang="en">has power value type</rdfs:label>
    <rdfs:comment xml:lang="en">A relationship representing a power value type</rdfs:comment>
  </owl:ObjectProperty>
  <owl:ObjectProperty rdf:about="https://saref.etsi.org/saref4ener/relatesToRequest">
    <rdfs:range rdf:resource="https://saref.etsi.org/saref4ener/FlexRequest"/>
    <rdfs:label xml:lang="en">relates to request</rdfs:label>
    <rdfs:domain rdf:resource="https://saref.etsi.org/saref4ener/FlexOffer"/>
    <rdfs:comment xml:lang="en">The relationship between the flexibility offer and flexibility request</rdfs:comment>
  </owl:ObjectProperty>
  <owl:ObjectProperty rdf:about="https://saref.etsi.org/saref4ener/hasValueType">
    <rdfs:label xml:lang="en">has value type</rdfs:label>
    <rdfs:comment xml:lang="en">A relation representing the value type of an entity</rdfs:comment>
  </owl:ObjectProperty>
  <owl:ObjectProperty rdf:about="https://saref.etsi.org/saref4ener/hasDemandRate">
    <rdfs:range rdf:resource="https://saref.etsi.org/saref4ener/NumberRange"/>
    <rdfs:label xml:lang="en">has demand rate</rdfs:label>
    <rdfs:domain rdf:resource="https://saref.etsi.org/saref4ener/DemandDrivenProfile"/>
    <rdfs:comment>The present demand rate that needs to be satisfied by the system</rdfs:comment>
  </owl:ObjectProperty>
  <owl:ObjectProperty rdf:about="https://saref.etsi.org/saref4ener/hasRoleType">
    <rdfs:range rdf:resource="https://saref.etsi.org/saref4ener/RoleType"/>
    <rdfs:label xml:lang="en">role type</rdfs:label>
    <rdfs:domain rdf:resource="https://saref.etsi.org/saref4ener/Role"/>
    <rdfs:comment>The type of this specific role</rdfs:comment>
  </owl:ObjectProperty>
  <owl:ObjectProperty rdf:about="https://saref.etsi.org/saref4ener/hasSupplyRange">
    <rdfs:range rdf:resource="https://saref.etsi.org/saref4ener/NumberRange"/>
    <rdfs:label xml:lang="en">Has Supply Range</rdfs:label>
    <rdfs:domain rdf:resource="https://saref.etsi.org/saref4ener/OperationMode"/>
    <rdfs:comment>The SupplyRange this OperationMode of a Demand Driven Profile can deliver for the CEM to match the DemandRate. The start of the NumberRange is associated with an operation_mode_factor of 0, the end is associated with an operation_mode_factor of 1.</rdfs:comment>
  </owl:ObjectProperty>
  <owl:ObjectProperty rdf:about="https://saref.etsi.org/saref4ener/hasPowerLimitConsumptionMax">
    <rdfs:range rdf:resource="https://saref.etsi.org/core/Measurement"/>
    <rdfs:label xml:lang="en">has power limit consumption Max</rdfs:label>
    <rdfs:domain rdf:resource="https://saref.etsi.org/saref4ener/PowerLimit"/>
    <rdfs:comment xml:lang="en">The relationship between the power limit and the value indicating the max limit consumption.</rdfs:comment>
  </owl:ObjectProperty>
  <owl:ObjectProperty rdf:about="https://saref.etsi.org/saref4ener/hasLowerBoundary">
    <rdfs:range rdf:resource="https://saref.etsi.org/saref4ener/DataPoint"/>
    <rdfs:label xml:lang="en">has lower boundary</rdfs:label>
    <rdfs:domain rdf:resource="https://saref.etsi.org/saref4ener/Incentive"/>
    <rdfs:comment>This property relates an IncentiveTableBoundary to the datapoint describing its lower boundary or starting point at which this boundary becomes active.</rdfs:comment>
  </owl:ObjectProperty>
  <owl:ObjectProperty rdf:about="https://saref.etsi.org/saref4ener/producedBy">
    <rdfs:range>
      <owl:Class>
        <owl:unionOf rdf:parseType="Collection">
          <owl:Class rdf:about="http://xmlns.com/foaf/0.1/Agent"/>
          <rdf:Description rdf:about="https://saref.etsi.org/core/Device"/>
        </owl:unionOf>
      </owl:Class>
    </rdfs:range>
    <rdfs:label xml:lang="en">produced by</rdfs:label>
    <rdfs:comment>A relation between an entity (datapoint, message, timeseries, instruction) that has been produced by a device or other agent.&#xD;
  &#xD;
  In the context of SAREF4ENER this property is intended for s4ener:DataPoint, s4ener:TimeSeries, and the various types of flexibility instructions, FlexOffers and FlexRequests.</rdfs:comment>
  </owl:ObjectProperty>
  <owl:ObjectProperty rdf:about="https://saref.etsi.org/saref4ener/hasDemandRateForecast">
    <rdfs:range rdf:resource="https://saref.etsi.org/saref4ener/TimeSeries"/>
    <rdfs:label xml:lang="en">has average demand rate forecast</rdfs:label>
    <rdfs:domain rdf:resource="https://saref.etsi.org/saref4ener/DemandDrivenProfile"/>
    <rdfs:comment>This property relates a Demand Driven Profile to a TimeSeries object that indicates a forecast of the average demand rate.</rdfs:comment>
  </owl:ObjectProperty>
  <owl:ObjectProperty rdf:about="https://saref.etsi.org/saref4ener/receives">
    <rdfs:label xml:lang="en">receives</rdfs:label>
    <rdfs:comment xml:lang="en">A relationship between a device (e.g., an appliance or a smart meter) and a load control event</rdfs:comment>
  </owl:ObjectProperty>
  <owl:ObjectProperty rdf:about="https://saref.etsi.org/saref4ener/isLimitedWith">
    <rdfs:range rdf:resource="https://saref.etsi.org/saref4ener/FailsafePowerLimit"/>
    <rdfs:label xml:lang="en">is limited with</rdfs:label>
    <rdfs:domain rdf:resource="https://saref.etsi.org/saref4ener/PowerLimitProfile"/>
    <rdfs:comment xml:lang="en">The relationship between device and failsafe power limit</rdfs:comment>
  </owl:ObjectProperty>
  <owl:ObjectProperty rdf:about="https://saref.etsi.org/saref4ener/hasAppliedEventActionConsume">
    <rdfs:label xml:lang="en">has applied event action consume</rdfs:label>
    <rdfs:comment xml:lang="en">A relationship between the state of a load control event consume and the action to be performed as a consequence of this event.</rdfs:comment>
  </owl:ObjectProperty>
  <owl:ObjectProperty rdf:about="https://saref.etsi.org/saref4ener/hasPowerSequenceStatus">
    <rdfs:range rdf:resource="https://saref.etsi.org/saref4ener/PowerSequenceStatus"/>
    <rdfs:label xml:lang="en">has power sequence status</rdfs:label>
    <rdfs:domain rdf:resource="https://saref.etsi.org/saref4ener/PowerSequenceContainer"/>
    <rdfs:comment>This property indicates the current status of this Power Sequence.</rdfs:comment>
  </owl:ObjectProperty>
  <owl:ObjectProperty rdf:about="https://saref.etsi.org/saref4ener/hasPowerSequenceElement">
    <rdfs:range rdf:resource="https://saref.etsi.org/saref4ener/PowerSequenceElement"/>
    <rdfs:label xml:lang="en">has power sequence element</rdfs:label>
    <rdfs:domain rdf:resource="https://saref.etsi.org/saref4ener/PowerSequence"/>
    <rdfs:comment>A connection between the Power Sequence and the elements (or Slots) describing the exact contents.</rdfs:comment>
  </owl:ObjectProperty>
  <owl:ObjectProperty rdf:about="https://saref.etsi.org/saref4ener/relatesToOffer">
    <rdfs:range rdf:resource="https://saref.etsi.org/saref4ener/FlexOffer"/>
    <rdfs:label xml:lang="en">relates to offer</rdfs:label>
    <rdfs:domain rdf:resource="https://saref.etsi.org/saref4ener/FlexibilityInstruction"/>
    <rdfs:comment xml:lang="en">The relationship between the s4ener:FlexibilityInstruction and the flexibility offer.</rdfs:comment>
  </owl:ObjectProperty>
  <owl:ObjectProperty rdf:about="https://saref.etsi.org/saref4ener/hasPowerSource">
    <rdfs:range rdf:resource="https://saref.etsi.org/saref4ener/PowerSource"/>
    <rdfs:label xml:lang="en">Power source</rdfs:label>
    <rdfs:comment xml:lang="en">Indicates the power source of a device. Possible values are e.g. mainsSinglePhase or battery </rdfs:comment>
  </owl:ObjectProperty>
  <owl:ObjectProperty rdf:about="https://saref.etsi.org/saref4ener/hasFillLevelTargetProfileElement">
    <rdfs:range rdf:resource="https://saref.etsi.org/saref4ener/FillLevelTargetProfileElement"/>
    <rdfs:label xml:lang="en">has fill level target profile element</rdfs:label>
    <rdfs:domain rdf:resource="https://saref.etsi.org/saref4ener/FillLevelTargetProfile"/>
    <rdfs:comment>The various Fill Level Target Profile Elements detailing the Fill Level Target Profile that the current Fill Level Based Profile tries to accomodate for.</rdfs:comment>
  </owl:ObjectProperty>
  <owl:ObjectProperty rdf:about="https://saref.etsi.org/saref4ener/limitType">
    <rdfs:range rdf:resource="https://saref.etsi.org/saref4ener/PowerEnvelopeLimitType"/>
    <rdfs:label xml:lang="en">Limit Type</rdfs:label>
    <rdfs:domain rdf:resource="https://saref.etsi.org/saref4ener/AllowedLimitRange"/>
    <rdfs:comment>Indicates if this ranges applies to the upper limit or the lower limit.</rdfs:comment>
  </owl:ObjectProperty>
  <owl:ObjectProperty rdf:about="https://saref.etsi.org/saref4ener/hasRole">
    <rdfs:range rdf:resource="https://saref.etsi.org/saref4ener/Role"/>
    <rdfs:label xml:lang="en">performs role</rdfs:label>
    <rdfs:domain rdf:resource="https://saref.etsi.org/saref4ener/Device"/>
    <rdfs:comment>Each Resource Manager provides one or more energy Roles</rdfs:comment>
  </owl:ObjectProperty>
  <owl:ObjectProperty rdf:about="https://saref.etsi.org/saref4ener/hasMessagingType">
    <rdfs:label xml:lang="en">has messaging type</rdfs:label>
    <rdfs:comment>The messaging type associated with this element.</rdfs:comment>
  </owl:ObjectProperty>
  <owl:ObjectProperty rdf:about="https://saref.etsi.org/saref4ener/belongsTo">
    <rdfs:label xml:lang="en">belongs to</rdfs:label>
    <rdfs:comment xml:lang="en">A relationship identifying the ownership of an entity. In particular, a slot belongs to a power sequence, a power sequence belongs to an alternative, an alternative  belongs to a power profile, a power profile belongs to a device.  </rdfs:comment>
  </owl:ObjectProperty>
  <owl:ObjectProperty rdf:about="https://saref.etsi.org/saref4ener/triggersEventActionConsume">
    <rdfs:label xml:lang="en">triggers event action consume</rdfs:label>
    <rdfs:comment xml:lang="en">A relationship between a load control event and the consume action triggered by this event</rdfs:comment>
  </owl:ObjectProperty>
  <owl:ObjectProperty rdf:about="https://saref.etsi.org/saref4ener/hasPowerSequence">
    <rdfs:range rdf:resource="https://saref.etsi.org/saref4ener/PowerSequence"/>
    <rdfs:label xml:lang="en">has power sequence</rdfs:label>
    <rdfs:domain rdf:resource="https://saref.etsi.org/saref4ener/PowerSequenceContainer"/>
    <rdfs:comment>The various Sequences contained in a Power Sequence Container among which the EMS can choose the proper PowerSequence for the current energy demands.</rdfs:comment>
  </owl:ObjectProperty>
  <owl:ObjectProperty rdf:about="https://saref.etsi.org/saref4ener/relatesToPowerProfile">
    <rdfs:range rdf:resource="https://saref.etsi.org/saref4ener/PowerProfile"/>
    <rdfs:label xml:lang="en">Relates to power profile</rdfs:label>
    <rdfs:domain rdf:resource="https://saref.etsi.org/saref4ener/PPBCInstruction"/>
    <rdfs:comment>ID of the PPBC.PowerProfileDefinition of which the PPBC.PowerSequence is being selected and scheduled by the CEM.</rdfs:comment>
  </owl:ObjectProperty>
  <owl:ObjectProperty rdf:about="https://saref.etsi.org/saref4ener/hasPowerLimitState">
    <rdfs:label xml:lang="en">has power limit state</rdfs:label>
    <rdfs:domain rdf:resource="https://saref.etsi.org/saref4ener/PowerLimit"/>
    <rdfs:comment xml:lang="en">The relationship between the power limit state and its state (active/ inactive).</rdfs:comment>
  </owl:ObjectProperty>
  <owl:ObjectProperty rdf:about="https://saref.etsi.org/saref4ener/hasPowerEnvelopeElement">
    <rdfs:range rdf:resource="https://saref.etsi.org/saref4ener/PowerEnvelope"/>
    <rdfs:label xml:lang="en">has power envelope element</rdfs:label>
    <rdfs:domain rdf:resource="https://saref.etsi.org/saref4ener/PowerEnvelopeProfile"/>
    <rdfs:comment>This property relates a PowerEnvelopeProfile to the various specific PowerEnvelops contained in the profile.</rdfs:comment>
  </owl:ObjectProperty>
  <owl:ObjectProperty rdf:about="https://saref.etsi.org/saref4ener/hasEnvelope">
    <rdfs:range rdf:resource="https://saref.etsi.org/saref4ener/TimeSeries"/>
    <rdfs:label xml:lang="en">has envelope</rdfs:label>
    <rdfs:domain rdf:resource="https://saref.etsi.org/saref4ener/PowerEnvelope"/>
    <rdfs:comment>This property relates a Power Envelope to the Timeseries object that describes the envelope</rdfs:comment>
  </owl:ObjectProperty>
  <owl:ObjectProperty rdf:about="https://saref.etsi.org/saref4ener/hasPowerLimitProductionMax">
    <rdfs:range rdf:resource="https://saref.etsi.org/core/Measurement"/>
    <rdfs:label xml:lang="en">has power limit production Max</rdfs:label>
    <rdfs:domain rdf:resource="https://saref.etsi.org/saref4ener/PowerLimit"/>
    <rdfs:comment xml:lang="en">The relationship between the power limit and the value indicating the max limit production.</rdfs:comment>
  </owl:ObjectProperty>
  <owl:ObjectProperty rdf:about="https://saref.etsi.org/saref4ener/hasPowerEnvelope">
    <rdfs:range rdf:resource="https://saref.etsi.org/saref4ener/PowerEnvelope"/>
    <rdfs:label xml:lang="en">has power envelope</rdfs:label>
    <rdfs:domain>
      <owl:Class>
        <owl:unionOf rdf:parseType="Collection">
          <owl:Class rdf:about="https://saref.etsi.org/saref4ener/PEBCInstruction"/>
          <owl:Class rdf:about="https://saref.etsi.org/saref4ener/PowerEnvelopeProfile"/>
        </owl:unionOf>
      </owl:Class>
    </rdfs:domain>
    <rdfs:comment>The PEBC.PowerEnvelope(s) that should be followed by the Resource Manager. There shall be at least one PEBC.PowerEnvelope, but at most one PEBC.PowerEnvelope for each CommodityQuantity.</rdfs:comment>
  </owl:ObjectProperty>
  <owl:ObjectProperty rdf:about="https://saref.etsi.org/saref4ener/hasUpperBoundary">
    <rdfs:range rdf:resource="https://saref.etsi.org/saref4ener/DataPoint"/>
    <rdfs:label xml:lang="en">has upper boundary</rdfs:label>
    <rdfs:domain rdf:resource="https://saref.etsi.org/saref4ener/Incentive"/>
    <rdfs:comment>This property relates a boundary to its upper boundary or the value at which this incentive becomes inactive. This value is optional, because the upper boundary can be inferred from the lower boundary of the next boundary.</rdfs:comment>
  </owl:ObjectProperty>
  <owl:ObjectProperty rdf:about="https://saref.etsi.org/saref4ener/isProtectedBy">
    <rdfs:range rdf:resource="https://saref.etsi.org/saref4ener/NominalPowerLimit"/>
    <rdfs:label xml:lang="en">is protected by</rdfs:label>
    <rdfs:domain rdf:resource="https://saref.etsi.org/saref4ener/PowerLimitProfile"/>
    <rdfs:comment xml:lang="en">The relationship between the device and the nominal power limit</rdfs:comment>
  </owl:ObjectProperty>
  <owl:ObjectProperty rdf:about="https://saref.etsi.org/saref4ener/leakageRate">
    <rdfs:range rdf:resource="https://saref.etsi.org/core/Measurement"/>
    <rdfs:label xml:lang="en">Leakage Rate</rdfs:label>
    <rdfs:domain rdf:resource="https://saref.etsi.org/saref4ener/LeakageBehaviourElement"/>
    <rdfs:comment>Indicates how fast the momentary fill level will decrease per second due to leakage within the given range of the fill level.</rdfs:comment>
  </owl:ObjectProperty>
  <owl:ObjectProperty rdf:about="https://saref.etsi.org/saref4ener/hasEventStateConsume">
    <rdfs:subPropertyOf rdf:resource="https://saref.etsi.org/core/hasState"/>
    <rdfs:label xml:lang="en">has event state consume</rdfs:label>
    <rdfs:comment xml:lang="en">A relationship between the specification of the state of a load control event consume and the value that this state can assume.</rdfs:comment>
  </owl:ObjectProperty>
  <owl:ObjectProperty rdf:about="https://saref.etsi.org/saref4ener/hasOperationModeElement">
    <rdfs:range rdf:resource="https://saref.etsi.org/saref4ener/OperationModeElement"/>
    <rdfs:label xml:lang="en">Has Operation Mode Element</rdfs:label>
    <rdfs:domain rdf:resource="https://saref.etsi.org/saref4ener/OperationMode"/>
    <rdfs:comment>List of OperationModeElements, which describe the properties of this FRBC.OperationMode depending on the fill_level. The fill_level_ranges of the items in the Array must be contiguous.</rdfs:comment>
  </owl:ObjectProperty>
  <owl:ObjectProperty rdf:about="https://saref.etsi.org/saref4ener/hasEffectivePeriod">
    <rdfs:range rdf:resource="http://www.w3.org/2006/time#Interval"/>
    <rdfs:label xml:lang="en">has effective period</rdfs:label>
    <rdfs:comment>This connects to the temporal entity which describes when (time interval) the quantity of this data point was, is, or will be in effect. This is the time interval which is covered by the forecast.&#xD;
This should be equivalent to the time interval covered by the time-series that express the forecast. *A potential application of SHACL?*</rdfs:comment>
  </owl:ObjectProperty>
  <owl:ObjectProperty rdf:about="https://saref.etsi.org/saref4ener/hasEnergy">
    <rdfs:range rdf:resource="https://saref.etsi.org/saref4ener/Energy"/>
    <rdfs:label xml:lang="en">has energy</rdfs:label>
    <rdfs:comment xml:lang="en">A relationship between a power sequence and its energy (in terms of value and unit of measure)</rdfs:comment>
  </owl:ObjectProperty>
  <owl:ObjectProperty rdf:about="https://saref.etsi.org/saref4ener/hasFunction">
    <owl:deprecated rdf:datatype="http://www.w3.org/2001/XMLSchema#boolean"
    >true</owl:deprecated>
    <rdfs:label xml:lang="en">has function</rdfs:label>
    <rdfs:comment xml:lang="en">A relationship identifying the functions performed by an actuator level and an actuator switch</rdfs:comment>
  </owl:ObjectProperty>
  <owl:ObjectProperty rdf:about="https://saref.etsi.org/saref4ener/hasNominalProduction">
    <rdfs:subPropertyOf rdf:resource="https://saref.etsi.org/saref4ener/hasPowerLimitProductionMax"/>
    <rdfs:range rdf:resource="https://saref.etsi.org/core/Measurement"/>
    <rdfs:label xml:lang="en">has nominal production Max</rdfs:label>
    <rdfs:domain rdf:resource="https://saref.etsi.org/saref4ener/NominalPowerLimit"/>
    <rdfs:comment xml:lang="en">The relationship between the nominal power limit and the value indicating the max limit production.</rdfs:comment>
  </owl:ObjectProperty>
  <owl:ObjectProperty rdf:about="https://saref.etsi.org/saref4ener/hasValueSource">
    <rdfs:range rdf:resource="https://saref.etsi.org/saref4ener/ValueSource"/>
    <rdfs:label xml:lang="en">has value source</rdfs:label>
    <rdfs:comment xml:lang="en">Indicates the source (origin/foundation) of the measurement forecasted values for a power sequence. If absent, the source is undefined. Remark: This element shall express the reliability of the forecast.</rdfs:comment>
  </owl:ObjectProperty>
  <owl:ObjectProperty rdf:about="https://saref.etsi.org/saref4ener/hasPowerRange">
    <rdfs:range rdf:resource="https://saref.etsi.org/saref4ener/PowerRange"/>
    <rdfs:label xml:lang="en">has power ranges</rdfs:label>
    <rdfs:domain>
      <owl:Class>
        <owl:unionOf rdf:parseType="Collection">
          <owl:Class rdf:about="https://saref.etsi.org/saref4ener/OperationMode"/>
          <owl:Class rdf:about="https://saref.etsi.org/saref4ener/OperationModeElement"/>
        </owl:unionOf>
      </owl:Class>
    </rdfs:domain>
    <rdfs:comment>The power produced or consumed by this operation mode. The start of each PowerRange is associated with an operation_mode_factor of 0, the end is associated with an operation_mode_factor of 1. In the array there must be at least one PowerRange, and at most one PowerRange per CommodityQuantity.</rdfs:comment>
  </owl:ObjectProperty>
  <owl:ObjectProperty rdf:about="https://saref.etsi.org/saref4ener/hasPreviousOperationMode">
    <rdfs:range rdf:resource="https://saref.etsi.org/saref4ener/OperationMode"/>
    <rdfs:label xml:lang="en">has previous operation mode</rdfs:label>
    <rdfs:domain>
      <owl:Class>
        <owl:unionOf rdf:parseType="Collection">
          <rdf:Description rdf:about="https://saref.etsi.org/core/Actuator"/>
          <owl:Class rdf:about="https://saref.etsi.org/saref4ener/OperationMode"/>
        </owl:unionOf>
      </owl:Class>
    </rdfs:domain>
    <rdfs:comment>The previous operation mode this device was in</rdfs:comment>
  </owl:ObjectProperty>
  <owl:ObjectProperty rdf:about="https://saref.etsi.org/saref4ener/rangeBoundary">
    <rdfs:range rdf:resource="https://saref.etsi.org/saref4ener/NumberRange"/>
    <rdfs:label xml:lang="en">range boundary</rdfs:label>
    <rdfs:domain>
      <owl:Class>
        <owl:unionOf rdf:parseType="Collection">
          <rdfs:Class rdf:about="https://saref.etsi.org/saref4ener/AllowedLimitRange"/>
          <owl:Class rdf:about="https://saref.etsi.org/saref4ener/EnergyConstraint"/>
        </owl:unionOf>
      </owl:Class>
    </rdfs:domain>
    <rdfs:comment>Boundaries of the power range of this PEBC.AllowedLimitRange. The CEM is allowed to choose values within this range for the power envelope for the limit as described in limit_type. The start of the range shall be smaller or equal than the end of the range.</rdfs:comment>
  </owl:ObjectProperty>
  <owl:ObjectProperty rdf:about="https://saref.etsi.org/saref4ener/presentFillLevel">
    <rdfs:range rdf:resource="https://saref.etsi.org/core/Measurement"/>
    <rdfs:label xml:lang="en">present fill level</rdfs:label>
    <rdfs:domain rdf:resource="https://saref.etsi.org/saref4ener/Storage"/>
    <rdfs:comment>A saref:Measurement with a percentage value indicating the fill level of the storage.</rdfs:comment>
  </owl:ObjectProperty>
  <owl:ObjectProperty rdf:about="https://saref.etsi.org/saref4ener/hasFillLevelTargetProfile">
    <rdfs:range rdf:resource="https://saref.etsi.org/saref4ener/FillLevelTargetProfile"/>
    <rdfs:label xml:lang="en">has fill level target profile</rdfs:label>
    <rdfs:domain rdf:resource="https://saref.etsi.org/saref4ener/Storage"/>
    <rdfs:comment>The Fill Level Target Profile of the storage that the current Fill Rate Profile tries to accomodate for. &#xD;
&#xD;
NB. This cannot be modelled as a TimeSeries, since the x-axis is not time.</rdfs:comment>
  </owl:ObjectProperty>
  <owl:ObjectProperty rdf:about="https://saref.etsi.org/saref4ener/hasOperationMode">
    <rdfs:range rdf:resource="https://saref.etsi.org/saref4ener/OperationMode"/>
    <rdfs:label xml:lang="en">has Operation Modes</rdfs:label>
    <rdfs:comment>This property indicates the s4ener:OperationMode inidicated by this Actuator, Instruction, or OperationModeProfile.&#xD;
&#xD;
The SAREF4ENER extension expects the following classes to be used as domain:&#xD;
- saref:Actuator&#xD;
- s4ener:FRBCInstruction&#xD;
- s4ener:DDBCInstruction&#xD;
- s4ener:OMBCInstruction&#xD;
- s4ener:OperationModeProfile</rdfs:comment>
  </owl:ObjectProperty>
  <owl:ObjectProperty rdf:about="https://saref.etsi.org/saref4ener/relatesToCommodityQuantity">
    <rdfs:range rdf:resource="https://saref.etsi.org/saref4ener/CommodityQuantity"/>
    <rdfs:label xml:lang="en">relates to commodity quantity</rdfs:label>
    <rdfs:comment>Relates the classes to the various commodity quantities introduced by the S2 standard.&#xD;
&#xD;
In the SAREF4ENER extension this property is intended for the following:&#xD;
- s4ener:PowerRange&#xD;
- s4ener:AllowedLimitRange&#xD;
- s4ener:EnergyConstraint&#xD;
- s4ener:PowerEnvelope</rdfs:comment>
  </owl:ObjectProperty>
  <owl:ObjectProperty rdf:about="https://saref.etsi.org/saref4ener/hasConstraints">
    <rdfs:range>
      <owl:Class>
        <owl:unionOf rdf:parseType="Collection">
          <owl:Class rdf:about="https://saref.etsi.org/saref4ener/PowerConstraint"/>
          <owl:Class rdf:about="https://saref.etsi.org/saref4ener/EnergyConstraint"/>
        </owl:unionOf>
      </owl:Class>
    </rdfs:range>
    <rdfs:label xml:lang="en">has constraints</rdfs:label>
    <rdfs:domain>
      <owl:Class>
        <owl:unionOf rdf:parseType="Collection">
          <owl:Class rdf:about="https://saref.etsi.org/saref4ener/PEBCInstruction"/>
          <owl:Class rdf:about="https://saref.etsi.org/saref4ener/PowerEnvelopeProfile"/>
        </owl:unionOf>
      </owl:Class>
    </rdfs:domain>
    <rdfs:comment>This property relates a Power Envelop Instruction or Profile to the constraints it needs to follow. There are two types of constraints modelled: Power constraints and energy constraints.</rdfs:comment>
  </owl:ObjectProperty>
  <owl:ObjectProperty rdf:about="https://saref.etsi.org/saref4ener/relatesToPowerProfileSequenceContainer">
    <rdfs:range rdf:resource="https://saref.etsi.org/saref4ener/PowerSequenceContainer"/>
    <rdfs:label xml:lang="en">Relates to power profile sequence container</rdfs:label>
    <rdfs:domain rdf:resource="https://saref.etsi.org/saref4ener/PPBCInstruction"/>
    <rdfs:comment>ID of the PPBC.PowerSequnceContainer of which the PPBC.PowerSequence is being selected and scheduled by the CEM.</rdfs:comment>
  </owl:ObjectProperty>
  <owl:ObjectProperty rdf:about="https://saref.etsi.org/saref4ener/hasIncentive">
    <rdfs:range rdf:resource="https://saref.etsi.org/saref4ener/Incentive"/>
    <rdfs:label xml:lang="en">has incentive</rdfs:label>
    <rdfs:domain>
      <owl:Class>
        <owl:unionOf rdf:parseType="Collection">
          <owl:Class rdf:about="https://saref.etsi.org/saref4ener/IncentiveTableSlot"/>
          <owl:Class rdf:about="https://saref.etsi.org/saref4ener/IncentiveTableTier"/>
        </owl:unionOf>
      </owl:Class>
    </rdfs:domain>
    <rdfs:comment>This property relates an IncentiveTable element, such as an IncentiveTableSlot or an IncentiveTableTier to the boundaries that it consists of.</rdfs:comment>
  </owl:ObjectProperty>
  <owl:ObjectProperty rdf:about="https://saref.etsi.org/saref4ener/allowedLimitRange">
    <rdfs:range rdf:resource="https://saref.etsi.org/saref4ener/AllowedLimitRange"/>
    <rdfs:label xml:lang="en">allowed limit range</rdfs:label>
    <rdfs:domain>
      <owl:Class>
        <owl:unionOf rdf:parseType="Collection">
          <owl:Class rdf:about="https://saref.etsi.org/saref4ener/PowerConstraint"/>
          <owl:Class rdf:about="https://saref.etsi.org/saref4ener/EnergyConstraint"/>
        </owl:unionOf>
      </owl:Class>
    </rdfs:domain>
    <rdfs:comment>This property indicates the various AllowedLimitRanges or PowerLimits that this PowerConstraint object consists of.</rdfs:comment>
  </owl:ObjectProperty>
  <owl:ObjectProperty rdf:about="https://saref.etsi.org/saref4ener/fromOperationMode">
    <rdfs:range rdf:resource="https://saref.etsi.org/saref4ener/OperationMode"/>
    <rdfs:label xml:lang="en">from operation mode</rdfs:label>
    <rdfs:domain rdf:resource="https://saref.etsi.org/saref4ener/Transition"/>
    <rdfs:comment>ID of the OperationMode (exact type differs per ControlType) that should be switched from.</rdfs:comment>
  </owl:ObjectProperty>
  <owl:ObjectProperty rdf:about="https://saref.etsi.org/saref4ener/hasTier">
    <rdfs:label xml:lang="en">has tier incentive</rdfs:label>
    <rdfs:domain rdf:resource="https://saref.etsi.org/saref4ener/IncentiveTableBasedProfile"/>
    <rdfs:comment xml:lang="en">The relationship between the incentive table and the tiers it consists of</rdfs:comment>
  </owl:ObjectProperty>
  <owl:ObjectProperty rdf:about="https://saref.etsi.org/saref4ener/includes">
    <rdfs:label xml:lang="en">includes</rdfs:label>
    <rdfs:comment xml:lang="en">This property can be used to connect the flexibility offer and/or flexibility request to the flexibility profile. Additionally, it can be used to specify the s4ener:datapoint, s4ener:timeseries and ic-fc:forecast included in the flexibility offer and/or  flexibility request.</rdfs:comment>
  </owl:ObjectProperty>
  <owl:ObjectProperty rdf:about="https://saref.etsi.org/saref4ener/hasLeakageBehaviour">
    <rdfs:range rdf:resource="https://saref.etsi.org/saref4ener/LeakageBehaviour"/>
    <rdfs:label xml:lang="en">has leakage behaviour</rdfs:label>
    <rdfs:domain rdf:resource="https://saref.etsi.org/saref4ener/Storage"/>
    <rdfs:comment>The Leakage Behaviour associated with this storage.</rdfs:comment>
  </owl:ObjectProperty>
  <owl:ObjectProperty rdf:about="https://saref.etsi.org/saref4ener/belongsToTimeSeries">
    <owl:inverseOf rdf:resource="https://saref.etsi.org/saref4ener/hasDataPoint"/>
    <rdfs:range rdf:resource="https://saref.etsi.org/saref4ener/TimeSeries"/>
    <rdfs:label xml:lang="en">belongs to time series</rdfs:label>
    <rdfs:domain rdf:resource="https://saref.etsi.org/saref4ener/DataPoint"/>
    <rdfs:comment xml:lang="en">The relationship that connects a data point to a time series.</rdfs:comment>
  </owl:ObjectProperty>
  <owl:ObjectProperty rdf:about="https://saref.etsi.org/saref4ener/hasUsageForecast">
    <rdfs:range rdf:resource="https://saref.etsi.org/saref4ener/TimeSeries"/>
    <rdfs:label xml:lang="en">Has Usage Forecast</rdfs:label>
    <rdfs:comment>Indicates the usage forecast that may be relevant to decide the energy flexibility strategy following a specific flexibility profile, specifically a fill rate based profile or incentive table.&#xD;
&#xD;
In SAREF4ENER this property is intended to be applied on an s4ener:FlexibilityProfile.</rdfs:comment>
  </owl:ObjectProperty>
  <owl:ObjectProperty rdf:about="https://saref.etsi.org/saref4ener/hasTimer">
    <rdfs:range rdf:resource="https://saref.etsi.org/saref4ener/Timer"/>
    <rdfs:label xml:lang="en">Has Timer</rdfs:label>
    <rdfs:domain>
      <owl:Class>
        <owl:unionOf rdf:parseType="Collection">
          <rdf:Description rdf:about="https://saref.etsi.org/core/Actuator"/>
          <owl:Class rdf:about="https://saref.etsi.org/saref4ener/OperationModeProfile"/>
        </owl:unionOf>
      </owl:Class>
    </rdfs:domain>
    <rdfs:comment>The set of timers that are available in this Actuator or OperationModeProfile</rdfs:comment>
  </owl:ObjectProperty>
  <owl:DatatypeProperty rdf:about="https://saref.etsi.org/saref4ener/hasFailsafeDuration">
    <rdfs:subPropertyOf>
      <owl:DatatypeProperty rdf:about="https://saref.etsi.org/saref4ener/hasDuration"/>
    </rdfs:subPropertyOf>
    <rdfs:range rdf:resource="http://www.w3.org/2001/XMLSchema#duration"/>
    <rdfs:label xml:lang="en">has failsafe duration</rdfs:label>
    <rdfs:domain rdf:resource="https://saref.etsi.org/saref4ener/FailsafeState"/>
    <rdfs:comment xml:lang="en">The relationship between the failsafe power limit and its duration. This property indicates the minimum duration the fail safe state will take once a device has entered that state.</rdfs:comment>
  </owl:DatatypeProperty>
  <owl:DatatypeProperty rdf:about="https://saref.etsi.org/saref4ener/alternativesGroupID">
    <owl:deprecated rdf:datatype="http://www.w3.org/2001/XMLSchema#boolean"
    >true</owl:deprecated>
    <rdfs:range rdf:resource="http://www.w3.org/2001/XMLSchema#integer"/>
    <rdfs:label xml:lang="en">alternatives group ID</rdfs:label>
    <rdfs:comment xml:lang="en">The endpoint-wide unique identifier for the alternatives group instances provided by a power profile</rdfs:comment>
  </owl:DatatypeProperty>
  <owl:DatatypeProperty rdf:about="https://saref.etsi.org/saref4ener/hasTemporalResolution">
    <rdfs:range rdf:resource="http://www.w3.org/2001/XMLSchema#duration"/>
    <rdfs:label xml:lang="en">has temporal resolution</rdfs:label>
    <rdfs:comment>The resolution is the distance between two measurement time-stapms. This only makes sense if the measurements are equidistant.</rdfs:comment>
  </owl:DatatypeProperty>
  <owl:DatatypeProperty rdf:about="https://saref.etsi.org/saref4ener/hasEarliestStartTime">
    <rdfs:subPropertyOf rdf:resource="https://saref.etsi.org/core/hasTimestamp"/>
    <rdfs:range rdf:resource="http://www.w3.org/2001/XMLSchema#dateTimeStamp"/>
    <rdfs:label xml:lang="en">has earliest start time</rdfs:label>
    <rdfs:comment>The earliest possible start time for a power sequence or a slot. Only 'xs:duration' value types SHALL be used to denote a relative time which relates to 'now' as time 0.&#xD;
&#xD;
Note: This element applies to the first repetition of the slot number only.&#xD;
&#xD;
This property is suggested to be added to SAREF4Ener_v2 to replace the time:TemporalEntity and/or time:DurationDescription.</rdfs:comment>
  </owl:DatatypeProperty>
  <owl:DatatypeProperty rdf:about="https://saref.etsi.org/saref4ener/isFinishedAt">
    <rdfs:subPropertyOf rdf:resource="https://saref.etsi.org/core/hasTimestamp"/>
    <rdfs:range rdf:resource="http://www.w3.org/2001/XMLSchema#dateTimeStamp"/>
    <rdfs:label xml:lang="en">is finished at</rdfs:label>
    <rdfs:domain rdf:resource="https://saref.etsi.org/saref4ener/Timer"/>
    <rdfs:comment>Indicates when the Timer will be finished. If the DateTimeStamp is in the future, the timer is not yet finished. If the DateTimeStamp is in the past, the timer is finished. When the timer was never started, the value can be an arbitrary DateTimeStamp in the past.</rdfs:comment>
  </owl:DatatypeProperty>
  <owl:DatatypeProperty rdf:about="https://saref.etsi.org/saref4ener/hasTransitionTimestamp">
    <rdfs:subPropertyOf rdf:resource="https://saref.etsi.org/core/hasTimestamp"/>
    <rdfs:range rdf:resource="http://www.w3.org/2001/XMLSchema#dateTimeStamp"/>
    <rdfs:label xml:lang="en">transition Timestamp</rdfs:label>
    <rdfs:domain>
      <owl:Class>
        <owl:unionOf rdf:parseType="Collection">
          <owl:Class rdf:about="https://saref.etsi.org/saref4ener/OperationMode"/>
          <rdf:Description rdf:about="https://saref.etsi.org/core/Actuator"/>
        </owl:unionOf>
      </owl:Class>
    </rdfs:domain>
    <rdfs:comment>Time at which the transition from the previous Operation Mode was initiated. This value shall always be provided, unless the active OperationMode is the first OperationMode the Resource Manager is aware of.</rdfs:comment>
  </owl:DatatypeProperty>
  <owl:DatatypeProperty rdf:about="https://saref.etsi.org/saref4ener/isChangeable">
    <rdfs:range rdf:resource="http://www.w3.org/2001/XMLSchema#boolean"/>
    <rdfs:label xml:lang="en">is changeable</rdfs:label>
    <rdfs:comment xml:lang="en">A relationship indicating that this element can be changed by its operator. The boolean value indicates whether it is indeed changeable.&#xD;
&#xD;
In the SAREF4ENER extension this property is intended for PowerLimits and IncentiveTable elements, such as the IncentivebasedProfile, IncentiveTableSlot, and the IncentiveTableTier.</rdfs:comment>
  </owl:DatatypeProperty>
  <owl:DatatypeProperty rdf:about="https://saref.etsi.org/saref4ener/hasQuantile">
    <rdfs:range rdf:resource="http://www.w3.org/2001/XMLSchema#decimal"/>
    <rdfs:label xml:lang="en">has quantile</rdfs:label>
    <rdfs:domain rdf:resource="https://saref.etsi.org/saref4ener/DataPoint"/>
    <rdfs:comment xml:lang="en">Used to define a quantile for example on a data point of a quantile time series. The quantile must be a ratio, usually a percentage. In a quantile forecast the hasQuantile property cannot be empty</rdfs:comment>
  </owl:DatatypeProperty>
  <owl:DatatypeProperty rdf:about="https://saref.etsi.org/saref4ener/hasLatestEndTime">
    <rdfs:subPropertyOf rdf:resource="https://saref.etsi.org/core/hasTimestamp"/>
    <rdfs:label xml:lang="en">has latest end time</rdfs:label>
    <rdfs:comment>The latest possible end time for a power sequence or a slot. Only 'xs:duration' value types SHALL be used to denote a relative time which relates to 'now' as time 0.&#xD;
&#xD;
Note: This element applies to the first repetition of the slot number only.&#xD;
&#xD;
This property is suggested to be added to SAREF4Ener_v2 to replace the time:TemporalEntity and/or time:DurationDescription.</rdfs:comment>
  </owl:DatatypeProperty>
  <owl:DatatypeProperty rdf:about="https://saref.etsi.org/saref4ener/hasActiveDurationMin">
    <rdfs:subPropertyOf>
      <owl:DatatypeProperty rdf:about="https://saref.etsi.org/saref4ener/hasDuration"/>
    </rdfs:subPropertyOf>
    <rdfs:range rdf:resource="http://www.w3.org/2001/XMLSchema#duration"/>
    <rdfs:label xml:lang="en">active duration min</rdfs:label>
    <rdfs:comment>The active mininum duration a power sequence can run without interruption.&#xD;
&#xD;
This property is suggested to be added to SAREF4Ener_v2 to replace the time:TemporalEntity and/or time:DurationDescription.</rdfs:comment>
  </owl:DatatypeProperty>
  <owl:DatatypeProperty rdf:about="https://saref.etsi.org/saref4ener/slotNumber">
    <rdfs:range rdf:resource="http://www.w3.org/2001/XMLSchema#unsignedInt"/>
    <rdfs:label xml:lang="en">slot number</rdfs:label>
    <rdfs:comment xml:lang="en">Provides a unique slot identifier for a certain power sequence</rdfs:comment>
  </owl:DatatypeProperty>
  <owl:DatatypeProperty rdf:about="https://saref.etsi.org/saref4ener/activateSlot">
    <rdfs:range rdf:resource="http://www.w3.org/2001/XMLSchema#boolean"/>
    <rdfs:label xml:lang="en">activate slot</rdfs:label>
    <rdfs:comment xml:lang="en">Indicates whether a slot is used (activateSlot = true) or not (activateSlot = false). SHALL be present if a slot is optional (i.e., the property s4ee:optionalSlot is TRUE), otherwise SHALL be absent (i.e. in case the slot is mandatory).</rdfs:comment>
  </owl:DatatypeProperty>
  <owl:DatatypeProperty rdf:about="https://saref.etsi.org/saref4ener/activeRepetitionNumber">
    <rdfs:range rdf:resource="http://www.w3.org/2001/XMLSchema#unsignedInt"/>
    <rdfs:label xml:lang="en">active repetition number</rdfs:label>
    <rdfs:comment xml:lang="en">Indicates the current repetition of the sequence of slots. SHALL be present if a power sequence can repeat its sequence of slots (i.e., if s4ee:repetitionTotal is present and has a value &gt; 1). Otherwise, it SHALL be absent. </rdfs:comment>
  </owl:DatatypeProperty>
  <owl:DatatypeProperty rdf:about="https://saref.etsi.org/saref4ener/hasName">
    <owl:deprecated rdf:datatype="http://www.w3.org/2001/XMLSchema#boolean"
    >true</owl:deprecated>
    <rdfs:range rdf:resource="http://www.w3.org/2001/XMLSchema#string"/>
    <rdfs:label xml:lang="en">Has Name</rdfs:label>
    <rdfs:comment>Human readable name given by user</rdfs:comment>
  </owl:DatatypeProperty>
  <owl:DatatypeProperty rdf:about="https://saref.etsi.org/saref4ener/hasTransitionCosts">
    <rdfs:range rdf:resource="http://www.w3.org/2001/XMLSchema#decimal"/>
    <rdfs:label xml:lang="en">has transition costs</rdfs:label>
    <rdfs:domain rdf:resource="https://saref.etsi.org/saref4ener/Transition"/>
    <rdfs:comment>Absolute costs for going through this Transition in the currency as described in the ResourceManagerDetails.</rdfs:comment>
  </owl:DatatypeProperty>
  <owl:DatatypeProperty rdf:about="https://saref.etsi.org/saref4ener/optionalSlot">
    <rdfs:range rdf:resource="http://www.w3.org/2001/XMLSchema#boolean"/>
    <rdfs:label xml:lang="en">optional slot</rdfs:label>
    <rdfs:comment xml:lang="en">Indicates whether a slot is optional (if set to TRUE). Otherwise, if a slot is mandatory, SHALL be omitted or set to FALSE. Note: This element applies to every repetition of the slot number.</rdfs:comment>
  </owl:DatatypeProperty>
  <owl:DatatypeProperty rdf:about="https://saref.etsi.org/saref4ener/isObligatory">
    <rdfs:range rdf:resource="http://www.w3.org/2001/XMLSchema#boolean"/>
    <rdfs:label xml:lang="en">is obligatory</rdfs:label>
    <rdfs:domain rdf:resource="https://saref.etsi.org/saref4ener/PowerLimit"/>
    <rdfs:comment xml:lang="en">A relationship between the power limit and the boolean value indicating whether the power limit is obligatory</rdfs:comment>
  </owl:DatatypeProperty>
  <owl:DatatypeProperty rdf:about="https://saref.etsi.org/saref4ener/hasDuration">
    <rdfs:range rdf:resource="http://www.w3.org/2001/XMLSchema#duration"/>
    <rdfs:label xml:lang="en">duration in xsd </rdfs:label>
    <rdfs:comment>This property specifies that the componenrt has a duration attribute further specified in the subproperty&#xD;
&#xD;
This property is suggested to be added to SAREF4Ener_v2 to replace the time:TemporalEntity and/or time:DurationDescription.</rdfs:comment>
    <rdfs:comment xml:lang="en">This property is added to the  time:DurationDescription class to allow to express time duration also as xsd:duration. This is necessary because in the EEBus/E@h model time is always expressed as xsd:duration. We use this property to express the following time information in the EEBus/E@h model:&#xD;
&#xD;
- the startTime of the power sequence (in the PowerSequence class). SHALL be present&#xD;
- the endTime of the power sequence (in the PowerSequence class). If the value is available, it SHALL be denoted here. Otherwise the element SHALL be omitted.&#xD;
- the startTime of measurement as absolute or relative value (in the Measurement class).&#xD;
- the endTime of measurement as absolute or relative value (in the Measurement class).&#xD;
&#xD;
The duration is expected to be described as in xsd:duration</rdfs:comment>
  </owl:DatatypeProperty>
  <owl:DatatypeProperty rdf:about="https://saref.etsi.org/saref4ener/hasActiveDurationSumMax">
    <rdfs:subPropertyOf rdf:resource="https://saref.etsi.org/saref4ener/hasDuration"/>
    <rdfs:range rdf:resource="http://www.w3.org/2001/XMLSchema#duration"/>
    <rdfs:label xml:lang="en">active duration sum max</rdfs:label>
    <rdfs:comment>The active maximum duration a power sequence can run in total (summation of all active times).&#xD;
&#xD;
This property is suggested to be added to SAREF4Ener_v2 to replace the time:TemporalEntity and/or time:DurationDescription.</rdfs:comment>
  </owl:DatatypeProperty>
  <owl:DatatypeProperty rdf:about="https://saref.etsi.org/saref4ener/hasCreationTime">
    <rdfs:range rdf:resource="http://www.w3.org/2001/XMLSchema#dateTimeStamp"/>
    <rdfs:label xml:lang="en">has creation time</rdfs:label>
    <rdfs:comment xml:lang="en">The time instant that defines the creation time of a data point or quantity or forecast or similar entities. This is not the same as the time at which the quantity is in effect. For example, if a temperature is forecasted today at 12:30 (creation time of the forecast) for the following day at 14:45 (time when the temperature is expected to be in effect), the this instant should be 12:30 of today.&#xD;
&#xD;
A creation time (instant). This is the point in time when the data point was created, which is not necessarily the time for which it is valid. In the case of soft-sensors or forecasters, a data point might have been created ahead of time, in the case of a direcet measurement a data point might created at its time of validity (or at the end of its validity time interval) and in the case of an archived value the data point might have been created after the fact.</rdfs:comment>
  </owl:DatatypeProperty>
  <owl:DatatypeProperty rdf:about="https://saref.etsi.org/saref4ener/hasDurationMin">
    <rdfs:subPropertyOf rdf:resource="https://saref.etsi.org/saref4ener/hasDuration"/>
    <rdfs:range rdf:resource="http://www.w3.org/2001/XMLSchema#duration"/>
    <rdfs:label xml:lang="en">duration minimum</rdfs:label>
    <rdfs:comment>The minimum duration for some component&#xD;
&#xD;
This property is suggested to be added in SAREF4ENER_V2</rdfs:comment>
  </owl:DatatypeProperty>
  <owl:DatatypeProperty rdf:about="https://saref.etsi.org/saref4ener/deviceCode">
    <rdfs:range rdf:resource="http://www.w3.org/2001/XMLSchema#string"/>
    <rdfs:label xml:lang="en">device code</rdfs:label>
    <rdfs:comment xml:lang="en">Provides a device code for the device as defined by the manufacturer.</rdfs:comment>
  </owl:DatatypeProperty>
  <owl:DatatypeProperty rdf:about="https://saref.etsi.org/saref4ener/repetitionsTotal">
    <rdfs:range rdf:resource="http://www.w3.org/2001/XMLSchema#unsignedInt"/>
    <rdfs:label xml:lang="en">repetition total</rdfs:label>
    <rdfs:comment xml:lang="en">Contains the total number of repetitions, if a power sequence repeats its sequence of slots. Absence of the element is equal to a presence with a value of 0 (zero). SHALL be absent if the value is 1. </rdfs:comment>
  </owl:DatatypeProperty>
  <owl:DatatypeProperty rdf:about="https://saref.etsi.org/saref4ener/supportsReselection">
    <rdfs:range rdf:resource="http://www.w3.org/2001/XMLSchema#boolean"/>
    <rdfs:label xml:lang="en">supports reselection</rdfs:label>
    <rdfs:comment xml:lang="en">If set toTRUE, the power profile of a device does not restrict the number of power sequence re-selections by the CEM, i.e. within a given alternative the CEM may first choose one power sequence, alter the selection by configuring another sequence later on, then alter the selection again, etc. (provided the process rules and data still permit configuration). If supportsReselection is set to FALSE, the device permits the CEM to select a power sequence of an alternative only once.</rdfs:comment>
  </owl:DatatypeProperty>
  <owl:DatatypeProperty rdf:about="https://saref.etsi.org/saref4ener/softwareRevision">
    <rdfs:range rdf:resource="http://www.w3.org/2001/XMLSchema#string"/>
    <rdfs:label xml:lang="en">software revision</rdfs:label>
    <rdfs:comment xml:lang="en">Indicates the software revision of a device as defined by the manufacturer.</rdfs:comment>
  </owl:DatatypeProperty>
  <owl:DatatypeProperty rdf:about="https://saref.etsi.org/saref4ener/hasValue">
    <rdfs:range rdf:resource="http://www.w3.org/2001/XMLSchema#decimal"/>
    <rdfs:label xml:lang="en">has value</rdfs:label>
    <rdfs:comment>Power value expressed in the unit associated with the CommodityQuantity of the Power Value.</rdfs:comment>
  </owl:DatatypeProperty>
  <owl:DatatypeProperty rdf:about="https://saref.etsi.org/saref4ener/hasOperationModeFactor">
    <rdfs:range rdf:resource="http://www.w3.org/2001/XMLSchema#decimal"/>
    <rdfs:label xml:lang="en">Has Operation Mode Factor</rdfs:label>
    <rdfs:comment>The number indicates the factor with which the FRBC.OperationMode or OMBC.OperationMode is usedconfigured. The factor should be greater than or equal than 0 and less or equal to 1.&#xD;
&#xD;
Within the SAREF4ENER extension, this property is to be used on the following classes:&#xD;
- s4ener:OMBCInstruction&#xD;
- s4ener:OperationMode&#xD;
- saref:Actuator&#xD;
- s4ener:FRBCInstruction&#xD;
- s4ener:DDBCInstruction</rdfs:comment>
  </owl:DatatypeProperty>
  <owl:DatatypeProperty rdf:about="https://saref.etsi.org/saref4ener/messagingType">
    <owl:deprecated rdf:datatype="http://www.w3.org/2001/XMLSchema#boolean"
    >true</owl:deprecated>
    <rdfs:range>
      <rdfs:Datatype>
        <owl:oneOf rdf:parseType="Resource">
          <rdf:rest rdf:parseType="Resource">
            <rdf:rest rdf:parseType="Resource">
              <rdf:rest rdf:parseType="Resource">
                <rdf:rest rdf:parseType="Resource">
                  <rdf:rest rdf:parseType="Resource">
                    <rdf:rest rdf:resource="http://www.w3.org/1999/02/22-rdf-syntax-ns#nil"/>
                    <rdf:first>obsolete</rdf:first>
                  </rdf:rest>
                  <rdf:first>emergency</rdf:first>
                </rdf:rest>
                <rdf:first>alarm</rdf:first>
              </rdf:rest>
              <rdf:first>warning</rdf:first>
            </rdf:rest>
            <rdf:first>information</rdf:first>
          </rdf:rest>
          <rdf:first>logging</rdf:first>
        </owl:oneOf>
      </rdfs:Datatype>
    </rdfs:range>
    <rdfs:label xml:lang="en">messaging type</rdfs:label>
    <rdfs:comment xml:lang="en">Indicates the type of the message. Possible values are:&#xD;
-	logging (used for messages, that shall be stored in a log file)&#xD;
-	information (messages, that shall be presented to the customer on a display; lower priority)&#xD;
-	warning (messages, that shall be presented to the customer on a display; medium priority)&#xD;
-	alarm (messages, that shall be presented to the customer on a display; high priority; if there is an alarm device in the household, it shall generate an alarm)&#xD;
-	emergency (messages, that shall be presented to the customer on a display; very high priority; if there is an alarm device in the household, it shall generate an alarm; additionally, if possible and configured, an emergency call shall be done)&#xD;
-	obsolete (previously sent messages, that shall be marked as obsolete)</rdfs:comment>
  </owl:DatatypeProperty>
  <owl:DatatypeProperty rdf:about="https://saref.etsi.org/saref4ener/hardwareRevision">
    <rdfs:range rdf:resource="http://www.w3.org/2001/XMLSchema#string"/>
    <rdfs:label xml:lang="en">hardware revision </rdfs:label>
    <rdfs:comment xml:lang="en">Indicates the hardware revision of the device as defined by the manufacturer.</rdfs:comment>
  </owl:DatatypeProperty>
  <owl:DatatypeProperty rdf:about="https://saref.etsi.org/saref4ener/hasStandardDeviation">
    <rdfs:range rdf:resource="http://www.w3.org/2001/XMLSchema#decimal"/>
    <rdfs:label xml:lang="en">has standard deviation</rdfs:label>
    <rdfs:domain rdf:resource="https://saref.etsi.org/saref4ener/GaussianDataPoint"/>
    <rdfs:comment xml:lang="en">Adds a standard deviation to a data point.</rdfs:comment>
  </owl:DatatypeProperty>
  <owl:DatatypeProperty rdf:about="https://saref.etsi.org/saref4ener/nodeRemoteControllable">
    <rdfs:range rdf:resource="http://www.w3.org/2001/XMLSchema#boolean"/>
    <rdfs:label xml:lang="en">node remote controllable</rdfs:label>
    <rdfs:comment xml:lang="en">Indicates whether the power profile of a device is configured for remote control (e.g., by an energy management system).This refers to the selection chosen by the user on the remote control feature of the device. If nodeRemoteControllable is equal to FALSE, all the supported power sequences shall set the sequenceRemoteControllable property to FALSE. If nodeRemoteControllable is equal to TRUE, at least one power sequence shall be remotely controllable by setting the sequenceRemoteControllable property to TRUE.</rdfs:comment>
  </owl:DatatypeProperty>
  <owl:DatatypeProperty rdf:about="https://saref.etsi.org/saref4ener/abnormalCondition">
    <rdfs:range rdf:resource="http://www.w3.org/2001/XMLSchema#boolean"/>
    <rdfs:label xml:lang="en">abnormal condition</rdfs:label>
    <rdfs:domain rdf:resource="https://saref.etsi.org/saref4ener/FlexibilityInstruction"/>
    <rdfs:comment>Indicates if this is an instruction during an abnormal condition</rdfs:comment>
  </owl:DatatypeProperty>
  <owl:DatatypeProperty rdf:about="https://saref.etsi.org/saref4ener/hasUpdateRate">
    <rdfs:range rdf:resource="http://www.w3.org/2001/XMLSchema#duration"/>
    <rdfs:label xml:lang="en">has update rate</rdfs:label>
    <rdfs:comment xml:lang="en">The rate at which a data point or time-series or forecast or other data entity is being updated.&#xD;
&#xD;
If the time series gets regularly updated, then the time between two updates can be recorded here.</rdfs:comment>
  </owl:DatatypeProperty>
  <owl:DatatypeProperty rdf:about="https://saref.etsi.org/saref4ener/vendorName">
    <rdfs:range rdf:resource="http://www.w3.org/2001/XMLSchema#string"/>
    <rdfs:label xml:lang="en">vendor name</rdfs:label>
    <rdfs:comment xml:lang="en">Provides the name of the vendor of the device as defined by the manufacturer.</rdfs:comment>
  </owl:DatatypeProperty>
  <owl:DatatypeProperty rdf:about="https://saref.etsi.org/saref4ener/hasInterruptionStartTime">
    <rdfs:subPropertyOf rdf:resource="https://saref.etsi.org/core/hasTimestamp"/>
    <rdfs:range rdf:resource="http://www.w3.org/2001/XMLSchema#dateTimeStamp"/>
    <rdfs:label xml:lang="en">Has Interruption Start Time</rdfs:label>
    <rdfs:domain rdf:resource="https://saref.etsi.org/saref4ener/InterruptionInstruction"/>
    <rdfs:comment>The start time included in an Interruption Instruction message indicating when the interruption should start.</rdfs:comment>
  </owl:DatatypeProperty>
  <owl:DatatypeProperty rdf:about="https://saref.etsi.org/saref4ener/cheapest">
    <rdfs:range rdf:resource="http://www.w3.org/2001/XMLSchema#boolean"/>
    <rdfs:label xml:lang="en">cheapest</rdfs:label>
    <rdfs:comment xml:lang="en">Indicates whether a power sequence applies a configuration that minimises the user's energy bill (if set to TRUE). MAY be present. Absence of this element is equal to the presence with value FALSE. </rdfs:comment>
  </owl:DatatypeProperty>
  <owl:DatatypeProperty rdf:about="https://saref.etsi.org/saref4ener/progress">
    <rdfs:range rdf:resource="http://www.w3.org/2001/XMLSchema#duration"/>
    <rdfs:label xml:lang="en">progress</rdfs:label>
    <rdfs:domain rdf:resource="https://saref.etsi.org/saref4ener/PowerSequenceContainer"/>
    <rdfs:comment>Time that has passed since the selected sequence has started. A value must be provided, unless no sequence has been selected or the selected sequence hasn't started yet.</rdfs:comment>
  </owl:DatatypeProperty>
  <owl:DatatypeProperty rdf:about="https://saref.etsi.org/saref4ener/hasPowerLimitDuration">
    <rdfs:subPropertyOf rdf:resource="https://saref.etsi.org/saref4ener/hasDuration"/>
    <rdfs:range rdf:resource="http://www.w3.org/2001/XMLSchema#duration"/>
    <rdfs:label xml:lang="en">has power limit duration</rdfs:label>
    <rdfs:domain rdf:resource="https://saref.etsi.org/saref4ener/PowerLimit"/>
    <rdfs:comment xml:lang="en">The relationship between the power limit and its duration. Power limit may come with a time period of validity based on duration</rdfs:comment>
  </owl:DatatypeProperty>
  <owl:DatatypeProperty rdf:about="https://saref.etsi.org/saref4ener/messagingNumber">
    <owl:deprecated rdf:datatype="http://www.w3.org/2001/XMLSchema#boolean"
    >true</owl:deprecated>
    <rdfs:range rdf:resource="http://www.w3.org/2001/XMLSchema#unsignedInt"/>
    <rdfs:label xml:lang="en">messaging number</rdfs:label>
    <rdfs:comment xml:lang="en">An identifier for one specific message. If a message is marked as obsolete, this number can be used to identify the original message.</rdfs:comment>
  </owl:DatatypeProperty>
  <owl:DatatypeProperty rdf:about="https://saref.etsi.org/saref4ener/hasExecutionTime">
    <rdfs:subPropertyOf rdf:resource="https://saref.etsi.org/core/hasTimestamp"/>
    <rdfs:range rdf:resource="http://www.w3.org/2001/XMLSchema#dateTimeStamp"/>
    <rdfs:label xml:lang="en">has execution time</rdfs:label>
    <rdfs:domain rdf:resource="https://saref.etsi.org/saref4ener/FlexibilityInstruction"/>
    <rdfs:comment>Start time of the instruction</rdfs:comment>
  </owl:DatatypeProperty>
  <owl:DatatypeProperty rdf:about="https://saref.etsi.org/saref4ener/sequenceRemoteControllable">
    <rdfs:range rdf:resource="http://www.w3.org/2001/XMLSchema#boolean"/>
    <rdfs:label xml:lang="en">sequence remote controllable</rdfs:label>
    <rdfs:comment xml:lang="en">Denotes whether a power sequence is modifiable (if value is TRUE) or not (if value is FALSE). Modifiability is required to configure power sequences and slots. It is also required to change a power sequence state.</rdfs:comment>
  </owl:DatatypeProperty>
  <owl:DatatypeProperty rdf:about="https://saref.etsi.org/saref4ener/maxCyclesPerDay">
    <rdfs:range rdf:resource="http://www.w3.org/2001/XMLSchema#unsignedInt"/>
    <rdfs:label xml:lang="en">max cycles per day</rdfs:label>
    <rdfs:comment xml:lang="en">States the maximum amount of starts a power sequence (of a device) allows per day.</rdfs:comment>
  </owl:DatatypeProperty>
  <owl:DatatypeProperty rdf:about="https://saref.etsi.org/saref4ener/taskIdentifier">
    <owl:deprecated rdf:datatype="http://www.w3.org/2001/XMLSchema#boolean"
    >true</owl:deprecated>
    <rdfs:range rdf:resource="http://www.w3.org/2001/XMLSchema#unsignedInt"/>
    <rdfs:label xml:lang="en">task identifier</rdfs:label>
    <rdfs:comment xml:lang="en">Represents the task identifier of the power sequence.</rdfs:comment>
  </owl:DatatypeProperty>
  <owl:DatatypeProperty rdf:about="https://saref.etsi.org/saref4ener/totalSequencesCountMax">
    <rdfs:range rdf:resource="http://www.w3.org/2001/XMLSchema#unsignedInt"/>
    <rdfs:label xml:lang="en">total sequences count max</rdfs:label>
    <rdfs:comment xml:lang="en">Represents the total number of power sequences supported by the power profile of a device</rdfs:comment>
  </owl:DatatypeProperty>
  <owl:DatatypeProperty rdf:about="https://saref.etsi.org/saref4ener/sequenceID">
    <owl:deprecated rdf:datatype="http://www.w3.org/2001/XMLSchema#boolean"
    >true</owl:deprecated>
    <rdfs:range rdf:resource="http://www.w3.org/2001/XMLSchema#unsignedInt"/>
    <rdfs:label xml:lang="en">sequence ID</rdfs:label>
    <rdfs:comment xml:lang="en">Provides a unique power sequence identifier for a certain device</rdfs:comment>
  </owl:DatatypeProperty>
  <owl:DatatypeProperty rdf:about="https://saref.etsi.org/saref4ener/hasEndTime">
    <rdfs:subPropertyOf rdf:resource="https://saref.etsi.org/core/hasTimestamp"/>
    <rdfs:range rdf:resource="http://www.w3.org/2001/XMLSchema#duration"/>
    <rdfs:label xml:lang="en">end time</rdfs:label>
    <rdfs:comment xml:lang="en">The endTime of a power sequence. If the value is available, it SHALL be denoted here. Otherwise the element SHALL be omitted.&#xD;
The end time of a slot MAY be stated in this element. The following equation SHALL apply: endTime - startTime = defaultDuration.</rdfs:comment>
  </owl:DatatypeProperty>
  <owl:DatatypeProperty rdf:about="https://saref.etsi.org/saref4ener/hasActiveDurationMax">
    <rdfs:subPropertyOf rdf:resource="https://saref.etsi.org/saref4ener/hasDuration"/>
    <rdfs:range rdf:resource="http://www.w3.org/2001/XMLSchema#duration"/>
    <rdfs:label xml:lang="en">active duration max</rdfs:label>
    <rdfs:comment>The active maximum duration a power sequence can run without interruption.&#xD;
&#xD;
This property is suggested to be added to SAREF4Ener_v2 to replace the time:TemporalEntity and/or time:DurationDescription.</rdfs:comment>
  </owl:DatatypeProperty>
  <owl:DatatypeProperty rdf:about="https://saref.etsi.org/saref4ener/isInterruptible">
    <rdfs:range rdf:resource="http://www.w3.org/2001/XMLSchema#boolean"/>
    <rdfs:label xml:lang="en">is interruptible</rdfs:label>
    <rdfs:domain rdf:resource="https://saref.etsi.org/saref4ener/PowerSequence"/>
    <rdfs:comment>This property indicates whether the PowerSequence is interruptible.</rdfs:comment>
  </owl:DatatypeProperty>
  <owl:DatatypeProperty rdf:about="https://saref.etsi.org/saref4ener/manufacturerNodeIdentification">
    <owl:deprecated rdf:datatype="http://www.w3.org/2001/XMLSchema#boolean"
    >true</owl:deprecated>
    <rdfs:range rdf:resource="http://www.w3.org/2001/XMLSchema#string"/>
    <rdfs:label xml:lang="en">manufacturer node identification</rdfs:label>
    <rdfs:comment xml:lang="en">Indicates a node identification for the device as defined by the manufacturer. This could be used for the identification of a device, even if it was removed from the network and rejoined later with changed node address.</rdfs:comment>
  </owl:DatatypeProperty>
  <owl:DatatypeProperty rdf:about="https://saref.etsi.org/saref4ener/serialNumber">
    <rdfs:range rdf:resource="http://www.w3.org/2001/XMLSchema#string"/>
    <rdfs:label xml:lang="en">serial number</rdfs:label>
    <rdfs:comment xml:lang="en">Indicates the serial number of a device as defined by the manufacturer. Usually the same as printed on the case.</rdfs:comment>
  </owl:DatatypeProperty>
  <owl:DatatypeProperty rdf:about="https://saref.etsi.org/saref4ener/hasDurationDefault">
    <rdfs:subPropertyOf rdf:resource="https://saref.etsi.org/saref4ener/hasDuration"/>
    <rdfs:range rdf:resource="http://www.w3.org/2001/XMLSchema#duration"/>
    <rdfs:label xml:lang="en">duration default</rdfs:label>
    <rdfs:comment>The duration of a slot (SHALL be present in case of 'determined slot'). If a slot has a configurable lenght, this element SHALL reflect the currently configured lenght&#xD;
&#xD;
This property is suggested to be added to SAREF4Ener_v2 to replace the time:TemporalEntity and/or time:DurationDescription.</rdfs:comment>
  </owl:DatatypeProperty>
  <owl:DatatypeProperty rdf:about="https://saref.etsi.org/saref4ener/hasActiveDurationSumMin">
    <rdfs:subPropertyOf rdf:resource="https://saref.etsi.org/saref4ener/hasDuration"/>
    <rdfs:range rdf:resource="http://www.w3.org/2001/XMLSchema#duration"/>
    <rdfs:label xml:lang="en">active duration sum min</rdfs:label>
    <rdfs:comment>The active minimum duration a power sequence must run in total (summation of all active times).&#xD;
&#xD;
This property is suggested to be added to SAREF4Ener_v2 to replace the time:TemporalEntity and/or time:DurationDescription.</rdfs:comment>
  </owl:DatatypeProperty>
  <owl:DatatypeProperty rdf:about="https://saref.etsi.org/saref4ener/measurementID">
    <owl:deprecated rdf:datatype="http://www.w3.org/2001/XMLSchema#boolean"
    >true</owl:deprecated>
    <rdfs:range rdf:resource="http://www.w3.org/2001/XMLSchema#unsignedInt"/>
    <rdfs:label xml:lang="en">measurement id</rdfs:label>
    <rdfs:comment xml:lang="en">Enables the identification of different sensors on one EEBus address.</rdfs:comment>
  </owl:DatatypeProperty>
  <owl:DatatypeProperty rdf:about="https://saref.etsi.org/saref4ener/hasMaxPauseBefore">
    <rdfs:subPropertyOf rdf:resource="https://saref.etsi.org/saref4ener/hasDuration"/>
    <rdfs:range rdf:resource="http://www.w3.org/2001/XMLSchema#duration"/>
    <rdfs:label xml:lang="en">max pause before</rdfs:label>
    <rdfs:domain rdf:resource="https://saref.etsi.org/saref4ener/PowerSequence"/>
    <rdfs:comment>The maximum duration for which a device can be paused between the end of the previous running sequence and the start of this one</rdfs:comment>
  </owl:DatatypeProperty>
  <owl:DatatypeProperty rdf:about="https://saref.etsi.org/saref4ener/isPausable">
    <rdfs:range rdf:resource="http://www.w3.org/2001/XMLSchema#boolean"/>
    <rdfs:label xml:lang="en">is pausable</rdfs:label>
    <rdfs:comment xml:lang="en">Specifies if the power sequence is pausable.</rdfs:comment>
  </owl:DatatypeProperty>
  <owl:DatatypeProperty rdf:about="https://saref.etsi.org/saref4ener/activeSlotNumber">
    <rdfs:range rdf:resource="http://www.w3.org/2001/XMLSchema#unsignedInt"/>
    <rdfs:label xml:lang="en">active slot number</rdfs:label>
    <rdfs:comment xml:lang="en">Indicates the currently active slot number, if the power sequence state is set to 'running' or 'paused'. Otherwise it SHALL be omitted.</rdfs:comment>
  </owl:DatatypeProperty>
  <owl:DatatypeProperty rdf:about="https://saref.etsi.org/saref4ener/supportsSingleSlotSchedulingOnly">
    <rdfs:range rdf:resource="http://www.w3.org/2001/XMLSchema#boolean"/>
    <rdfs:label xml:lang="en">supports single slot scheduling only</rdfs:label>
    <rdfs:comment xml:lang="en">If set toTRUE, the power profile of a device does NOT permit the modification of more than one slot per configuration command.</rdfs:comment>
  </owl:DatatypeProperty>
  <owl:DatatypeProperty rdf:about="https://saref.etsi.org/saref4ener/firmwareVersion">
    <rdfs:range rdf:resource="http://www.w3.org/2001/XMLSchema#string"/>
    <rdfs:label xml:lang="en">has firmware version</rdfs:label>
    <rdfs:domain rdf:resource="https://saref.etsi.org/saref4ener/Device"/>
    <rdfs:comment>Version identifier of the firmware used in the device (provided by the manufacturer)</rdfs:comment>
  </owl:DatatypeProperty>
  <owl:DatatypeProperty rdf:about="https://saref.etsi.org/saref4ener/brandName">
    <rdfs:range rdf:resource="http://www.w3.org/2001/XMLSchema#string"/>
    <rdfs:label xml:lang="en">brand name</rdfs:label>
    <rdfs:comment xml:lang="en">Provides the name of the brand of a device. Useful where the name of the brand and the vendor differs.</rdfs:comment>
  </owl:DatatypeProperty>
  <owl:DatatypeProperty rdf:about="https://saref.etsi.org/saref4ener/alternativesCount">
    <owl:deprecated rdf:datatype="http://www.w3.org/2001/XMLSchema#boolean"
    >true</owl:deprecated>
    <rdfs:range rdf:resource="http://www.w3.org/2001/XMLSchema#integer"/>
    <rdfs:label xml:lang="en">alternatives count</rdfs:label>
    <rdfs:comment xml:lang="en">Indicates the number of alternatives groups provided by a power profile</rdfs:comment>
  </owl:DatatypeProperty>
  <owl:DatatypeProperty rdf:about="https://saref.etsi.org/saref4ener/abnormalConditionOnly">
    <rdfs:range rdf:resource="http://www.w3.org/2001/XMLSchema#boolean"/>
    <rdfs:label xml:lang="en">Abnormal Condition Only</rdfs:label>
    <rdfs:comment>Indicates if this element can only be used during an abnormal condition.&#xD;
&#xD;
In SAREF4ENER this property is intended to be used on the following properties:&#xD;
- s4ener:OperationMode&#xD;
- s4ener:Transition&#xD;
- s4ener:AllowedLimitRange&#xD;
- s4ener:PowerSequence</rdfs:comment>
  </owl:DatatypeProperty>
  <owl:DatatypeProperty rdf:about="https://saref.etsi.org/saref4ener/hasTransitionDuration">
    <rdfs:subPropertyOf rdf:resource="https://saref.etsi.org/saref4ener/hasDuration"/>
    <rdfs:range rdf:resource="http://www.w3.org/2001/XMLSchema#duration"/>
    <rdfs:label xml:lang="en">Transition Duration</rdfs:label>
    <rdfs:domain rdf:resource="https://saref.etsi.org/saref4ener/Transition"/>
    <rdfs:comment>Indicates the time between the initiation of this Transition, and the time at which the device behaves according to the Operation Mode which is defined in the appropriate data element. When no value is provided it is assumed the transition duration is negligible.</rdfs:comment>
  </owl:DatatypeProperty>
  <owl:DatatypeProperty rdf:about="https://saref.etsi.org/saref4ener/slotActivated">
    <rdfs:range rdf:resource="http://www.w3.org/2001/XMLSchema#boolean"/>
    <rdfs:label xml:lang="en">slot activated</rdfs:label>
    <rdfs:comment xml:lang="en">If a slot is optional, represents the current status of the slot (true = the slot will be executed, false = the slot will not be executed). If the slot is not optional, this element SHALL be absent.</rdfs:comment>
  </owl:DatatypeProperty>
  <owl:DatatypeProperty rdf:about="https://saref.etsi.org/saref4ener/hasStartTime">
    <rdfs:subPropertyOf rdf:resource="https://saref.etsi.org/core/hasTimestamp"/>
    <rdfs:range rdf:resource="http://www.w3.org/2001/XMLSchema#dateTimeStamp"/>
    <rdfs:label xml:lang="en">has start time</rdfs:label>
    <rdfs:comment xml:lang="en">The startTime of a power sequence or slot. SHALL be present</rdfs:comment>
  </owl:DatatypeProperty>
  <owl:DatatypeProperty rdf:about="https://saref.etsi.org/saref4ener/eventID">
    <owl:deprecated rdf:datatype="http://www.w3.org/2001/XMLSchema#boolean"
    >true</owl:deprecated>
    <rdfs:range rdf:resource="http://www.w3.org/2001/XMLSchema#unsignedInt"/>
    <rdfs:label xml:lang="en">event ID</rdfs:label>
    <rdfs:comment xml:lang="en">Used in the Demand Response use case to identify an event</rdfs:comment>
  </owl:DatatypeProperty>
  <owl:DatatypeProperty rdf:about="https://saref.etsi.org/saref4ener/hasLowerAveragePower">
    <rdfs:range rdf:resource="http://www.w3.org/2001/XMLSchema#integer"/>
    <rdfs:label xml:lang="en">has lower average power</rdfs:label>
    <rdfs:domain rdf:resource="https://saref.etsi.org/saref4ener/EnergyConstraint"/>
    <rdfs:comment>The lower average power associated with this Energy constraint.</rdfs:comment>
  </owl:DatatypeProperty>
  <owl:DatatypeProperty rdf:about="https://saref.etsi.org/saref4ener/manufacturerDescription">
    <owl:deprecated rdf:datatype="http://www.w3.org/2001/XMLSchema#boolean"
    >true</owl:deprecated>
    <rdfs:range rdf:resource="http://www.w3.org/2001/XMLSchema#string"/>
    <rdfs:label xml:lang="en">manufacturer description</rdfs:label>
    <rdfs:comment xml:lang="en">A description for the device as defined by the manufacturer.</rdfs:comment>
  </owl:DatatypeProperty>
  <owl:DatatypeProperty rdf:about="https://saref.etsi.org/saref4ener/hasActivationDelay">
    <rdfs:subPropertyOf rdf:resource="https://saref.etsi.org/saref4ener/hasDuration"/>
    <rdfs:range rdf:resource="http://www.w3.org/2001/XMLSchema#duration"/>
    <rdfs:label xml:lang="en">delay</rdfs:label>
    <rdfs:comment>The scheduled activation delay for a slot.&#xD;
&#xD;
This property is suggested to be added in SAREF4Ener_v2 to replace the subclasses of time:TemporalEntity and/or time:DurationDescription</rdfs:comment>
  </owl:DatatypeProperty>
  <owl:DatatypeProperty rdf:about="https://saref.etsi.org/saref4ener/vendorCode">
    <rdfs:range rdf:resource="http://www.w3.org/2001/XMLSchema#string"/>
    <rdfs:label xml:lang="en">vendor code</rdfs:label>
    <rdfs:comment xml:lang="en">Provides a code for the vendor of the device as defined by the manufacturer.</rdfs:comment>
  </owl:DatatypeProperty>
  <owl:DatatypeProperty rdf:about="https://saref.etsi.org/saref4ener/hasUpperAveragePower">
    <rdfs:range rdf:resource="http://www.w3.org/2001/XMLSchema#integer"/>
    <rdfs:label xml:lang="en">has upper average power</rdfs:label>
    <rdfs:domain rdf:resource="https://saref.etsi.org/saref4ener/EnergyConstraint"/>
    <rdfs:comment>The upper average power of an Energy constraint of a Power Envelope profile.</rdfs:comment>
  </owl:DatatypeProperty>
  <owl:DatatypeProperty rdf:about="https://saref.etsi.org/saref4ener/hasIndex">
    <rdfs:range rdf:resource="http://www.w3.org/2001/XMLSchema#integer"/>
    <rdfs:label xml:lang="en">has index</rdfs:label>
    <rdfs:comment>Gives the index for elements that are an array in the S2 specification. Can be used regularly as well as in RDF* manner on properties.</rdfs:comment>
  </owl:DatatypeProperty>
  <owl:DatatypeProperty rdf:about="https://saref.etsi.org/saref4ener/manufacturerLabel">
    <owl:deprecated rdf:datatype="http://www.w3.org/2001/XMLSchema#boolean"
    >true</owl:deprecated>
    <rdfs:range rdf:resource="http://www.w3.org/2001/XMLSchema#string"/>
    <rdfs:label xml:lang="en">manufacturer label</rdfs:label>
    <rdfs:comment xml:lang="en">A short label of the device as defined by the manufacturer. </rdfs:comment>
  </owl:DatatypeProperty>
  <owl:DatatypeProperty rdf:about="https://saref.etsi.org/saref4ener/isStoppable">
    <rdfs:range rdf:resource="http://www.w3.org/2001/XMLSchema#boolean"/>
    <rdfs:label xml:lang="en">is stoppable</rdfs:label>
    <rdfs:comment xml:lang="en">Specifies if the power sequence is stoppable.</rdfs:comment>
  </owl:DatatypeProperty>
  <owl:DatatypeProperty rdf:about="https://saref.etsi.org/saref4ener/isActive">
    <rdfs:range rdf:resource="http://www.w3.org/2001/XMLSchema#boolean"/>
    <rdfs:label xml:lang="en">is active</rdfs:label>
    <rdfs:domain rdf:resource="https://saref.etsi.org/saref4ener/PowerLimit"/>
    <rdfs:comment>Indicates whether the power limit is currently active</rdfs:comment>
  </owl:DatatypeProperty>
  <owl:DatatypeProperty rdf:about="https://saref.etsi.org/saref4ener/deviceName">
    <rdfs:range rdf:resource="http://www.w3.org/2001/XMLSchema#string"/>
    <rdfs:label xml:lang="en">device name</rdfs:label>
    <rdfs:comment xml:lang="en">Provides the name of the device as defined by the manufacturer.</rdfs:comment>
  </owl:DatatypeProperty>
  <owl:DatatypeProperty rdf:about="https://saref.etsi.org/saref4ener/hasMaxPauseDuration">
    <rdfs:subPropertyOf rdf:resource="https://saref.etsi.org/saref4ener/hasDuration"/>
    <rdfs:range rdf:resource="http://www.w3.org/2001/XMLSchema#duration"/>
    <rdfs:label xml:lang="en">Pause before Maximum</rdfs:label>
    <rdfs:domain rdf:resource="https://saref.etsi.org/saref4ener/PowerSequence"/>
    <rdfs:comment>The maximum duration for which a device can be paused between the end of the previous running sequence and the start of this one</rdfs:comment>
  </owl:DatatypeProperty>
  <owl:DatatypeProperty rdf:about="https://saref.etsi.org/saref4ener/hasInterruptionEndTime">
    <rdfs:subPropertyOf rdf:resource="https://saref.etsi.org/core/hasTimestamp"/>
    <rdfs:range rdf:resource="http://www.w3.org/2001/XMLSchema#dateTimeStamp"/>
    <rdfs:label xml:lang="en">has end time Interruption</rdfs:label>
    <rdfs:domain rdf:resource="https://saref.etsi.org/saref4ener/InterruptionInstruction"/>
    <rdfs:comment>The end time included in an Interruption Instruction message indicating when the interruption should end.</rdfs:comment>
  </owl:DatatypeProperty>
  <owl:DatatypeProperty rdf:about="https://saref.etsi.org/saref4ener/greenest">
    <rdfs:range rdf:resource="http://www.w3.org/2001/XMLSchema#boolean"/>
    <rdfs:label xml:lang="en">greenest</rdfs:label>
    <rdfs:comment xml:lang="en">Indicates whether a power sequence optimises the configuration towards the maximum availability of renewable energy (if set to TRUE). MAY be present. Absence of this element is equal to the presence with value FALSE. </rdfs:comment>
  </owl:DatatypeProperty>
  <owl:DatatypeProperty rdf:about="https://saref.etsi.org/saref4ener/requiresUpdate">
    <rdfs:range rdf:resource="http://www.w3.org/2001/XMLSchema#boolean"/>
    <rdfs:label xml:lang="en">requiresUpdate</rdfs:label>
    <rdfs:comment xml:lang="en">The relationship between the incentive table element and the boolean data indicating whether the incentive table requires an update.&#xD;
&#xD;
In the SAREF4ENER extension this property is intended for the following classes:&#xD;
- IncentiveTableBasedProfile&#xD;
- IncentiveTableTier&#xD;
- IncentiveTableSlot</rdfs:comment>
  </owl:DatatypeProperty>
  <owl:DatatypeProperty rdf:about="https://saref.etsi.org/saref4ener/hasActivationDelayMax">
    <rdfs:subPropertyOf rdf:resource="https://saref.etsi.org/saref4ener/hasDuration"/>
    <rdfs:range rdf:resource="http://www.w3.org/2001/XMLSchema#duration"/>
    <rdfs:label xml:lang="en">activation delay max</rdfs:label>
    <rdfs:comment>Maximum delay time between the end of the previous slot and the beginning of the current slot.&#xD;
&#xD;
This property is suggested to be added to SAREF4Ener_v2 to replace the time:TemporalEntity and/or time:DurationDescription.</rdfs:comment>
  </owl:DatatypeProperty>
  <s4ener:PowerSequenceState rdf:about="https://saref.etsi.org/saref4ener/Scheduled">
    <rdfs:label xml:lang="en">Scheduled</rdfs:label>
    <rdfs:comment xml:lang="en">Power sequence state with value 'scheduled'</rdfs:comment>
    <rdf:type rdf:resource="http://www.w3.org/2002/07/owl#NamedIndividual"/>
  </s4ener:PowerSequenceState>
  <s4ener:IncentiveType rdf:about="https://saref.etsi.org/saref4ener/RelativeCost">
    <rdfs:label xml:lang="en">Relative cost</rdfs:label>
    <rdfs:comment xml:lang="en">The incentive type ''relative cost'' defined in the incentive table.</rdfs:comment>
    <rdf:type rdf:resource="http://www.w3.org/2002/07/owl#NamedIndividual"/>
  </s4ener:IncentiveType>
  <s4ener:InstructionStatus rdf:about="https://saref.etsi.org/saref4ener/Succeeded">
    <rdfs:label xml:lang="en">Succeeded</rdfs:label>
    <rdfs:comment>Instruction finished successfully</rdfs:comment>
    <rdf:type rdf:resource="http://www.w3.org/2002/07/owl#NamedIndividual"/>
  </s4ener:InstructionStatus>
  <s4ener:PowerSequenceState rdf:about="https://saref.etsi.org/saref4ener/Pending">
    <rdfs:label xml:lang="en">Pending</rdfs:label>
    <rdfs:comment xml:lang="en">Power sequence state with value 'pending'</rdfs:comment>
    <rdf:type rdf:resource="http://www.w3.org/2002/07/owl#NamedIndividual"/>
  </s4ener:PowerSequenceState>
  <s4ener:PowerSequenceState rdf:about="https://saref.etsi.org/saref4ener/ScheduledPaused">
    <rdfs:label xml:lang="en">Scheduled paused</rdfs:label>
    <rdfs:comment xml:lang="en">Power sequence state with value 'scheduled paused'</rdfs:comment>
    <rdf:type rdf:resource="http://www.w3.org/2002/07/owl#NamedIndividual"/>
  </s4ener:PowerSequenceState>
  <s4ener:Usage rdf:about="https://saref.etsi.org/saref4ener/Downflex">
    <rdfs:label xml:lang="en">Downflex</rdfs:label>
    <rdfs:comment>This datapoint indicates the down flexibility.</rdfs:comment>
    <rdf:type rdf:resource="http://www.w3.org/2002/07/owl#NamedIndividual"/>
  </s4ener:Usage>
  <s4ener:CommodityQuantity rdf:about="https://saref.etsi.org/saref4ener/NaturalGasFlowRate">
    <rdfs:label xml:lang="en">Natural Gas Flow Rate</rdfs:label>
    <rdfs:comment>Gas flow rate described in liters per second</rdfs:comment>
  </s4ener:CommodityQuantity>
  <owl:AnnotationProperty rdf:about="http://purl.org/vocab/vann/preferredNamespaceUri"/>
  <s4ener:PowerSource rdf:about="https://saref.etsi.org/saref4ener/DCPowerSource">
    <rdfs:label xml:lang="en">DC Power source</rdfs:label>
    <rdfs:comment>This Power Source codelist element indicates that the type of power source is DC.</rdfs:comment>
  </s4ener:PowerSource>
  <s4ener:PowerSequenceState rdf:about="https://saref.etsi.org/saref4ener/Paused">
    <rdfs:label xml:lang="en">Paused</rdfs:label>
    <rdfs:comment xml:lang="en">Power sequence state or sensor state with value 'paused'</rdfs:comment>
    <rdf:type rdf:resource="http://www.w3.org/2002/07/owl#NamedIndividual"/>
  </s4ener:PowerSequenceState>
  <s4ener:ValueSource rdf:about="https://saref.etsi.org/saref4ener/Calculated">
    <rdfs:label xml:lang="en">Calculated</rdfs:label>
    <rdfs:comment>This value source codelist element indicates that this measurement has been calculated instead of measured or empirical.</rdfs:comment>
  </s4ener:ValueSource>
  <s4ener:CommodityQuantity rdf:about="https://saref.etsi.org/saref4ener/HeatTemperature">
    <rdfs:label xml:lang="en">Heat Temperature</rdfs:label>
    <rdfs:comment>Heat described in degrees Celsius</rdfs:comment>
  </s4ener:CommodityQuantity>
  <saref:UnitOfMeasure rdf:about="https://saref.etsi.org/saref4ener/EuroPerKilowattHour">
    <rdfs:label xml:lang="en">Euro per kilo watt hour</rdfs:label>
    <rdfs:comment>Unit of Measure to represent euro's per kilowatt per hour</rdfs:comment>
  </saref:UnitOfMeasure>
  <s4ener:IncentiveType rdf:about="https://saref.etsi.org/saref4ener/CO2Emission">
    <rdfs:label xml:lang="en">CO2 Emission</rdfs:label>
    <rdfs:comment xml:lang="en">The incentive type ''CO2 Emission'' defined in the incentive table.</rdfs:comment>
    <rdf:type rdf:resource="http://www.w3.org/2002/07/owl#NamedIndividual"/>
  </s4ener:IncentiveType>
  <s4ener:Usage rdf:about="https://saref.etsi.org/saref4ener/SetPoint">
    <rdfs:label xml:lang="en">Setpoint</rdfs:label>
    <rdfs:comment>This datapoint indicates a setpoint.</rdfs:comment>
    <rdf:type rdf:resource="http://www.w3.org/2002/07/owl#NamedIndividual"/>
  </s4ener:Usage>
  <owl:AnnotationProperty rdf:about="http://purl.org/vocab/vann/preferredNamespacePrefix"/>
  <owl:AnnotationProperty rdf:about="http://purl.org/dc/terms/contributor"/>
  <s4ener:CommodityQuantity rdf:about="https://saref.etsi.org/saref4ener/HeatFlowRate">
    <rdfs:label xml:lang="en">Heat Flow Rate</rdfs:label>
    <rdfs:comment>Flow rate of heat carrying gas or liquid in liters per second</rdfs:comment>
  </s4ener:CommodityQuantity>
  <s4ener:CommodityQuantity rdf:about="https://saref.etsi.org/saref4ener/ElectricPowerL2">
    <rdfs:label xml:lang="en">Electric Power L2</rdfs:label>
    <rdfs:comment>Electric power described in Watt on phase 2. Only applicable for 3 phase devices.</rdfs:comment>
  </s4ener:CommodityQuantity>
  <s4ener:ValueSource rdf:about="https://saref.etsi.org/saref4ener/Empirical">
    <rdfs:label xml:lang="en">Empirical</rdfs:label>
    <rdfs:comment>This value source codelist element indicates this value is an empirical value instead of a calculated or measured value.</rdfs:comment>
  </s4ener:ValueSource>
  <s4ener:Usage rdf:about="https://saref.etsi.org/saref4ener/Upflex">
    <rdfs:label xml:lang="en">Upflex</rdfs:label>
    <rdfs:comment>This datapoint indicates the upper flexibility.</rdfs:comment>
    <rdf:type rdf:resource="http://www.w3.org/2002/07/owl#NamedIndividual"/>
  </s4ener:Usage>
  <s4ener:CommodityQuantity rdf:about="https://saref.etsi.org/saref4ener/ElectricPowerL3">
    <rdfs:label xml:lang="en">Electric Power L3</rdfs:label>
    <rdfs:comment>Electric power described in Watt on phase 3. Only applicable for 3 phase devices.</rdfs:comment>
  </s4ener:CommodityQuantity>
  <s4ener:InstructionStatus rdf:about="https://saref.etsi.org/saref4ener/New">
    <rdfs:label xml:lang="en">New</rdfs:label>
    <rdfs:comment>Instruction was newly created</rdfs:comment>
    <rdf:type rdf:resource="http://www.w3.org/2002/07/owl#NamedIndividual"/>
  </s4ener:InstructionStatus>
  <s4ener:ValueTendency rdf:about="https://saref.etsi.org/saref4ener/Rising">
    <rdfs:label xml:lang="en">Rising</rdfs:label>
    <rdfs:comment>This value tendency codelist element indicates that the tendency of this measurement indicates that the value is increasing (i.e., rising).</rdfs:comment>
  </s4ener:ValueTendency>
  <s4ener:PowerSource rdf:about="https://saref.etsi.org/saref4ener/Mains3Phase">
    <rdfs:label xml:lang="en">Mains3Phase</rdfs:label>
    <rdfs:comment>This Power Source codelist element indicates that the power source of this device is Mains 3 Phase.</rdfs:comment>
  </s4ener:PowerSource>
  <s4ener:IncentiveType rdf:about="https://saref.etsi.org/saref4ener/AbsoluteCost">
    <rdfs:label xml:lang="en">Absolute cost</rdfs:label>
    <rdfs:comment xml:lang="en">The incentive type ''absolute cost''  defined in the incentive table.</rdfs:comment>
    <rdf:type rdf:resource="http://www.w3.org/2002/07/owl#NamedIndividual"/>
  </s4ener:IncentiveType>
  <s4ener:PowerSequenceStatus rdf:about="https://saref.etsi.org/saref4ener/Executing">
    <rdfs:label xml:lang="en">EXECUTING</rdfs:label>
    <rdfs:comment>The selected PPBC.PowerSequence is currently being executed</rdfs:comment>
  </s4ener:PowerSequenceStatus>
  <s4ener:CommodityQuantity rdf:about="https://saref.etsi.org/saref4ener/HeatThermalPower">
    <rdfs:label xml:lang="en">Heat Thermal Power</rdfs:label>
    <rdfs:comment>Thermal power in Watt</rdfs:comment>
  </s4ener:CommodityQuantity>
  <s4ener:Usage rdf:about="https://saref.etsi.org/saref4ener/Minimum">
    <rdfs:label xml:lang="en">Minimum</rdfs:label>
    <rdfs:comment>The usage of this datapoint is the Minimum value.</rdfs:comment>
    <rdf:type rdf:resource="http://www.w3.org/2002/07/owl#NamedIndividual"/>
  </s4ener:Usage>
  <s4ener:CommodityQuantity rdf:about="https://saref.etsi.org/saref4ener/OilFlowRate">
    <rdfs:label xml:lang="en">Oil Flow Rate</rdfs:label>
    <rdfs:comment>Oil flow rate described in liters per hour</rdfs:comment>
  </s4ener:CommodityQuantity>
  <s4ener:RoleType rdf:about="https://saref.etsi.org/saref4ener/EnergyProducer">
    <rdfs:label xml:lang="en">Energy Producer</rdfs:label>
    <rdfs:comment>Identifier for RoleType Producer</rdfs:comment>
    <rdf:type rdf:resource="http://www.w3.org/2002/07/owl#NamedIndividual"/>
  </s4ener:RoleType>
  <s4ener:Usage rdf:about="https://saref.etsi.org/saref4ener/Consumption">
    <rdfs:label xml:lang="en">Consumption</rdfs:label>
    <rdfs:comment>This datapoint indicates the consumption.</rdfs:comment>
    <rdf:type rdf:resource="http://www.w3.org/2002/07/owl#NamedIndividual"/>
  </s4ener:Usage>
  <s4ener:Usage rdf:about="https://saref.etsi.org/saref4ener/Production">
    <rdfs:label xml:lang="en">Production</rdfs:label>
    <rdfs:comment>This datapoint indicates the energy production.</rdfs:comment>
    <rdf:type rdf:resource="http://www.w3.org/2002/07/owl#NamedIndividual"/>
  </s4ener:Usage>
  <s4ener:ScopeType rdf:about="https://saref.etsi.org/saref4ener/Preliminary">
    <rdfs:label xml:lang="en">Preliminary</rdfs:label>
    <rdfs:comment xml:lang="en">The preliminary version of this concept, usually an incentive table or power plan</rdfs:comment>
    <rdf:type rdf:resource="http://www.w3.org/2002/07/owl#NamedIndividual"/>
  </s4ener:ScopeType>
  <s4ener:InstructionStatus rdf:about="https://saref.etsi.org/saref4ener/Accepted">
    <rdfs:label xml:lang="en">Accepted</rdfs:label>
    <rdfs:comment>Instruction has been accepted</rdfs:comment>
    <rdf:type rdf:resource="http://www.w3.org/2002/07/owl#NamedIndividual"/>
  </s4ener:InstructionStatus>
  <s4ener:Usage rdf:about="https://saref.etsi.org/saref4ener/Average">
    <rdfs:label xml:lang="en">Average</rdfs:label>
    <rdfs:comment>The datapoint indicates an average value aggregated over a number of values.</rdfs:comment>
    <rdf:type rdf:resource="http://www.w3.org/2002/07/owl#NamedIndividual"/>
  </s4ener:Usage>
  <s4ener:InstructionStatus rdf:about="https://saref.etsi.org/saref4ener/Revoked">
    <rdfs:label xml:lang="en">Revoked</rdfs:label>
    <rdfs:comment>Instruction was revoked</rdfs:comment>
    <rdf:type rdf:resource="http://www.w3.org/2002/07/owl#NamedIndividual"/>
  </s4ener:InstructionStatus>
  <s4ener:InstructionStatus rdf:about="https://saref.etsi.org/saref4ener/Rejected">
    <rdfs:label xml:lang="en">Rejected</rdfs:label>
    <rdfs:comment>Instruction was rejected</rdfs:comment>
    <rdf:type rdf:resource="http://www.w3.org/2002/07/owl#NamedIndividual"/>
  </s4ener:InstructionStatus>
  <s4ener:Usage rdf:about="https://saref.etsi.org/saref4ener/BaseLine">
    <rdfs:label xml:lang="en">Baseline</rdfs:label>
    <rdfs:comment>This datapoint indicates the baseline.</rdfs:comment>
    <rdf:type rdf:resource="http://www.w3.org/2002/07/owl#NamedIndividual"/>
  </s4ener:Usage>
  <s4ener:PowerSequenceState rdf:about="https://saref.etsi.org/saref4ener/Inactive">
    <rdfs:label xml:lang="en">Inactive</rdfs:label>
    <rdfs:comment xml:lang="en">Power sequence state with value 'inactive'</rdfs:comment>
    <rdf:type rdf:resource="http://www.w3.org/2002/07/owl#NamedIndividual"/>
  </s4ener:PowerSequenceState>
  <s4ener:PowerSource rdf:about="https://saref.etsi.org/saref4ener/BatteryPowerSource">
    <rdfs:label xml:lang="en">Battery power source</rdfs:label>
    <rdfs:comment>This Power Source codelist element indicates that a battery is the power source of this device.</rdfs:comment>
  </s4ener:PowerSource>
  <s4ener:PowerSequenceState rdf:about="https://saref.etsi.org/saref4ener/Invalid">
    <rdfs:label xml:lang="en">Invalid</rdfs:label>
    <rdfs:comment xml:lang="en">Power sequence state with value 'invalid'</rdfs:comment>
    <rdf:type rdf:resource="http://www.w3.org/2002/07/owl#NamedIndividual"/>
  </s4ener:PowerSequenceState>
  <s4ener:CommodityQuantity rdf:about="https://saref.etsi.org/saref4ener/ElectricPower3PhaseSymmetric">
    <rdfs:label xml:lang="en">Electric Power 3 Phase Symmetric</rdfs:label>
    <rdfs:comment>Electric power described in Watt on when power is equally shared among the three phases. Only applicable for 3 phase devices.</rdfs:comment>
  </s4ener:CommodityQuantity>
  <s4ener:PowerSequenceState rdf:about="https://saref.etsi.org/saref4ener/Running">
    <rdfs:label xml:lang="en">Running</rdfs:label>
    <rdfs:comment xml:lang="en">Power sequence state with value 'running'</rdfs:comment>
    <rdf:type rdf:resource="http://www.w3.org/2002/07/owl#NamedIndividual"/>
  </s4ener:PowerSequenceState>
  <s4ener:RoleType rdf:about="https://saref.etsi.org/saref4ener/EnergyStorage">
    <rdfs:label xml:lang="en">Energy Storage</rdfs:label>
    <rdfs:comment>Identifier for RoleType Storage</rdfs:comment>
    <rdf:type rdf:resource="http://www.w3.org/2002/07/owl#NamedIndividual"/>
  </s4ener:RoleType>
  <s4ener:Usage rdf:about="https://saref.etsi.org/saref4ener/LowerLimit">
    <rdfs:label xml:lang="en">Lower limit</rdfs:label>
    <rdfs:label xml:lang="en">Lower Limit</rdfs:label>
    <rdfs:comment>This data point indicates the lower limit.</rdfs:comment>
    <rdfs:comment>The PowerEnvelopeLimitType codelist element indicating the lower limit.</rdfs:comment>
    <rdf:type rdf:resource="https://saref.etsi.org/saref4ener/PowerEnvelopeLimitType"/>
    <rdf:type rdf:resource="http://www.w3.org/2002/07/owl#NamedIndividual"/>
  </s4ener:Usage>
  <s4ener:ValueTendency rdf:about="https://saref.etsi.org/saref4ener/Falling">
    <rdfs:label xml:lang="en">Falling</rdfs:label>
    <rdfs:comment>This value tendency codelist element indicates that the tendency of this measurement indicates that the value is decreasing (i.e., falling).</rdfs:comment>
  </s4ener:ValueTendency>
  <s4ener:ScopeType rdf:about="https://saref.etsi.org/saref4ener/Committed">
    <rdfs:label xml:lang="en">Committed</rdfs:label>
    <rdfs:comment xml:lang="en">The committed version of this concept, usually an incentive table or power plan</rdfs:comment>
    <rdf:type rdf:resource="http://www.w3.org/2002/07/owl#NamedIndividual"/>
  </s4ener:ScopeType>
  <s4ener:CommodityQuantity rdf:about="https://saref.etsi.org/saref4ener/ElectricPowerL1">
    <rdfs:label xml:lang="en">Electric Power L1</rdfs:label>
    <rdfs:comment>Electric power described in Watt on phase 1. If a device utilizes only one phase it should always use L1.</rdfs:comment>
  </s4ener:CommodityQuantity>
  <s4ener:PowerSequenceState rdf:about="https://saref.etsi.org/saref4ener/Completed">
    <rdfs:label xml:lang="en">Completed</rdfs:label>
    <rdfs:comment xml:lang="en">Power sequence state with value 'completed'</rdfs:comment>
    <rdf:type rdf:resource="http://www.w3.org/2002/07/owl#NamedIndividual"/>
  </s4ener:PowerSequenceState>
  <s4ener:ValueSource rdf:about="https://saref.etsi.org/saref4ener/Measured">
    <rdfs:label xml:lang="en">Measured</rdfs:label>
    <rdfs:comment>The value source type indicates that this data point has been measured by a device.</rdfs:comment>
  </s4ener:ValueSource>
  <s4ener:PowerSequenceStatus rdf:about="https://saref.etsi.org/saref4ener/Finished">
    <rdfs:label xml:lang="en">Finished</rdfs:label>
    <rdfs:comment>The selected PPBC.PowerSequence was executed and finished successfully</rdfs:comment>
  </s4ener:PowerSequenceStatus>
  <saref:Commodity rdf:about="https://saref.etsi.org/saref4ener/Heat">
    <rdfs:label xml:lang="en">Heat</rdfs:label>
    <rdfs:comment>Identifier for Commodity Heat</rdfs:comment>
  </saref:Commodity>
  <s4ener:PowerSource rdf:about="https://saref.etsi.org/saref4ener/MainsSinglePhase">
    <rdfs:label xml:lang="en">Mains single phase</rdfs:label>
    <rdfs:comment>This codelist element of power source indicates that the power source is the mains single phase.</rdfs:comment>
  </s4ener:PowerSource>
  <saref:Gas rdf:about="https://saref.etsi.org/saref4ener/Gas">
    <rdfs:label xml:lang="en">Gas</rdfs:label>
    <rdfs:comment>Identifier for Commodity GAS</rdfs:comment>
  </saref:Gas>
  <saref:Electricity rdf:about="https://saref.etsi.org/saref4ener/Electricity">
    <rdfs:label xml:lang="en">Electricity</rdfs:label>
    <rdfs:comment>Identifier for Commodity ELECTRICITY</rdfs:comment>
  </saref:Electricity>
  <s4ener:ValueTendency rdf:about="https://saref.etsi.org/saref4ener/Stable">
    <rdfs:label xml:lang="en">Stable</rdfs:label>
    <rdfs:comment>This value tendency codelist element indicates that the tendency this measurement has is to stay stable, instead of rising or falling.</rdfs:comment>
  </s4ener:ValueTendency>
  <saref:Commodity rdf:about="https://saref.etsi.org/saref4ener/Oil">
    <rdfs:label xml:lang="en">Oil</rdfs:label>
    <rdfs:comment>Identifier for Commodity OIL</rdfs:comment>
  </saref:Commodity>
  <s4ener:IncentiveType rdf:about="https://saref.etsi.org/saref4ener/RenewableEnergyPercentage">
    <rdfs:label xml:lang="en">Renewable energy percentage</rdfs:label>
    <rdfs:comment xml:lang="en">The  incentive type ''renewable energy percentage'' defined in the incentive table.</rdfs:comment>
    <rdf:type rdf:resource="http://www.w3.org/2002/07/owl#NamedIndividual"/>
  </s4ener:IncentiveType>
  <s4ener:PowerEnvelopeConsequenceType rdf:about="https://saref.etsi.org/saref4ener/Vanish">
    <rdfs:label xml:lang="en">Vanish</rdfs:label>
    <rdfs:comment>The load or generation that is limited will vanish. This is for example the case with curtailing production from solar panels; the potentially generated energy is lost and will never reappear.</rdfs:comment>
    <rdf:type rdf:resource="http://www.w3.org/2002/07/owl#NamedIndividual"/>
  </s4ener:PowerEnvelopeConsequenceType>
  <s4ener:InstructionStatus rdf:about="https://saref.etsi.org/saref4ener/Started">
    <rdfs:label xml:lang="en">Started</rdfs:label>
    <rdfs:comment>Instruction was executed</rdfs:comment>
    <rdf:type rdf:resource="http://www.w3.org/2002/07/owl#NamedIndividual"/>
  </s4ener:InstructionStatus>
  <s4ener:PowerSequenceStatus rdf:about="https://saref.etsi.org/saref4ener/Interrupted">
    <rdfs:label xml:lang="en">Interrupted</rdfs:label>
    <rdfs:comment>The selected PPBC.PowerSequence is being executed, but is currently interrupted and will continue afterwards</rdfs:comment>
  </s4ener:PowerSequenceStatus>
  <s4ener:CommodityQuantity rdf:about="https://saref.etsi.org/saref4ener/HydrogenFlowRate">
    <rdfs:label xml:lang="en">Hydrogen Flow Rate</rdfs:label>
    <rdfs:comment>Gas flow rate described in grams per second</rdfs:comment>
  </s4ener:CommodityQuantity>
  <s4ener:PowerSequenceStatus rdf:about="https://saref.etsi.org/saref4ener/NotScheduled">
    <rdfs:label xml:lang="en">NotScheduled</rdfs:label>
    <rdfs:comment>No PPBC.PowerSequence within the PPBC.PowerSequenceContainer is scheduled</rdfs:comment>
  </s4ener:PowerSequenceStatus>
  <s4ener:PowerSequenceStatus rdf:about="https://saref.etsi.org/saref4ener/Aborted">
    <rdfs:label xml:lang="en">Aborted</rdfs:label>
    <rdfs:comment>The selected PPBC.PowerSequence was aborted by the device and will not continue</rdfs:comment>
    <rdfs:comment>Instruction was aborted.</rdfs:comment>
    <rdf:type rdf:resource="https://saref.etsi.org/saref4ener/InstructionStatus"/>
    <rdf:type rdf:resource="http://www.w3.org/2002/07/owl#NamedIndividual"/>
  </s4ener:PowerSequenceStatus>
  <s4ener:Usage rdf:about="https://saref.etsi.org/saref4ener/Maximum">
    <rdfs:label xml:lang="en">Maximum</rdfs:label>
    <rdfs:comment>The usage of this datapoint is the Maximum value.</rdfs:comment>
    <rdf:type rdf:resource="http://www.w3.org/2002/07/owl#NamedIndividual"/>
  </s4ener:Usage>
  <s4ener:RoleType rdf:about="https://saref.etsi.org/saref4ener/EnergyConsumer">
    <rdfs:label xml:lang="en">Energy Consumer</rdfs:label>
    <rdfs:comment>Identifier for RoleType Consumer</rdfs:comment>
    <rdf:type rdf:resource="http://www.w3.org/2002/07/owl#NamedIndividual"/>
  </s4ener:RoleType>
  <s4ener:Usage rdf:about="https://saref.etsi.org/saref4ener/UpperLimit">
    <rdfs:label xml:lang="en">Upper limit</rdfs:label>
    <rdfs:label xml:lang="en">Upper Limit</rdfs:label>
    <rdfs:comment>This datapoint indicates the upperlimit.</rdfs:comment>
    <rdfs:comment>The PowerEnvelopeLimitType enumeration for the upper limit.</rdfs:comment>
    <rdf:type rdf:resource="https://saref.etsi.org/saref4ener/PowerEnvelopeLimitType"/>
    <rdf:type rdf:resource="http://www.w3.org/2002/07/owl#NamedIndividual"/>
  </s4ener:Usage>
  <s4ener:PowerEnvelopeConsequenceType rdf:about="https://saref.etsi.org/saref4ener/Defer">
    <rdfs:label xml:lang="en">Defer</rdfs:label>
    <rdfs:comment>Indicating that the limited load or generation will be postponed to a later moment </rdfs:comment>
    <rdf:type rdf:resource="http://www.w3.org/2002/07/owl#NamedIndividual"/>
  </s4ener:PowerEnvelopeConsequenceType>
</rdf:RDF>
