<rdf:RDF
    xmlns:rdf="http://www.w3.org/1999/02/22-rdf-syntax-ns#"
    xmlns:dcterms="http://purl.org/dc/terms/"
    xmlns:s4bldg="https://saref.etsi.org/saref4bldg/"
    xmlns:s4syst="https://saref.etsi.org/saref4syst/"
    xmlns:owl="http://www.w3.org/2002/07/owl#"
    xmlns:s4lift="https://saref.etsi.org/saref4lift/"
    xmlns:skos="http://www.w3.org/2004/02/skos/core#"
    xmlns:schema="http://schema.org/"
    xmlns:rdfs="http://www.w3.org/2000/01/rdf-schema#"
    xmlns:saref="https://saref.etsi.org/core/"
    xmlns:vann="http://purl.org/vocab/vann/"
    xmlns:xsd="http://www.w3.org/2001/XMLSchema#">
  <owl:Ontology rdf:about="https://saref.etsi.org/saref4lift/">
    <dcterms:issued rdf:datatype="http://www.w3.org/2001/XMLSchema#date"
    >2021-05-25</dcterms:issued>
    <dcterms:creator rdf:resource="https://www.linkedin.com/in/albafernandezizquierdo"/>
    <dcterms:creator rdf:resource="http://www.maxime-lefrancois.info/"/>
    <dcterms:publisher rdf:resource="https://www.etsi.org/"/>
    <owl:versionInfo>v1.1.1</owl:versionInfo>
    <dcterms:modified rdf:datatype="http://www.w3.org/2001/XMLSchema#date"
    >2021-03-15</dcterms:modified>
    <dcterms:creator rdf:resource="https://pdi.fbk.eu/people/profile/dragoni"/>
    <vann:preferredNamespaceUri>https://saref.etsi.org/saref4lift/</vann:preferredNamespaceUri>
    <owl:versionIRI rdf:resource="https://saref.etsi.org/saref4lift/v1.1.1/"/>
    <dcterms:creator rdf:resource="http://www.garcia-castro.com/foaf.rdf#me"/>
    <dcterms:source rdf:resource="https://saref.etsi.org/sources/saref4lift/"/>
    <vann:preferredNamespacePrefix>s4lift</vann:preferredNamespacePrefix>
    <owl:imports rdf:resource="https://saref.etsi.org/saref4bldg/v1.1.2/"/>
    <dcterms:description xml:lang="en">This ontology extends the SAREF ontology for the Smart Lifts domain.</dcterms:description>
    <owl:imports rdf:resource="https://saref.etsi.org/saref4syst/v1.1.2/"/>
    <owl:imports rdf:resource="https://saref.etsi.org/core/v3.1.1/"/>
    <dcterms:creator rdf:resource="https://www.linkedin.com/in/mahdi-bennara/"/>
    <dcterms:title xml:lang="en">SAREF extension for Smart Lifts</dcterms:title>
    <rdfs:seeAlso rdf:resource="https://www.etsi.org/deliver/etsi_ts/103400_103499/10341011/01.01.01_60/ts_10341011v010101p.pdf"/>
    <dcterms:license rdf:resource="https://forge.etsi.org/etsi-software-license"/>
  </owl:Ontology>
  <rdfs:Datatype rdf:about="http://www.opengis.net/ont/geosparql#wktLiteral">
    <rdfs:label xml:lang="en">Well-known Text Literal</rdfs:label>
    <rdfs:isDefinedBy rdf:resource="http://www.opengis.net/ont/geosparql#"/>
    <rdfs:comment xml:lang="en">A Well-known Text serialization of a geometry object.</rdfs:comment>
  </rdfs:Datatype>
  <owl:Class rdf:about="https://saref.etsi.org/saref4lift/TestRideCommand">
    <rdfs:label xml:lang="en">Test ride command</rdfs:label>
    <rdfs:comment xml:lang="en">A type of command to set the test ride state.</rdfs:comment>
    <rdfs:subClassOf rdf:resource="https://saref.etsi.org/core/Command"/>
  </owl:Class>
  <owl:Class rdf:about="https://saref.etsi.org/saref4lift/AlarmInTheMachineryState">
    <rdfs:comment xml:lang="en">State of a device when the alarm in the machinery has been activated.</rdfs:comment>
    <rdfs:label xml:lang="en">Alarm in the machinery state</rdfs:label>
    <rdfs:subClassOf>
      <owl:Class rdf:about="https://saref.etsi.org/saref4lift/AlarmState"/>
    </rdfs:subClassOf>
  </owl:Class>
  <owl:Class rdf:about="https://saref.etsi.org/saref4lift/NumberOfCallsStatistics">
    <rdfs:comment xml:lang="en">Total counter of the number of calls since the last reset. As per concept historyPeriodic in ISO 16484-5</rdfs:comment>
    <rdfs:label xml:lang="en">Number of calls statistics</rdfs:label>
    <rdfs:subClassOf>
      <owl:Class rdf:about="https://saref.etsi.org/saref4lift/StatisticsMeasurement"/>
    </rdfs:subClassOf>
  </owl:Class>
  <owl:Class rdf:about="https://saref.etsi.org/saref4lift/EmergencyPowerSupplyState">
    <rdfs:comment xml:lang="en">The state of a device that is using the emergency power supply.</rdfs:comment>
    <rdfs:label xml:lang="en">Emergency Power Supply State</rdfs:label>
    <rdfs:subClassOf>
      <owl:Class rdf:about="https://saref.etsi.org/saref4lift/PowerSupplyState"/>
    </rdfs:subClassOf>
  </owl:Class>
  <owl:Class rdf:about="https://saref.etsi.org/saref4lift/MovingUpwardDirectionState">
    <rdfs:comment xml:lang="en">The state of a device that is moving in the upward direction</rdfs:comment>
    <rdfs:label xml:lang="en">Moving Upward Direction State</rdfs:label>
    <rdfs:subClassOf>
      <owl:Class rdf:about="https://saref.etsi.org/saref4lift/MovingDirectionState"/>
    </rdfs:subClassOf>
  </owl:Class>
  <owl:Class rdf:about="https://saref.etsi.org/saref4lift/Load">
    <rdfs:label xml:lang="en">Load</rdfs:label>
    <rdfs:comment xml:lang="en">A saref:Property related to the load carried by a device.</rdfs:comment>
    <rdfs:subClassOf rdf:resource="https://saref.etsi.org/core/Property"/>
  </owl:Class>
  <owl:Class rdf:about="https://saref.etsi.org/saref4lift/StatisticSignal">
    <rdfs:comment xml:lang="en">A signal associated to some statistics measurement of a device</rdfs:comment>
    <rdfs:label xml:lang="en">Statistic signal</rdfs:label>
    <rdfs:subClassOf>
      <owl:Restriction>
        <owl:someValuesFrom>
          <owl:Class rdf:about="https://saref.etsi.org/saref4lift/StatisticsMeasurement"/>
        </owl:someValuesFrom>
        <owl:onProperty>
          <owl:ObjectProperty rdf:about="https://saref.etsi.org/saref4lift/conveys"/>
        </owl:onProperty>
      </owl:Restriction>
    </rdfs:subClassOf>
    <rdfs:subClassOf>
      <owl:Class rdf:about="https://saref.etsi.org/saref4lift/Signal"/>
    </rdfs:subClassOf>
  </owl:Class>
  <owl:Class rdf:about="https://saref.etsi.org/saref4lift/ElectricalConnectionPoint">
    <rdfs:label xml:lang="en">Electrical Conection Point</rdfs:label>
    <rdfs:comment xml:lang="en">The class of electrical connection points of electric power systems, at which they may be electricaly connected to other systems.</rdfs:comment>
    <rdfs:subClassOf rdf:resource="https://saref.etsi.org/saref4syst/ConnectionPoint"/>
  </owl:Class>
  <owl:Class rdf:about="https://saref.etsi.org/saref4lift/MainBoardResetCommand">
    <rdfs:label xml:lang="en">Main board reset command</rdfs:label>
    <rdfs:comment xml:lang="en">A type of command to initiate the board reset</rdfs:comment>
    <rdfs:subClassOf rdf:resource="https://saref.etsi.org/core/Command"/>
  </owl:Class>
  <owl:Class rdf:about="http://www.opengis.net/ont/geosparql#SpatialObject">
    <rdfs:label xml:lang="en">Spatial object</rdfs:label>
    <rdfs:isDefinedBy rdf:resource="http://www.opengis.net/ont/geosparql#"/>
  </owl:Class>
  <owl:Class rdf:about="https://saref.etsi.org/saref4lift/AlarmVoiceCommunicationState">
    <rdfs:comment xml:lang="en">State of a device when alarm voice communication has been activated. In UE and other applicable countries alarms shall comply to EN 81-28</rdfs:comment>
    <rdfs:label xml:lang="en">Alarm voice communication state</rdfs:label>
    <rdfs:subClassOf rdf:resource="https://saref.etsi.org/core/State"/>
  </owl:Class>
  <owl:Class rdf:about="https://saref.etsi.org/saref4lift/SendCarToSpecificServiceCommand">
    <rdfs:label xml:lang="en">Send car to specific service command</rdfs:label>
    <rdfs:comment xml:lang="en">A type of command to call the car to a specific service.</rdfs:comment>
    <rdfs:subClassOf rdf:resource="https://saref.etsi.org/core/Command"/>
  </owl:Class>
  <owl:Class rdf:about="https://saref.etsi.org/saref4lift/OutOfServiceState">
    <rdfs:comment xml:lang="en">The state of a device that is out of service.</rdfs:comment>
    <rdfs:label xml:lang="en">Out of service state</rdfs:label>
    <rdfs:subClassOf rdf:resource="https://saref.etsi.org/core/State"/>
  </owl:Class>
  <owl:Class rdf:about="https://saref.etsi.org/saref4lift/AccessibleGoodsOnlySmartLift">
    <rdfs:comment xml:lang="en">The class of Smart Lifts that are used for accessible goods only, as per [EN 81-31].</rdfs:comment>
    <rdfs:label xml:lang="en">Accessible goods only smart lift</rdfs:label>
    <rdfs:subClassOf>
      <owl:Class rdf:about="https://saref.etsi.org/saref4lift/SmartLiftInstallation"/>
    </rdfs:subClassOf>
  </owl:Class>
  <owl:Class rdf:about="https://saref.etsi.org/saref4lift/NetworkAccess">
    <rdfs:comment xml:lang="en">Network accesss is a connection capability between a system and a network.</rdfs:comment>
    <rdfs:label xml:lang="en">Network Access</rdfs:label>
    <rdfs:subClassOf rdf:resource="https://saref.etsi.org/saref4syst/Connection"/>
  </owl:Class>
  <owl:Class rdf:about="https://saref.etsi.org/saref4lift/MachineRoomLessSmartLift">
    <rdfs:comment xml:lang="en">The class of smart lifts which do not require a machine room.</rdfs:comment>
    <rdfs:label xml:lang="en">Machine room less smart lift</rdfs:label>
    <rdfs:subClassOf>
      <owl:Class rdf:about="https://saref.etsi.org/saref4lift/SmartLiftInstallation"/>
    </rdfs:subClassOf>
  </owl:Class>
  <owl:Class rdf:about="http://www.opengis.net/ont/geosparql#Feature">
    <rdfs:label xml:lang="en">Feature</rdfs:label>
    <rdfs:isDefinedBy rdf:resource="http://www.opengis.net/ont/geosparql#"/>
    <rdfs:comment xml:lang="en">This class represents the top-level feature type. This class is equivalent to GFI_Feature defined in ISO 19156:2011, and it is superclass of all feature types.</rdfs:comment>
    <rdfs:subClassOf rdf:resource="http://www.opengis.net/ont/geosparql#SpatialObject"/>
  </owl:Class>
  <owl:Class rdf:about="https://saref.etsi.org/saref4lift/SmartLiftEdgeControlUnit">
    <rdfs:label xml:lang="en">Smart Lift Edge Control Unit</rdfs:label>
    <rdfs:comment xml:lang="en">A  Smart Lift Edge Control Unit  is the main element of a Smart Lift installation and it is typically associated with the lift control cabinet</rdfs:comment>
    <rdfs:subClassOf rdf:resource="https://saref.etsi.org/saref4syst/System"/>
    <rdfs:subClassOf rdf:resource="https://saref.etsi.org/core/Device"/>
  </owl:Class>
  <owl:Class rdf:about="https://saref.etsi.org/saref4lift/SmartLiftGroup">
    <rdfs:label xml:lang="en">Smart Lift Group</rdfs:label>
    <rdfs:comment xml:lang="en">A Smart Lift Group represents the correlation of multiple Smart Lifts Installation and it is supported by the introduction of a Smart Lift Group identifier common each Smart Lifts Installation belonging to the same Smart Lift Group. Such kind of installations usually presents control units connected one each other to coordinate the movement and position of the different lifts, where the common commands (e.g. the call buttons) are given to one of these control units that acts as a principal master and coordinates the other installations or is composed by peer installations that coordinates one each othe</rdfs:comment>
    <rdfs:subClassOf rdf:resource="https://saref.etsi.org/saref4syst/System"/>
    <rdfs:subClassOf rdf:resource="https://saref.etsi.org/core/FeatureOfInterest"/>
  </owl:Class>
  <owl:Class rdf:about="https://saref.etsi.org/saref4lift/CarInUnlockingSpaceState">
    <rdfs:comment xml:lang="en">The state of a lift where the car is in some door unlocking building space.</rdfs:comment>
    <rdfs:label xml:lang="en">Car In Unlocking Space state</rdfs:label>
    <rdfs:subClassOf rdf:resource="https://saref.etsi.org/core/State"/>
  </owl:Class>
  <owl:Class rdf:about="https://saref.etsi.org/saref4lift/DirectCurrentConnectionPoint">
    <rdfs:subClassOf rdf:resource="https://saref.etsi.org/saref4lift/ElectricalConnectionPoint"/>
    <rdfs:comment xml:lang="en">The class of electrical connection points through which energy flows using direct current.</rdfs:comment>
    <rdfs:label xml:lang="en">Direct Current Connection Point</rdfs:label>
  </owl:Class>
  <owl:Class rdf:about="https://saref.etsi.org/saref4lift/DoorConnectionPoint">
    <rdfs:subClassOf rdf:resource="https://saref.etsi.org/saref4syst/ConnectionPoint"/>
    <rdfs:comment xml:lang="en">The class of door connection points, which have an open or close state. Smart Lift Car has some door connection points. A connection between building spaces can be at a door connection point.</rdfs:comment>
    <rdfs:label xml:lang="en">Door Connection Point</rdfs:label>
  </owl:Class>
  <owl:Class rdf:about="https://saref.etsi.org/saref4lift/StatisticsMeasurement">
    <rdfs:comment xml:lang="en">A measurement of some statistics of a feature of interest</rdfs:comment>
    <rdfs:label xml:lang="en">Statistics Measurement</rdfs:label>
    <rdfs:subClassOf rdf:resource="https://saref.etsi.org/core/Measurement"/>
  </owl:Class>
  <owl:Class rdf:about="https://saref.etsi.org/saref4lift/TestEmergencyNumberCommand">
    <rdfs:label xml:lang="en">Test emergency number command</rdfs:label>
    <rdfs:comment xml:lang="en">A type of command to test the emergency number</rdfs:comment>
    <rdfs:subClassOf rdf:resource="https://saref.etsi.org/core/Command"/>
  </owl:Class>
  <owl:Class rdf:about="http://www.opengis.net/ont/geosparql#Geometry">
    <rdfs:label xml:lang="en">Geometry</rdfs:label>
    <rdfs:isDefinedBy rdf:resource="http://www.opengis.net/ont/geosparql#"/>
    <rdfs:comment xml:lang="en">The class represents the top-level geometry type. This class is equivalent to the UML class GM_Object defined in ISO 19107, and it is superclass of all geometry types.</rdfs:comment>
    <rdfs:subClassOf rdf:resource="http://www.opengis.net/ont/geosparql#SpatialObject"/>
  </owl:Class>
  <owl:Class rdf:about="https://saref.etsi.org/saref4lift/SmartLiftEdgeComponent">
    <rdfs:label xml:lang="en">Smart Lift Edge Component</rdfs:label>
    <rdfs:comment xml:lang="en">A Smart Lift Edge Component is dedicated to the hosting of smart lift additional modules in the case that they are not hosted directly in the  Smart Lift Edge Control Unit. An example could be the case of an additional earthquake sensor added after the lift deployment and not controlled by the Smart Lift Edge Control Unit.</rdfs:comment>
    <rdfs:subClassOf rdf:resource="https://saref.etsi.org/saref4syst/System"/>
    <rdfs:subClassOf rdf:resource="https://saref.etsi.org/core/Device"/>
  </owl:Class>
  <owl:Class rdf:about="https://saref.etsi.org/saref4lift/PowerSupplyState">
    <rdfs:comment xml:lang="en">A type of state.</rdfs:comment>
    <rdfs:label xml:lang="en">Power Supply State</rdfs:label>
    <rdfs:subClassOf rdf:resource="https://saref.etsi.org/core/State"/>
  </owl:Class>
  <owl:Class rdf:about="https://saref.etsi.org/saref4lift/CarStopSpace">
    <rdfs:subClassOf>
      <owl:Restriction>
        <owl:someValuesFrom rdf:resource="https://saref.etsi.org/saref4lift/DoorConnectionPoint"/>
        <owl:onProperty rdf:resource="https://saref.etsi.org/saref4syst/connectsAt"/>
      </owl:Restriction>
    </rdfs:subClassOf>
    <rdfs:subClassOf rdf:resource="https://saref.etsi.org/saref4bldg/BuildingSpace"/>
    <rdfs:comment xml:lang="en">The class of building spaces where smart lift car can stop to enable doors opening unlocking</rdfs:comment>
    <rdfs:label xml:lang="en">Door Space</rdfs:label>
  </owl:Class>
  <owl:Class rdf:about="https://saref.etsi.org/saref4lift/AlarmInTheRoofState">
    <rdfs:comment xml:lang="en">State of a device when the alarm in the roof has been activated.</rdfs:comment>
    <rdfs:label xml:lang="en">Alarm in the roof state</rdfs:label>
    <rdfs:subClassOf>
      <owl:Class rdf:about="https://saref.etsi.org/saref4lift/AlarmState"/>
    </rdfs:subClassOf>
  </owl:Class>
  <owl:Class rdf:about="https://saref.etsi.org/saref4lift/NumberOfFaults">
    <rdfs:comment xml:lang="en">Number of faults.</rdfs:comment>
    <rdfs:label xml:lang="en">Number of faults</rdfs:label>
    <rdfs:subClassOf rdf:resource="https://saref.etsi.org/saref4lift/StatisticsMeasurement"/>
  </owl:Class>
  <owl:Class rdf:about="https://saref.etsi.org/saref4lift/FaultSignal">
    <rdfs:label xml:lang="en">Fault signal</rdfs:label>
    <rdfs:comment xml:lang="en">A signal describing some fault.</rdfs:comment>
    <rdfs:subClassOf>
      <owl:Class rdf:about="https://saref.etsi.org/saref4lift/Signal"/>
    </rdfs:subClassOf>
  </owl:Class>
  <owl:Class rdf:about="https://saref.etsi.org/saref4lift/ReservedServiceState">
    <rdfs:comment xml:lang="en">The state of a device when the reserved operation is on run. For Smart Lifts it is typically related to the use of a key or a proximity badge to reach a specific floor(s) or service(es). Some examples of reserved operation are the access to a hotel guest to the room floor, of the housekeeper to a floor (or a service door) to access a personnel-only area, the access of surgical room area in a hospital, etc.</rdfs:comment>
    <rdfs:label xml:lang="en">Reserved service state</rdfs:label>
    <rdfs:subClassOf rdf:resource="https://saref.etsi.org/core/State"/>
  </owl:Class>
  <owl:Class rdf:about="https://saref.etsi.org/saref4lift/ElectricPowerSystem">
    <rdfs:label xml:lang="en">Electric Power System</rdfs:label>
    <rdfs:comment xml:lang="en">The class of electric power systems, i.e., systems that exchange electricity (i.e., electric power) with other systems.</rdfs:comment>
    <rdfs:subClassOf rdf:resource="https://saref.etsi.org/saref4syst/System"/>
  </owl:Class>
  <owl:Class rdf:about="https://saref.etsi.org/saref4lift/MovingDownwardDirectionState">
    <rdfs:comment xml:lang="en">The state of a device that is moving in the downward direction</rdfs:comment>
    <rdfs:label xml:lang="en">Moving Downward Direction State</rdfs:label>
    <rdfs:subClassOf>
      <owl:Class rdf:about="https://saref.etsi.org/saref4lift/MovingDirectionState"/>
    </rdfs:subClassOf>
  </owl:Class>
  <owl:Class rdf:about="https://saref.etsi.org/saref4lift/TestRideInExecutionState">
    <rdfs:comment xml:lang="en">The state of a device that is subject to a test ride.</rdfs:comment>
    <rdfs:label xml:lang="en">Test ride in execution state</rdfs:label>
    <rdfs:subClassOf rdf:resource="https://saref.etsi.org/core/State"/>
  </owl:Class>
  <owl:Class rdf:about="https://saref.etsi.org/saref4lift/GoodBatteryPowerState">
    <rdfs:comment xml:lang="en">The state of a system whose battery is in good operating conditions.</rdfs:comment>
    <rdfs:label xml:lang="en">Good Battery Power State</rdfs:label>
    <rdfs:subClassOf>
      <owl:Class rdf:about="https://saref.etsi.org/saref4lift/BatteryPowerState"/>
    </rdfs:subClassOf>
  </owl:Class>
  <owl:Class rdf:about="https://saref.etsi.org/saref4lift/SetRealTimeModeCommand">
    <rdfs:label xml:lang="en">Set real time mode command</rdfs:label>
    <rdfs:comment xml:lang="en">A type of command to set the real time mode on or off.</rdfs:comment>
    <rdfs:subClassOf rdf:resource="https://saref.etsi.org/core/Command"/>
  </owl:Class>
  <owl:Class rdf:about="https://saref.etsi.org/saref4lift/AlarmInTheWellState">
    <rdfs:comment xml:lang="en">State of a device when the alarm in the well has been activated.</rdfs:comment>
    <rdfs:label xml:lang="en">Alarm in the well state</rdfs:label>
    <rdfs:subClassOf>
      <owl:Class rdf:about="https://saref.etsi.org/saref4lift/AlarmState"/>
    </rdfs:subClassOf>
  </owl:Class>
  <owl:Class rdf:about="https://saref.etsi.org/saref4lift/Voltage">
    <rdfs:label xml:lang="en">Voltage</rdfs:label>
    <rdfs:comment xml:lang="en">A saref:Property related to some measurements that are characterized by a certain value that is measured in a voltage unit (such as volt or kilovolt).</rdfs:comment>
    <rdfs:subClassOf rdf:resource="https://saref.etsi.org/core/Property"/>
  </owl:Class>
  <owl:Class rdf:about="https://saref.etsi.org/saref4lift/CriticalBatteryPowerState">
    <rdfs:comment xml:lang="en">The state of a system whose battery is in operating in critically reduced capability. For an emergency battery of a Smart Lift, a battery in critical state still has the power to send the car to the closest floor in case in failure, but needs to be replaced. For an emergency battery of a SOS Alarm system, the battery still has the power to sustain the alarm system active for the minimum time defined by applicable regulation, but needs to be replaced;</rdfs:comment>
    <rdfs:label xml:lang="en">Critical Battery Power State</rdfs:label>
    <rdfs:subClassOf>
      <owl:Class rdf:about="https://saref.etsi.org/saref4lift/BatteryPowerState"/>
    </rdfs:subClassOf>
  </owl:Class>
  <owl:Class rdf:about="https://saref.etsi.org/saref4lift/RealTimeModeState">
    <rdfs:comment xml:lang="en">The state of a device when the real time mode is active.</rdfs:comment>
    <rdfs:label xml:lang="en">Real time mode state</rdfs:label>
    <rdfs:subClassOf rdf:resource="https://saref.etsi.org/core/State"/>
  </owl:Class>
  <owl:Class rdf:about="https://saref.etsi.org/saref4lift/SmartLiftWithoutEmergencyCallSupport">
    <rdfs:subClassOf>
      <owl:Class rdf:about="https://saref.etsi.org/saref4lift/SmartLiftInstallation"/>
    </rdfs:subClassOf>
    <rdfs:comment xml:lang="en">The class of smart lift installatinos that lack support for emergency call. Emergency call support is typically mandatory in new lifts but may be lacking in old installations.</rdfs:comment>
    <rdfs:label xml:lang="en">Smart Lift Without Emergency Call Support</rdfs:label>
  </owl:Class>
  <owl:Class rdf:about="https://saref.etsi.org/saref4lift/NumberOfResetSequencesStatistics">
    <rdfs:comment xml:lang="en">Total counter of the number of reset sequences since the last reset. As per concept historyPeriodic in ISO 16484-5</rdfs:comment>
    <rdfs:label xml:lang="en">Number of reset sequences statistics</rdfs:label>
    <rdfs:subClassOf rdf:resource="https://saref.etsi.org/saref4lift/StatisticsMeasurement"/>
  </owl:Class>
  <owl:Class rdf:about="https://saref.etsi.org/saref4lift/InsufficientBatteryPowerState">
    <rdfs:comment xml:lang="en">The state of a system whose battery has insufficient capability. For an emergency battery of a Smart Lift, a battery in insufficient state does not have the power to send the car to the closest floor in case in failure; It needs to be urgently replaced. For an emergency battery of a SOS Alarm system, the battery does not have the power to sustain the alarm system active for the minimum time defined by applicable regulation; It needs to be urgently replaced. In UE and other applicable countries such minimum time is at least one hour (as required by EN 81-28).</rdfs:comment>
    <rdfs:label xml:lang="en">Insufficient Battery Power State</rdfs:label>
    <rdfs:subClassOf>
      <owl:Class rdf:about="https://saref.etsi.org/saref4lift/BatteryPowerState"/>
    </rdfs:subClassOf>
  </owl:Class>
  <owl:Class rdf:about="https://saref.etsi.org/saref4lift/AlarmSignal">
    <rdfs:comment xml:lang="en">High priority signal used to attract the operator’s attention to important deviations or abnormal events in system operation (from ISO 11064-5)</rdfs:comment>
    <rdfs:label xml:lang="en">Alarm Signal</rdfs:label>
    <rdfs:subClassOf>
      <owl:Class rdf:about="https://saref.etsi.org/saref4lift/Signal"/>
    </rdfs:subClassOf>
  </owl:Class>
  <owl:Class rdf:about="https://saref.etsi.org/saref4lift/TotalNumberOfOpeningOfDoorStatistics">
    <rdfs:comment xml:lang="en">Total counter of the number of opening of door since the last reset. As per concept historyPeriodic in ISO 16484-5</rdfs:comment>
    <rdfs:label xml:lang="en">Total number of opening of door statistics</rdfs:label>
    <rdfs:subClassOf rdf:resource="https://saref.etsi.org/saref4lift/StatisticsMeasurement"/>
  </owl:Class>
  <owl:Class rdf:about="https://saref.etsi.org/saref4lift/TotalFloorsCoveredStatistics">
    <rdfs:comment xml:lang="en">Total counter of the number of floors covered since the last reset. As per concept historyPeriodic in ISO 16484-5</rdfs:comment>
    <rdfs:label xml:lang="en">Total Floors Covered Statistics</rdfs:label>
    <rdfs:subClassOf rdf:resource="https://saref.etsi.org/saref4lift/StatisticsMeasurement"/>
  </owl:Class>
  <owl:Class rdf:about="https://saref.etsi.org/saref4lift/VerticalSmartLiftingPlatform">
    <rdfs:comment xml:lang="en">The class of vertical smart lifting platforms intended for use by persons with impaired mobility, as per [81-41].</rdfs:comment>
    <rdfs:label xml:lang="en">Vertical Smart lifting platform</rdfs:label>
    <rdfs:subClassOf>
      <owl:Class rdf:about="https://saref.etsi.org/saref4lift/SmartLiftInstallation"/>
    </rdfs:subClassOf>
  </owl:Class>
  <owl:Class rdf:about="https://saref.etsi.org/saref4lift/PassengerAndGoodsPassengerSmartLift">
    <rdfs:comment xml:lang="en">The class of passenger and goods passenger lifts, as per [EN 81-20].</rdfs:comment>
    <rdfs:label xml:lang="en">Passenger and goods passenger smart lift</rdfs:label>
    <rdfs:subClassOf>
      <owl:Class rdf:about="https://saref.etsi.org/saref4lift/SmartLiftInstallation"/>
    </rdfs:subClassOf>
  </owl:Class>
  <owl:Class rdf:about="https://saref.etsi.org/saref4lift/StandardPowerSupplyState">
    <rdfs:comment xml:lang="en">The state of a device that is using the standard power supply.</rdfs:comment>
    <rdfs:label xml:lang="en">Standard Power Supply State</rdfs:label>
    <rdfs:subClassOf rdf:resource="https://saref.etsi.org/saref4lift/PowerSupplyState"/>
  </owl:Class>
  <owl:Class rdf:about="https://saref.etsi.org/saref4lift/MovingDirectionState">
    <rdfs:comment xml:lang="en">A type of state</rdfs:comment>
    <rdfs:label xml:lang="en">Moving Direction State</rdfs:label>
    <rdfs:subClassOf rdf:resource="https://saref.etsi.org/core/State"/>
  </owl:Class>
  <owl:Class rdf:about="https://saref.etsi.org/saref4lift/SinglePhaseConnectionPoint">
    <rdfs:subClassOf rdf:resource="https://saref.etsi.org/saref4lift/ElectricalConnectionPoint"/>
    <rdfs:comment xml:lang="en">A single phase connection point is a connection point composed of two wires (plus the protective earth): 

- wire for the phase;
- wire for the neutral.</rdfs:comment>
    <rdfs:label xml:lang="en">Single Phase Connection Point</rdfs:label>
  </owl:Class>
  <owl:Class rdf:about="https://saref.etsi.org/saref4lift/SmartLiftInstallation">
    <rdfs:comment xml:lang="en">A Smart Lift Installation  in the Smart Lift  System corresponds to a single lift, with all its elements.</rdfs:comment>
    <rdfs:subClassOf rdf:resource="https://saref.etsi.org/core/FeatureOfInterest"/>
    <rdfs:subClassOf>
      <owl:Restriction>
        <owl:someValuesFrom rdf:resource="https://saref.etsi.org/saref4lift/SmartLiftEdgeControlUnit"/>
        <owl:onProperty rdf:resource="https://saref.etsi.org/saref4syst/hasSubSystem"/>
      </owl:Restriction>
    </rdfs:subClassOf>
    <rdfs:subClassOf rdf:resource="https://saref.etsi.org/saref4bldg/BuildingSpace"/>
    <rdfs:subClassOf>
      <owl:Restriction>
        <owl:someValuesFrom rdf:resource="https://saref.etsi.org/saref4lift/SmartLiftEdgeComponent"/>
        <owl:onProperty rdf:resource="https://saref.etsi.org/saref4syst/hasSubSystem"/>
      </owl:Restriction>
    </rdfs:subClassOf>
    <rdfs:subClassOf>
      <owl:Restriction>
        <owl:someValuesFrom rdf:resource="http://www.w3.org/2001/XMLSchema#anyURI"/>
        <owl:onProperty>
          <owl:DatatypeProperty rdf:about="https://saref.etsi.org/saref4lift/hasTelephoneNumber"/>
        </owl:onProperty>
      </owl:Restriction>
    </rdfs:subClassOf>
    <rdfs:subClassOf>
      <owl:Restriction>
        <owl:someValuesFrom rdf:resource="https://saref.etsi.org/saref4lift/CarStopSpace"/>
        <owl:onProperty rdf:resource="https://saref.etsi.org/saref4bldg/hasSpace"/>
      </owl:Restriction>
    </rdfs:subClassOf>
    <rdfs:subClassOf rdf:resource="http://www.opengis.net/ont/geosparql#Feature"/>
    <rdfs:subClassOf>
      <owl:Restriction>
        <owl:someValuesFrom rdf:resource="http://www.w3.org/2001/XMLSchema#anyURI"/>
        <owl:onProperty>
          <owl:DatatypeProperty rdf:about="https://saref.etsi.org/saref4lift/hasMainEmergencyTelephoneNumber"/>
        </owl:onProperty>
      </owl:Restriction>
    </rdfs:subClassOf>
    <rdfs:subClassOf>
      <owl:Restriction>
        <owl:minCardinality rdf:datatype="http://www.w3.org/2001/XMLSchema#integer"
        >1</owl:minCardinality>
        <owl:onProperty>
          <owl:DatatypeProperty rdf:about="https://saref.etsi.org/saref4lift/hasGeographicLocationValidator"/>
        </owl:onProperty>
      </owl:Restriction>
    </rdfs:subClassOf>
    <rdfs:subClassOf>
      <owl:Restriction>
        <owl:someValuesFrom rdf:resource="http://www.w3.org/2001/XMLSchema#anyURI"/>
        <owl:onProperty>
          <owl:DatatypeProperty rdf:about="https://saref.etsi.org/saref4lift/hasSecondaryEmergencyTelephoneNumber"/>
        </owl:onProperty>
      </owl:Restriction>
    </rdfs:subClassOf>
    <rdfs:subClassOf>
      <owl:Restriction>
        <owl:someValuesFrom>
          <owl:Class rdf:about="https://saref.etsi.org/saref4lift/Network"/>
        </owl:someValuesFrom>
        <owl:onProperty>
          <owl:ObjectProperty rdf:about="https://saref.etsi.org/saref4lift/canConnectToNetwork"/>
        </owl:onProperty>
      </owl:Restriction>
    </rdfs:subClassOf>
    <rdfs:label xml:lang="en">Smart lift Installation</rdfs:label>
    <rdfs:subClassOf rdf:resource="https://saref.etsi.org/saref4syst/System"/>
    <rdfs:subClassOf>
      <owl:Restriction>
        <owl:minCardinality rdf:datatype="http://www.w3.org/2001/XMLSchema#integer"
        >1</owl:minCardinality>
        <owl:onProperty>
          <owl:DatatypeProperty rdf:about="https://saref.etsi.org/saref4lift/hasMaintenanceCompany"/>
        </owl:onProperty>
      </owl:Restriction>
    </rdfs:subClassOf>
    <rdfs:subClassOf>
      <owl:Restriction>
        <owl:someValuesFrom rdf:resource="http://www.w3.org/2001/XMLSchema#integer"/>
        <owl:onProperty>
          <owl:DatatypeProperty rdf:about="https://saref.etsi.org/saref4lift/hasStops"/>
        </owl:onProperty>
      </owl:Restriction>
    </rdfs:subClassOf>
    <rdfs:subClassOf rdf:resource="https://saref.etsi.org/saref4lift/ElectricPowerSystem"/>
    <rdfs:subClassOf>
      <owl:Restriction>
        <owl:someValuesFrom rdf:resource="https://saref.etsi.org/saref4lift/Load"/>
        <owl:onProperty>
          <owl:ObjectProperty rdf:about="https://saref.etsi.org/saref4lift/hasCarloadLimit"/>
        </owl:onProperty>
      </owl:Restriction>
    </rdfs:subClassOf>
  </owl:Class>
  <owl:Class rdf:about="https://saref.etsi.org/saref4lift/SetOutOfServiceCommand">
    <rdfs:label xml:lang="en">Set out of service command</rdfs:label>
    <rdfs:comment xml:lang="en">A type of command to set the lift in Out of Service mode.</rdfs:comment>
    <rdfs:subClassOf rdf:resource="https://saref.etsi.org/core/Command"/>
  </owl:Class>
  <owl:Class rdf:about="https://saref.etsi.org/saref4lift/WarnBatteryPowerState">
    <rdfs:comment xml:lang="en">The state of a system whose battery is functionally in operating conditions but shows signs of reduced capability.</rdfs:comment>
    <rdfs:label xml:lang="en">Warn Battery Power State</rdfs:label>
    <rdfs:subClassOf>
      <owl:Class rdf:about="https://saref.etsi.org/saref4lift/BatteryPowerState"/>
    </rdfs:subClassOf>
  </owl:Class>
  <owl:Class rdf:about="https://saref.etsi.org/saref4lift/DetectedLoadState">
    <rdfs:comment xml:lang="en">The state of a device that detected load. For example when at least one person is in the smart lift car.</rdfs:comment>
    <rdfs:label xml:lang="en">Detected Load state</rdfs:label>
    <rdfs:subClassOf rdf:resource="https://saref.etsi.org/core/State"/>
  </owl:Class>
  <owl:Class rdf:about="https://saref.etsi.org/saref4lift/DownwardTravelsStatistics">
    <rdfs:comment xml:lang="en">Total counter of the number of downward travels since the last reset. As per concept historyPeriodic in ISO 16484-5</rdfs:comment>
    <rdfs:label xml:lang="en">Downward Travels Statistics</rdfs:label>
    <rdfs:subClassOf rdf:resource="https://saref.etsi.org/saref4lift/StatisticsMeasurement"/>
  </owl:Class>
  <owl:Class rdf:about="https://saref.etsi.org/saref4lift/BatteryPowerState">
    <rdfs:comment xml:lang="en">The state of a battery power supply.</rdfs:comment>
    <rdfs:label xml:lang="en">Battery Power State</rdfs:label>
    <rdfs:subClassOf rdf:resource="https://saref.etsi.org/core/State"/>
  </owl:Class>
  <owl:Class rdf:about="https://saref.etsi.org/saref4lift/Network">
    <rdfs:comment xml:lang="en">The class of communication networks.</rdfs:comment>
    <rdfs:label xml:lang="en">Network</rdfs:label>
    <rdfs:subClassOf rdf:resource="https://saref.etsi.org/saref4syst/System"/>
  </owl:Class>
  <owl:Class rdf:about="https://saref.etsi.org/saref4lift/AlarmState">
    <rdfs:comment xml:lang="en">State of a device when a high priority signal is used to attract the operator’s attention to important deviations or abnormal events in the device operation.</rdfs:comment>
    <rdfs:label xml:lang="en">Alarm State</rdfs:label>
    <rdfs:subClassOf rdf:resource="https://saref.etsi.org/core/State"/>
  </owl:Class>
  <owl:Class rdf:about="https://saref.etsi.org/saref4lift/InspectionOperationState">
    <rdfs:comment xml:lang="en">The state of a device that is subject to inspection operation by the maintenance technician</rdfs:comment>
    <rdfs:label xml:lang="en">Inspection operation state</rdfs:label>
    <rdfs:subClassOf rdf:resource="https://saref.etsi.org/core/State"/>
  </owl:Class>
  <owl:Class rdf:about="https://saref.etsi.org/saref4lift/UpwardTravelsStatistics">
    <rdfs:comment xml:lang="en">Total counter of the number of upward travels since the last reset. As per concept historyPeriodic in ISO 16484-5</rdfs:comment>
    <rdfs:label xml:lang="en">Upward Travels Statistics</rdfs:label>
    <rdfs:subClassOf rdf:resource="https://saref.etsi.org/saref4lift/StatisticsMeasurement"/>
  </owl:Class>
  <owl:Class rdf:about="https://saref.etsi.org/saref4lift/FireOperationState">
    <rdfs:comment xml:lang="en">The state of a device that is subject to fire operation, according to EN 81-73 (EN 81-77 for anti-seismic lifts).</rdfs:comment>
    <rdfs:label xml:lang="en">Fire operation state</rdfs:label>
    <rdfs:subClassOf rdf:resource="https://saref.etsi.org/core/State"/>
  </owl:Class>
  <owl:Class rdf:about="https://saref.etsi.org/saref4lift/HydraulicDevice">
    <rdfs:comment xml:lang="en">The class of devices with hydraulic principle of functioning.</rdfs:comment>
    <rdfs:label xml:lang="en">Hydraulic device</rdfs:label>
    <rdfs:subClassOf rdf:resource="https://saref.etsi.org/core/Device"/>
  </owl:Class>
  <owl:Class rdf:about="https://saref.etsi.org/saref4lift/StatusSignal">
    <rdfs:comment xml:lang="en">A signal associated to some state of a device.</rdfs:comment>
    <rdfs:label xml:lang="en">Status signal</rdfs:label>
    <rdfs:subClassOf>
      <owl:Restriction>
        <owl:someValuesFrom rdf:resource="https://saref.etsi.org/core/State"/>
        <owl:onProperty>
          <owl:ObjectProperty rdf:about="https://saref.etsi.org/saref4lift/conveys"/>
        </owl:onProperty>
      </owl:Restriction>
    </rdfs:subClassOf>
    <rdfs:subClassOf>
      <owl:Class rdf:about="https://saref.etsi.org/saref4lift/Signal"/>
    </rdfs:subClassOf>
  </owl:Class>
  <owl:Class rdf:about="https://saref.etsi.org/saref4lift/GoodsSmartLift">
    <rdfs:comment xml:lang="en">The class of Smart Lifts that are used for goods.</rdfs:comment>
    <rdfs:label xml:lang="en">Goods smart lift</rdfs:label>
    <rdfs:subClassOf rdf:resource="https://saref.etsi.org/saref4lift/SmartLiftInstallation"/>
  </owl:Class>
  <owl:Class rdf:about="https://saref.etsi.org/saref4lift/Signal">
    <rdfs:comment xml:lang="en">The class of signals that are conveying some information (e.g., Measurement, State) about a Feature of Interest, at some timestamp.</rdfs:comment>
    <rdfs:label xml:lang="en">Signal</rdfs:label>
    <rdfs:subClassOf>
      <owl:Restriction>
        <owl:someValuesFrom rdf:resource="http://www.w3.org/2001/XMLSchema#dateTime"/>
        <owl:onProperty rdf:resource="https://saref.etsi.org/core/hasTimestamp"/>
      </owl:Restriction>
    </rdfs:subClassOf>
    <rdfs:subClassOf>
      <owl:Restriction>
        <owl:someValuesFrom rdf:resource="http://www.w3.org/2002/07/owl#Thing"/>
        <owl:onProperty>
          <owl:ObjectProperty rdf:about="https://saref.etsi.org/saref4lift/conveys"/>
        </owl:onProperty>
      </owl:Restriction>
    </rdfs:subClassOf>
    <rdfs:subClassOf>
      <owl:Restriction>
        <owl:someValuesFrom rdf:resource="https://saref.etsi.org/core/FeatureOfInterest"/>
        <owl:onProperty rdf:resource="https://saref.etsi.org/core/isAbout"/>
      </owl:Restriction>
    </rdfs:subClassOf>
  </owl:Class>
  <owl:Class rdf:about="https://saref.etsi.org/saref4lift/ElectricalDevice">
    <rdfs:comment xml:lang="en">The class of devices with electrical principle of functioning.</rdfs:comment>
    <rdfs:label xml:lang="en">Electrical device</rdfs:label>
    <rdfs:subClassOf rdf:resource="https://saref.etsi.org/core/Device"/>
  </owl:Class>
  <owl:Class rdf:about="https://saref.etsi.org/saref4lift/SmartLiftCar">
    <rdfs:subClassOf>
      <owl:Restriction>
        <owl:someValuesFrom rdf:resource="https://saref.etsi.org/saref4lift/DoorConnectionPoint"/>
        <owl:onProperty rdf:resource="https://saref.etsi.org/saref4syst/connectsAt"/>
      </owl:Restriction>
    </rdfs:subClassOf>
    <rdfs:subClassOf rdf:resource="https://saref.etsi.org/saref4syst/System"/>
    <rdfs:subClassOf rdf:resource="https://saref.etsi.org/core/FeatureOfInterest"/>
    <rdfs:subClassOf rdf:resource="https://saref.etsi.org/saref4bldg/BuildingSpace"/>
    <rdfs:comment xml:lang="en">The car of a smart lift installation.</rdfs:comment>
    <rdfs:label xml:lang="en">Smart Lift Car</rdfs:label>
  </owl:Class>
  <owl:Class rdf:about="https://saref.etsi.org/saref4lift/TotalReversalDirectionStatistics">
    <rdfs:comment xml:lang="en">Total counter of the number of reversal directions since the last reset. As per concept historyPeriodic in ISO 16484-5</rdfs:comment>
    <rdfs:label xml:lang="en">Total reversal direction statistics</rdfs:label>
    <rdfs:subClassOf rdf:resource="https://saref.etsi.org/saref4lift/StatisticsMeasurement"/>
  </owl:Class>
  <owl:Class rdf:about="https://saref.etsi.org/saref4lift/FirefightersSmartLift">
    <rdfs:comment xml:lang="en">The class of Firefighters Smart Lifts, as per [EN 81-72].</rdfs:comment>
    <rdfs:label xml:lang="en">Firefighters smart lift</rdfs:label>
    <rdfs:subClassOf rdf:resource="https://saref.etsi.org/saref4lift/SmartLiftInstallation"/>
  </owl:Class>
  <owl:Class rdf:about="https://saref.etsi.org/saref4lift/PossibleSmartLiftCarService">
    <rdfs:comment xml:lang="en">A possible connection between a car stop space of a smart lift installation, a building space it can serve, and the door of the smart lift car used to serve this building space.</rdfs:comment>
    <rdfs:label xml:lang="en">Possible Smart lift car service</rdfs:label>
    <rdfs:subClassOf>
      <owl:Restriction>
        <owl:someValuesFrom rdf:resource="https://saref.etsi.org/saref4bldg/BuildingSpace"/>
        <owl:onProperty rdf:resource="https://saref.etsi.org/saref4syst/connectsSystem"/>
      </owl:Restriction>
    </rdfs:subClassOf>
    <rdfs:subClassOf>
      <owl:Restriction>
        <owl:someValuesFrom rdf:resource="https://saref.etsi.org/saref4lift/DoorConnectionPoint"/>
        <owl:onProperty rdf:resource="https://saref.etsi.org/saref4syst/connectsSystemAt"/>
      </owl:Restriction>
    </rdfs:subClassOf>
    <rdfs:subClassOf>
      <owl:Restriction>
        <owl:someValuesFrom rdf:resource="https://saref.etsi.org/saref4lift/CarStopSpace"/>
        <owl:onProperty rdf:resource="https://saref.etsi.org/saref4syst/connectsSystem"/>
      </owl:Restriction>
    </rdfs:subClassOf>
    <rdfs:subClassOf rdf:resource="https://saref.etsi.org/saref4syst/Connection"/>
  </owl:Class>
  <owl:Class rdf:about="https://saref.etsi.org/saref4lift/FloodInTheWellState">
    <rdfs:comment xml:lang="en">The state of a lift where a flood is detected in the well.</rdfs:comment>
    <rdfs:label xml:lang="en">Flood in the well state</rdfs:label>
    <rdfs:subClassOf rdf:resource="https://saref.etsi.org/saref4lift/AlarmState"/>
  </owl:Class>
  <owl:Class rdf:about="https://saref.etsi.org/saref4lift/SmartLiftCarService">
    <rdfs:comment xml:lang="en">A connection between a car stop space of a smart lift installation, a building space it can serve, and the door of the smart lift car used to serve this building space.</rdfs:comment>
    <rdfs:label xml:lang="en">Smart lift car service</rdfs:label>
    <rdfs:subClassOf rdf:resource="https://saref.etsi.org/saref4lift/PossibleSmartLiftCarService"/>
  </owl:Class>
  <owl:Class rdf:about="https://saref.etsi.org/saref4lift/ThreePhaseConnectionPoint">
    <rdfs:subClassOf rdf:resource="https://saref.etsi.org/saref4lift/ElectricalConnectionPoint"/>
    <rdfs:comment xml:lang="en">A three-phase connection point is a connection point composed of four wires (plus the protective earth): 

- wires R, S, T, for the phases;
- wire N for the neutral.
</rdfs:comment>
    <rdfs:label xml:lang="en">Three-Phase Connection Point</rdfs:label>
  </owl:Class>
  <owl:Class rdf:about="https://saref.etsi.org/saref4lift/OverloadedState">
    <rdfs:comment xml:lang="en">The state of a device that is overloaded.</rdfs:comment>
    <rdfs:label xml:lang="en">Overloaded state</rdfs:label>
    <rdfs:subClassOf rdf:resource="https://saref.etsi.org/core/State"/>
  </owl:Class>
  <owl:Class rdf:about="http://www.opengis.net/ont/sf#Point">
    <rdfs:label xml:lang="en">Point</rdfs:label>
    <rdfs:isDefinedBy rdf:resource="http://www.opengis.net/ont/sf#"/>
    <rdfs:subClassOf rdf:resource="http://www.opengis.net/ont/geosparql#Geometry"/>
  </owl:Class>
  <owl:Class rdf:about="https://saref.etsi.org/saref4lift/SmartLiftInstallationFaultState">
    <rdfs:comment xml:lang="en">A faulty state of a smart lift. The fault rdf:label shall be one of the values defined in EN 627, (e.g.: "01xx" broken security chain).</rdfs:comment>
    <rdfs:label xml:lang="en">Smart lift installation fault state state</rdfs:label>
    <rdfs:subClassOf rdf:resource="https://saref.etsi.org/core/State"/>
  </owl:Class>
  <owl:Class rdf:about="https://saref.etsi.org/saref4lift/AlarmInTheCarState">
    <rdfs:comment xml:lang="en">State of a device when the alarm in a car has been activated.</rdfs:comment>
    <rdfs:label xml:lang="en">Alarm in the car state</rdfs:label>
    <rdfs:subClassOf rdf:resource="https://saref.etsi.org/saref4lift/AlarmState"/>
  </owl:Class>
  <owl:ObjectProperty rdf:about="https://saref.etsi.org/saref4lift/hasShaftTemperature">
    <rdfs:comment xml:lang="en">A relationship between a smart lift installation and the temperature of the shaft.</rdfs:comment>
    <rdfs:label xml:lang="en">has shaft temperature</rdfs:label>
    <rdfs:range rdf:resource="https://saref.etsi.org/core/Temperature"/>
    <rdfs:domain rdf:resource="https://saref.etsi.org/saref4lift/SmartLiftInstallation"/>
    <rdfs:subPropertyOf rdf:resource="https://saref.etsi.org/core/hasProperty"/>
  </owl:ObjectProperty>
  <owl:ObjectProperty rdf:about="https://saref.etsi.org/saref4lift/hasReceivedSignalStrengthIndicator">
    <rdfs:comment xml:lang="en">Received Signal Strength Indicator of the network access. (via AT commands from the transmission module):
0: -113 dBm or lower quality;
1: -111 dBm;
2 .. 30: -109 dBm .. -53 dBm;
31: -51 dBm or greater;
99: Not Known or non-detectable.</rdfs:comment>
    <rdfs:label xml:lang="en">has Received Signal Strength Indicator</rdfs:label>
    <rdfs:range rdf:resource="https://saref.etsi.org/core/Property"/>
    <rdfs:domain rdf:resource="https://saref.etsi.org/saref4lift/NetworkAccess"/>
    <rdfs:subPropertyOf rdf:resource="https://saref.etsi.org/core/hasProperty"/>
  </owl:ObjectProperty>
  <owl:ObjectProperty rdf:about="https://saref.etsi.org/saref4lift/isSecondaryInGroup">
    <rdfs:label xml:lang="en">is secondary in group</rdfs:label>
    <rdfs:comment xml:lang="en">the smart lift installation acts as depends from the master smart lift installation in the smart lift group for the common capabilities.</rdfs:comment>
    <rdfs:subPropertyOf>
      <owl:ObjectProperty rdf:about="https://saref.etsi.org/saref4lift/isGroupedIn"/>
    </rdfs:subPropertyOf>
    <rdfs:range rdf:resource="https://saref.etsi.org/saref4lift/SmartLiftGroup"/>
    <rdfs:domain rdf:resource="https://saref.etsi.org/saref4lift/SmartLiftInstallation"/>
  </owl:ObjectProperty>
  <owl:ObjectProperty rdf:about="https://saref.etsi.org/saref4lift/connectedToEmergencyBattery">
    <rdfs:label xml:lang="en">connected to emergency battery</rdfs:label>
    <rdfs:comment xml:lang="en">A relationship defining the emergency battery of an electric power system.</rdfs:comment>
    <rdfs:range rdf:resource="https://saref.etsi.org/saref4lift/ElectricPowerSystem"/>
    <rdfs:domain rdf:resource="https://saref.etsi.org/saref4lift/ElectricPowerSystem"/>
    <rdfs:subPropertyOf rdf:resource="https://saref.etsi.org/saref4syst/connectedTo"/>
  </owl:ObjectProperty>
  <owl:ObjectProperty rdf:about="https://saref.etsi.org/saref4lift/hasCarService">
    <rdfs:comment xml:lang="en">A relationship between a system and a car service.</rdfs:comment>
    <rdfs:label xml:lang="en">has car service</rdfs:label>
    <rdfs:range rdf:resource="https://saref.etsi.org/saref4lift/PossibleSmartLiftCarService"/>
    <rdfs:domain rdf:resource="https://saref.etsi.org/saref4lift/SmartLiftInstallation"/>
    <rdfs:subPropertyOf rdf:resource="https://saref.etsi.org/saref4syst/connectedThrough"/>
  </owl:ObjectProperty>
  <owl:ObjectProperty rdf:about="https://saref.etsi.org/saref4lift/hasMainPowerSupply">
    <rdfs:label xml:lang="en">has main power supply</rdfs:label>
    <rdfs:comment xml:lang="en">A relationship defining the main power supply of an electric power system.</rdfs:comment>
    <rdfs:range rdf:resource="https://saref.etsi.org/saref4lift/ElectricalConnectionPoint"/>
    <rdfs:domain rdf:resource="https://saref.etsi.org/saref4lift/ElectricPowerSystem"/>
    <rdfs:subPropertyOf rdf:resource="https://saref.etsi.org/saref4syst/connectsAt"/>
  </owl:ObjectProperty>
  <owl:ObjectProperty rdf:about="https://saref.etsi.org/saref4lift/hasCoverage">
    <rdfs:comment xml:lang="en">Coverage of the network</rdfs:comment>
    <rdfs:label xml:lang="en">has coverage</rdfs:label>
    <rdfs:range rdf:resource="https://saref.etsi.org/core/Property"/>
    <rdfs:domain rdf:resource="https://saref.etsi.org/saref4lift/NetworkAccess"/>
    <rdfs:subPropertyOf rdf:resource="https://saref.etsi.org/core/hasProperty"/>
  </owl:ObjectProperty>
  <owl:ObjectProperty rdf:about="https://saref.etsi.org/saref4lift/containsCar">
    <rdfs:label xml:lang="en">contains car</rdfs:label>
    <rdfs:comment xml:lang="en">A relationship between a smart lift installation and its car.</rdfs:comment>
    <rdfs:subPropertyOf rdf:resource="https://saref.etsi.org/saref4bldg/hasSpace"/>
    <rdfs:range rdf:resource="https://saref.etsi.org/saref4lift/SmartLiftCar"/>
    <rdfs:domain rdf:resource="https://saref.etsi.org/saref4lift/SmartLiftInstallation"/>
  </owl:ObjectProperty>
  <owl:ObjectProperty rdf:about="https://saref.etsi.org/saref4lift/hasChannelBitErrorRate">
    <rdfs:comment xml:lang="en">Channel Bit Error Rate (via AT commands from the module); 0..7 as for RXQUAL defined by ETSI TS 145 008</rdfs:comment>
    <rdfs:label xml:lang="en">has Channel Bit Error Rate</rdfs:label>
    <rdfs:range rdf:resource="https://saref.etsi.org/core/Property"/>
    <rdfs:domain rdf:resource="https://saref.etsi.org/saref4lift/NetworkAccess"/>
    <rdfs:subPropertyOf rdf:resource="https://saref.etsi.org/core/hasProperty"/>
  </owl:ObjectProperty>
  <owl:ObjectProperty rdf:about="http://www.opengis.net/ont/geosparql#hasGeometry">
    <rdfs:range rdf:resource="http://www.opengis.net/ont/geosparql#Geometry"/>
    <rdfs:domain rdf:resource="http://www.opengis.net/ont/geosparql#Feature"/>
    <rdfs:comment xml:lang="en">A spatial representation for a given feature.</rdfs:comment>
    <rdfs:label xml:lang="en">hasGeometry</rdfs:label>
    <rdfs:isDefinedBy rdf:resource="http://www.opengis.net/ont/geosparql#"/>
  </owl:ObjectProperty>
  <owl:ObjectProperty rdf:about="https://saref.etsi.org/saref4lift/hasAlarmSOSSystem">
    <rdfs:label xml:lang="en">has alarm SOS system</rdfs:label>
    <rdfs:comment xml:lang="en">A relationship defining the alarm SOS subsystem of a system.</rdfs:comment>
    <rdfs:range rdf:resource="https://saref.etsi.org/saref4syst/System"/>
    <rdfs:domain rdf:resource="https://saref.etsi.org/saref4syst/System"/>
    <rdfs:subPropertyOf rdf:resource="https://saref.etsi.org/saref4syst/hasSubSystem"/>
  </owl:ObjectProperty>
  <owl:ObjectProperty rdf:about="https://saref.etsi.org/saref4lift/hasStandardPowerSupply">
    <rdfs:label xml:lang="en">has standard power supply</rdfs:label>
    <rdfs:comment xml:lang="en">A relationship defining the standard power supply of an electric power system.</rdfs:comment>
    <rdfs:range rdf:resource="https://saref.etsi.org/saref4lift/ElectricalConnectionPoint"/>
    <rdfs:domain rdf:resource="https://saref.etsi.org/saref4lift/ElectricPowerSystem"/>
    <rdfs:subPropertyOf rdf:resource="https://saref.etsi.org/saref4syst/connectsAt"/>
  </owl:ObjectProperty>
  <owl:ObjectProperty rdf:about="https://saref.etsi.org/saref4lift/hasTimeOfLastPeriodicTest72hAttempt">
    <rdfs:comment xml:lang="en">A relationship to the time of the last periodic test 72h attempt of a lift. In UE and other applicable countries, the periodic test shall comply with EN 81.28</rdfs:comment>
    <rdfs:label xml:lang="en">has time of last periodic test 72h attempt</rdfs:label>
    <rdfs:domain rdf:resource="https://saref.etsi.org/saref4lift/SmartLiftInstallation"/>
    <rdfs:subPropertyOf rdf:resource="https://saref.etsi.org/core/hasProperty"/>
  </owl:ObjectProperty>
  <owl:ObjectProperty rdf:about="https://saref.etsi.org/saref4lift/canConnectToNetwork">
    <rdfs:comment xml:lang="en">A relationship between a system and a network it can connect to.</rdfs:comment>
    <rdfs:label xml:lang="en">can connect to network</rdfs:label>
    <rdfs:range rdf:resource="https://saref.etsi.org/saref4lift/Network"/>
    <rdfs:domain rdf:resource="https://saref.etsi.org/saref4syst/System"/>
    <rdfs:subPropertyOf rdf:resource="https://saref.etsi.org/saref4syst/connectedTo"/>
  </owl:ObjectProperty>
  <owl:ObjectProperty rdf:about="https://saref.etsi.org/saref4lift/hasTimeOfConfirmationOfLastPeriodicTest72hAttempt">
    <rdfs:comment xml:lang="en">A relationship to the time of the confirmation of the last periodic test 72h attempt of a lift. In UE and other applicable countries, the periodic test shall comply with EN 81.28</rdfs:comment>
    <rdfs:label xml:lang="en">has time of confirmation of last periodic test 72h attempt</rdfs:label>
    <rdfs:domain rdf:resource="https://saref.etsi.org/saref4lift/SmartLiftInstallation"/>
    <rdfs:subPropertyOf rdf:resource="https://saref.etsi.org/core/hasProperty"/>
  </owl:ObjectProperty>
  <owl:ObjectProperty rdf:about="https://saref.etsi.org/saref4lift/hasCarTemperature">
    <rdfs:comment xml:lang="en">A relationship between a smart lift installation and the temperature of the smart lift car.</rdfs:comment>
    <rdfs:label xml:lang="en">has car temperature</rdfs:label>
    <rdfs:range rdf:resource="https://saref.etsi.org/core/Temperature"/>
    <rdfs:domain rdf:resource="https://saref.etsi.org/saref4lift/SmartLiftInstallation"/>
    <rdfs:subPropertyOf rdf:resource="https://saref.etsi.org/core/hasProperty"/>
  </owl:ObjectProperty>
  <owl:ObjectProperty rdf:about="https://saref.etsi.org/saref4lift/isPeerInGroup">
    <rdfs:label xml:lang="en">is peer in group</rdfs:label>
    <rdfs:comment xml:lang="en">the smart lift installation is part of an smart lift group and composed by peers smart lift installation respect to the common capabilities.</rdfs:comment>
    <rdfs:subPropertyOf>
      <owl:ObjectProperty rdf:about="https://saref.etsi.org/saref4lift/isGroupedIn"/>
    </rdfs:subPropertyOf>
    <rdfs:range rdf:resource="https://saref.etsi.org/saref4lift/SmartLiftGroup"/>
    <rdfs:domain rdf:resource="https://saref.etsi.org/saref4lift/SmartLiftInstallation"/>
  </owl:ObjectProperty>
  <owl:ObjectProperty rdf:about="https://saref.etsi.org/saref4lift/isMasterInGroup">
    <rdfs:label xml:lang="en">is master in group</rdfs:label>
    <rdfs:comment xml:lang="en">the smart lift installation acts as master for the common capabilities in the smart lift group.</rdfs:comment>
    <rdfs:subPropertyOf>
      <owl:ObjectProperty rdf:about="https://saref.etsi.org/saref4lift/isGroupedIn"/>
    </rdfs:subPropertyOf>
    <rdfs:range rdf:resource="https://saref.etsi.org/saref4lift/SmartLiftGroup"/>
    <rdfs:domain rdf:resource="https://saref.etsi.org/saref4lift/SmartLiftInstallation"/>
  </owl:ObjectProperty>
  <owl:ObjectProperty rdf:about="https://saref.etsi.org/saref4lift/hasEngineRoomTemperature">
    <rdfs:comment xml:lang="en">A relationship between a smart lift installation and the temperature of the engine room.</rdfs:comment>
    <rdfs:label xml:lang="en">has engine room temperature</rdfs:label>
    <rdfs:range rdf:resource="https://saref.etsi.org/core/Temperature"/>
    <rdfs:domain rdf:resource="https://saref.etsi.org/saref4lift/SmartLiftInstallation"/>
    <rdfs:subPropertyOf rdf:resource="https://saref.etsi.org/core/hasProperty"/>
  </owl:ObjectProperty>
  <owl:ObjectProperty rdf:about="https://saref.etsi.org/saref4lift/hasVoltage">
    <rdfs:range rdf:resource="https://saref.etsi.org/saref4lift/Voltage"/>
    <rdfs:domain rdf:resource="https://saref.etsi.org/core/FeatureOfInterest"/>
    <rdfs:subPropertyOf rdf:resource="https://saref.etsi.org/core/hasProperty"/>
    <rdfs:comment xml:lang="en">A relationship defining the voltage of a feature of interest.</rdfs:comment>
    <rdfs:label xml:lang="en">has voltage</rdfs:label>
  </owl:ObjectProperty>
  <owl:ObjectProperty rdf:about="https://saref.etsi.org/saref4lift/hasCarloadLimit">
    <rdfs:label xml:lang="en">has carload limit load</rdfs:label>
    <rdfs:comment xml:lang="en">A relationship defining the limit load to be safely carried by the car, as a design parameter.</rdfs:comment>
    <rdfs:range rdf:resource="https://saref.etsi.org/saref4lift/Load"/>
    <rdfs:domain rdf:resource="https://saref.etsi.org/saref4lift/SmartLiftCar"/>
  </owl:ObjectProperty>
  <owl:ObjectProperty rdf:about="https://saref.etsi.org/saref4lift/hasElectricPowerConsumption">
    <rdfs:comment xml:lang="en">A relationship between a feature of interest and its power consumption. If a property of a s4syst:System, or the property of a s4syst:ConnectionPoint thereof, by convention the power consumption is positive if the electric energy enters the system.</rdfs:comment>
    <rdfs:label xml:lang="en">has power consumption</rdfs:label>
    <rdfs:range rdf:resource="https://saref.etsi.org/core/Energy"/>
    <rdfs:domain rdf:resource="https://saref.etsi.org/core/FeatureOfInterest"/>
    <rdfs:subPropertyOf rdf:resource="https://saref.etsi.org/core/hasProperty"/>
  </owl:ObjectProperty>
  <owl:ObjectProperty rdf:about="https://saref.etsi.org/saref4lift/conveys">
    <rdfs:label xml:lang="en">conveys</rdfs:label>
    <rdfs:comment xml:lang="en">A relationship specifying an information (e.g., measurement, state) that is conveyed by a signal</rdfs:comment>
    <rdfs:domain rdf:resource="https://saref.etsi.org/saref4lift/Signal"/>
  </owl:ObjectProperty>
  <owl:ObjectProperty rdf:about="https://saref.etsi.org/saref4lift/isGroupedIn">
    <rdfs:label xml:lang="en">is grouped in</rdfs:label>
    <rdfs:comment xml:lang="en">A relationship specifying the smart lift installations grouped into smart lift groups</rdfs:comment>
    <rdfs:range rdf:resource="https://saref.etsi.org/saref4lift/SmartLiftGroup"/>
    <rdfs:domain rdf:resource="https://saref.etsi.org/saref4lift/SmartLiftInstallation"/>
  </owl:ObjectProperty>
  <owl:DatatypeProperty rdf:about="https://saref.etsi.org/saref4lift/hasDoors">
    <rdfs:label xml:lang="en">has doors</rdfs:label>
    <rdfs:comment xml:lang="en">The number of door connection points in a building space (e.g., a smart lift car) </rdfs:comment>
    <rdfs:range rdf:resource="http://www.w3.org/2001/XMLSchema#integer"/>
    <rdfs:domain rdf:resource="https://saref.etsi.org/saref4bldg/BuildingSpace"/>
  </owl:DatatypeProperty>
  <owl:DatatypeProperty rdf:about="https://saref.etsi.org/saref4lift/hasManufacturingCompanyRepresentative">
    <rdfs:label xml:lang="en">has manufacturing company representative</rdfs:label>
    <rdfs:comment xml:lang="en">A relationship identifying the local representative of the manufacturing company of a system, as per [ISO 16484-5: Profile_Name]. The value is expected to be a string or a string with language tag.</rdfs:comment>
    <rdfs:domain rdf:resource="https://saref.etsi.org/saref4syst/System"/>
  </owl:DatatypeProperty>
  <owl:DatatypeProperty rdf:about="https://saref.etsi.org/saref4lift/hasDoorCloseTime">
    <rdfs:label xml:lang="en">has door close time</rdfs:label>
    <rdfs:comment xml:lang="en">A relationship defining the time spent by an entity (e.g., a lift, a building space, a door) to close its doors</rdfs:comment>
    <rdfs:range rdf:resource="http://www.w3.org/2001/XMLSchema#duration"/>
    <rdfs:domain rdf:resource="https://saref.etsi.org/core/FeatureOfInterest"/>
  </owl:DatatypeProperty>
  <owl:DatatypeProperty rdf:about="https://saref.etsi.org/saref4lift/hasBuildingManager">
    <rdfs:label xml:lang="en">has building manager</rdfs:label>
    <rdfs:comment xml:lang="en">A relationship identifying the manager of the building where a system is located, as per [ISO 16484-5: inclusion in Description Property]. The value is expected to be a string or a string with language tag.</rdfs:comment>
    <rdfs:domain rdf:resource="https://saref.etsi.org/saref4syst/System"/>
  </owl:DatatypeProperty>
  <owl:DatatypeProperty rdf:about="https://saref.etsi.org/saref4lift/hasStops">
    <rdfs:label xml:lang="en">has stops</rdfs:label>
    <rdfs:comment xml:lang="en">The number of stops by an entity (e.g., a lift) </rdfs:comment>
    <rdfs:range rdf:resource="http://www.w3.org/2001/XMLSchema#integer"/>
    <rdfs:domain rdf:resource="https://saref.etsi.org/saref4syst/System"/>
  </owl:DatatypeProperty>
  <owl:DatatypeProperty rdf:about="https://saref.etsi.org/saref4lift/hasInstallerCompany">
    <rdfs:label xml:lang="en">has installer company</rdfs:label>
    <rdfs:comment xml:lang="en">A relationship identifying the installer company of a system (e.g., device), as per [ISO 16484-5: inclusion in Description Property]. The value is expected to be a string or a string with language tag.</rdfs:comment>
    <rdfs:domain rdf:resource="https://saref.etsi.org/saref4syst/System"/>
  </owl:DatatypeProperty>
  <owl:DatatypeProperty rdf:about="https://saref.etsi.org/saref4lift/hasLegalOwner">
    <rdfs:label xml:lang="en">has legal owner</rdfs:label>
    <rdfs:comment xml:lang="en">A relationship identifying the legal owner of a system, as per [ISO 16484-5: inclusion in Description Property]. The value is expected to be a string or a string with language tag.</rdfs:comment>
    <rdfs:domain rdf:resource="https://saref.etsi.org/saref4syst/System"/>
  </owl:DatatypeProperty>
  <owl:DatatypeProperty rdf:about="https://saref.etsi.org/saref4lift/hasSecondaryEmergencyTelephoneNumber">
    <rdfs:label xml:lang="en">has secondary emergency number</rdfs:label>
    <rdfs:comment xml:lang="en">Secondary emergency number to be called in case of emergency. The value is expected to be a URI with the tel: URI scheme as defined RFC 3966.</rdfs:comment>
    <rdfs:range rdf:resource="http://www.w3.org/2001/XMLSchema#anyURI"/>
    <rdfs:domain rdf:resource="https://saref.etsi.org/saref4syst/System"/>
  </owl:DatatypeProperty>
  <owl:DatatypeProperty rdf:about="https://saref.etsi.org/saref4lift/hasTravelTime">
    <rdfs:label xml:lang="en">has travel time</rdfs:label>
    <rdfs:comment xml:lang="en">A relationship defining the time spent by an entity (e.g., a lift car) to travel between stops</rdfs:comment>
    <rdfs:range rdf:resource="http://www.w3.org/2001/XMLSchema#duration"/>
    <rdfs:domain rdf:resource="https://saref.etsi.org/core/FeatureOfInterest"/>
  </owl:DatatypeProperty>
  <owl:DatatypeProperty rdf:about="https://saref.etsi.org/saref4lift/hasCarServices">
    <rdfs:label xml:lang="en">has car services</rdfs:label>
    <rdfs:comment xml:lang="en">The number of car services, taking care of the case where the car has multiple doors that give independent access to different locations on a given floor. It is expected to be greater or equal to the number of Car Stops.</rdfs:comment>
    <rdfs:range rdf:resource="http://www.w3.org/2001/XMLSchema#integer"/>
    <rdfs:domain rdf:resource="https://saref.etsi.org/saref4lift/SmartLiftInstallation"/>
  </owl:DatatypeProperty>
  <owl:DatatypeProperty rdf:about="https://saref.etsi.org/saref4lift/hasMainEmergencyTelephoneNumber">
    <rdfs:label xml:lang="en">has main emergency telephone number</rdfs:label>
    <rdfs:comment xml:lang="en">Main emergency telephone number to be called in case of emergency. The value is expected to be a URI with the tel: URI scheme as defined RFC 3966.</rdfs:comment>
    <rdfs:range rdf:resource="http://www.w3.org/2001/XMLSchema#anyURI"/>
    <rdfs:domain rdf:resource="https://saref.etsi.org/saref4syst/System"/>
  </owl:DatatypeProperty>
  <owl:DatatypeProperty rdf:about="https://saref.etsi.org/saref4lift/hasTelephoneNumber">
    <rdfs:label xml:lang="en">has telephone number</rdfs:label>
    <rdfs:comment xml:lang="en">Number corresponding to the lift communication module to be used for call terminated to the lift car. The value is expected to be a URI with the tel: URI scheme as defined RFC 3966.</rdfs:comment>
    <rdfs:range rdf:resource="http://www.w3.org/2001/XMLSchema#anyURI"/>
    <rdfs:domain rdf:resource="https://saref.etsi.org/saref4syst/System"/>
  </owl:DatatypeProperty>
  <owl:DatatypeProperty rdf:about="https://saref.etsi.org/saref4lift/hasGeographicLocationValidator">
    <rdfs:label xml:lang="en">has geographic location validator</rdfs:label>
    <rdfs:comment xml:lang="en">Name of who has provided the validation of the correctness of the geographic location of the system. The value is expected to be a string or a string with language tag.</rdfs:comment>
    <rdfs:domain rdf:resource="https://saref.etsi.org/saref4syst/System"/>
  </owl:DatatypeProperty>
  <owl:DatatypeProperty rdf:about="https://saref.etsi.org/saref4lift/hasDoorOpenTime">
    <rdfs:label xml:lang="en">has door open time</rdfs:label>
    <rdfs:comment xml:lang="en">A relationship defining the time spent by an entity (e.g., a lift, a building space, a door) to open its doors</rdfs:comment>
    <rdfs:range rdf:resource="http://www.w3.org/2001/XMLSchema#duration"/>
    <rdfs:domain rdf:resource="https://saref.etsi.org/core/FeatureOfInterest"/>
  </owl:DatatypeProperty>
  <owl:DatatypeProperty rdf:about="http://www.opengis.net/ont/geosparql#asWKT">
    <rdfs:label xml:lang="en">asWKT</rdfs:label>
    <rdfs:isDefinedBy rdf:resource="http://www.opengis.net/ont/geosparql#"/>
    <rdfs:comment xml:lang="en">The WKT serialization of a geometry</rdfs:comment>
    <rdfs:range rdf:resource="http://www.opengis.net/ont/geosparql#wktLiteral"/>
    <rdfs:domain rdf:resource="http://www.opengis.net/ont/geosparql#Geometry"/>
  </owl:DatatypeProperty>
  <owl:DatatypeProperty rdf:about="https://saref.etsi.org/saref4lift/hasPlateInformation">
    <rdfs:label xml:lang="en">has plate information</rdfs:label>
    <rdfs:comment xml:lang="en">An information usually also inscribed on a plate attached to the lift car.</rdfs:comment>
    <rdfs:range rdf:resource="http://www.w3.org/2001/XMLSchema#string"/>
    <rdfs:domain rdf:resource="https://saref.etsi.org/saref4lift/SmartLiftInstallation"/>
  </owl:DatatypeProperty>
  <owl:DatatypeProperty rdf:about="https://saref.etsi.org/saref4lift/hasMaintenanceCompany">
    <rdfs:label xml:lang="en">has maintenance company</rdfs:label>
    <rdfs:comment xml:lang="en">A relationship identifying the maintenance company of a system, as per [ISO 16484-5: inclusion in Description Property]. The value is expected to be a string or a string with language tag.</rdfs:comment>
    <rdfs:domain rdf:resource="https://saref.etsi.org/saref4syst/System"/>
  </owl:DatatypeProperty>
  <owl:DatatypeProperty rdf:about="https://saref.etsi.org/saref4lift/hasInspectionAuthority">
    <rdfs:label xml:lang="en">has inspection authority</rdfs:label>
    <rdfs:comment xml:lang="en">A relationship identifying the Authority that is entitled to periodically inspect the system installation and certify its suitability for the intended use, as per [ISO 16484-5: inclusion in Description Property]. The value is expected to be a string or a string with language tag.</rdfs:comment>
    <rdfs:domain rdf:resource="https://saref.etsi.org/saref4syst/System"/>
  </owl:DatatypeProperty>
  <owl:DatatypeProperty rdf:about="https://saref.etsi.org/saref4lift/hasAlarmMonitoringCentre">
    <rdfs:label xml:lang="en">has alarm monitoring centre</rdfs:label>
    <rdfs:comment xml:lang="en">A relationship identifying the monitoring centre of the alarms, as per [ISO 16484-5: inclusion in Description Property]. The value is expected to be a string or a string with language tag.</rdfs:comment>
    <rdfs:domain rdf:resource="https://saref.etsi.org/saref4syst/System"/>
  </owl:DatatypeProperty>
  <s4lift:Network rdf:about="https://saref.etsi.org/saref4lift/Network3G">
    <rdfs:comment xml:lang="en">The 3G Network</rdfs:comment>
    <rdfs:label xml:lang="en">Network 3G</rdfs:label>
    <rdf:type rdf:resource="http://www.w3.org/2002/07/owl#NamedIndividual"/>
  </s4lift:Network>
  <owl:AnnotationProperty rdf:about="http://purl.org/dc/terms/description"/>
  <s4lift:Network rdf:about="https://saref.etsi.org/saref4lift/Network2G">
    <rdfs:comment xml:lang="en">The 2G Network</rdfs:comment>
    <rdfs:label xml:lang="en">Network 2G</rdfs:label>
    <rdf:type rdf:resource="http://www.w3.org/2002/07/owl#NamedIndividual"/>
  </s4lift:Network>
  <owl:AnnotationProperty rdf:about="http://purl.org/dc/terms/publisher"/>
  <owl:AnnotationProperty rdf:about="http://purl.org/dc/terms/source"/>
  <owl:AnnotationProperty rdf:about="http://purl.org/vocab/vann/preferredNamespaceUri"/>
  <s4lift:Network rdf:about="https://saref.etsi.org/saref4lift/Network5G">
    <rdfs:comment xml:lang="en">The 5G Network</rdfs:comment>
    <rdfs:label xml:lang="en">Network 5G</rdfs:label>
    <rdf:type rdf:resource="http://www.w3.org/2002/07/owl#NamedIndividual"/>
  </s4lift:Network>
  <owl:AnnotationProperty rdf:about="http://www.w3.org/2004/02/skos/core#definition"/>
  <owl:AnnotationProperty rdf:about="http://www.w3.org/2002/07/owl#qualifiedCardinality"/>
  <owl:AnnotationProperty rdf:about="http://purl.org/dc/terms/license"/>
  <owl:AnnotationProperty rdf:about="http://purl.org/dc/terms/title"/>
  <s4lift:Network rdf:about="https://saref.etsi.org/saref4lift/Network4G">
    <rdfs:comment xml:lang="en">The 4G Network</rdfs:comment>
    <rdfs:label xml:lang="en">Network 4G</rdfs:label>
    <rdf:type rdf:resource="http://www.w3.org/2002/07/owl#NamedIndividual"/>
  </s4lift:Network>
  <owl:AnnotationProperty rdf:about="http://purl.org/vocab/vann/preferredNamespacePrefix"/>
  <s4lift:Network rdf:about="https://saref.etsi.org/saref4lift/NetworkFixedLine">
    <rdfs:comment xml:lang="en">The fixed line Network</rdfs:comment>
    <rdfs:label xml:lang="en">Network fixed line</rdfs:label>
    <rdf:type rdf:resource="http://www.w3.org/2002/07/owl#NamedIndividual"/>
  </s4lift:Network>
  <owl:AnnotationProperty rdf:about="http://purl.org/dc/terms/modified"/>
</rdf:RDF>
